@prefix dc: <http://purl.org/dc/elements/1.1/> .
@prefix ns: <http://creativecommons.org/ns#> .
@prefix ns1: <http://www.w3.org/2003/06/sw-vocab-status/ns#> .
@prefix ns11: <http://creativecommons.org/ns#> .
@prefix owl: <http://www.w3.org/2002/07/owl#> .
@prefix rdf: <http://www.w3.org/1999/02/22-rdf-syntax-ns#> .
@prefix rdfs: <http://www.w3.org/2000/01/rdf-schema#> .
@prefix skos: <http://www.w3.org/2004/02/skos/core#> .
@prefix terms: <http://purl.org/dc/terms/> .
@prefix vann: <http://purl.org/vocab/vann/> .
@prefix xml: <http://www.w3.org/XML/1998/namespace> .
@prefix xsd: <http://www.w3.org/2001/XMLSchema#> .

ns11:license a owl:AnnotationProperty .

<http://iflastandards.info/ns/fr/frbr/frbroo/CLP104_subject_to> rdfs:label "subject to"@en ;
    rdfs:comment """This property associates a publication, i.e. an instance of F3 Manifestation Product Type, with an instance of E30 Right, which applies to all exemplars of that publication, as long as they are recognised as exemplars of that publication.
The rights covered by this property may include: acquisition or access authorisation; terms of availability; access restrictions on the Manifestation Product Type; etc.
"""@en .

<http://iflastandards.info/ns/fr/frbr/frbroo/CLP104i_applies_to> rdfs:label "applies to"@en ;
    rdfs:comment """
"""@en .

<http://iflastandards.info/ns/fr/frbr/frbroo/CLP105_right_held_by> rdfs:label "right held by"@en ;
    rdfs:comment """This property associates a publication, i.e. an instance of F3 Manifestation Product Type, with an instance of E39 Actor, who holds an instance of E30 Right on all exemplars of that publication, as long as they are recognised as exemplars of that publication.
"""@en .

<http://iflastandards.info/ns/fr/frbr/frbroo/CLP105i_right_on> rdfs:label "right on"@en ;
    rdfs:comment """
"""@en .

<http://iflastandards.info/ns/fr/frbr/frbroo/CLP2_should_have_type> rdfs:label "should have type"@en ;
    rdfs:comment """This property associates a publication, i.e. an instance of F3 Manifestation Product Type, with an instance of E55 Type, which all exemplars of that publication should belong to, as long as they are recognised as exemplars of that publication. Typically, this property is observed on one exemplar of a publication, and extrapolated to all other exemplars of the same publication. This logical inference is an induction along the path that can be modelled as: F3 Manifestation Product Type R7i has example F5 Item P41i was classified by E17 Type Assignment P42 assigned E55 Type.
It can happen that a given exemplar, or subset of exemplars, originally produced, or intended to be produced, with that characteristic, accidentally lacks it. This fact should be recorded as a property of F5 Item, and not of F3 Manifestation Product Type.
"""@en .

<http://iflastandards.info/ns/fr/frbr/frbroo/CLP2i_should_be_type_of> rdfs:label "should be type of"@en ;
    rdfs:comment """
"""@en .

<http://iflastandards.info/ns/fr/frbr/frbroo/CLP43_should_have_dimension> rdfs:label "should have dimension"@en ;
    rdfs:comment """This property associates a publication, i.e. an instance of F3 Manifestation Product Type, with an instance of E54 Dimension, which all exemplars of that publication should have, as long as they are recognised as exemplars of that publication. Typically, this property is observed on one exemplar of a publication, and extrapolated to all other exemplars of the same publication. This logical inference is an induction along the path that can be modelled as: F3 Manifestation Product Type R7i has example F5 Item P39i was measured by E16 Measurement P40 observed dimension E54 Dimension.
It can happen that a given exemplar, or subset of exemplars, originally produced, or intended to be produced, with that characteristic, accidentally lacks it. This fact should be recorded as a property of F5 Item, and not of F3 Manifestation Product Type.
"""@en .

<http://iflastandards.info/ns/fr/frbr/frbroo/CLP43i_should_be_dimension_of> rdfs:label "should be dimension of"@en ;
    rdfs:comment """
"""@en .

<http://iflastandards.info/ns/fr/frbr/frbroo/CLP45_should_consist_of> rdfs:label "should consist of"@en ;
    rdfs:comment """This property associates a publication, i.e. an instance of F3 Manifestation Product Type, with an instance of E57 Material, which all exemplars of that publication should consist of, as long as they are recognised as exemplars of that publication. Typically, this property is observed on one exemplar of a publication, and extrapolated to all other exemplars of the same publication. This logical inference is an induction along the path that can be modelled as: F3 Manifestation Product Type R7i has example F5 Item P41i was classified by E17 Type Assignment P42 assigned E57 Material.
It can happen that a given exemplar, or subset of exemplars, originally produced, or intended to be produced, with that characteristic, accidentally lacks it. This fact should be recorded as a property of F5 Item, and not of F3 Manifestation Product Type.
"""@en .

<http://iflastandards.info/ns/fr/frbr/frbroo/CLP45i_should_be_incorporated_in> rdfs:label "should be incorporated in"@en ;
    rdfs:comment """
"""@en .

<http://iflastandards.info/ns/fr/frbr/frbroo/CLP46_should_be_composed_of> rdfs:label "should be composed of"@en ;
    rdfs:comment """This property associates an instance of F3 Manifestation Product Type which prescribes that all its Items will contain as parts an Item of another instance of F3 Manifestation Product Type with that instance of F3 Manifestation Product Type.
"""@en .

<http://iflastandards.info/ns/fr/frbr/frbroo/CLP46i_may_form_part_of> rdfs:label "may form part of"@en ;
    rdfs:comment """
"""@en .

<http://iflastandards.info/ns/fr/frbr/frbroo/CLR6_should_carry> rdfs:label "should carry"@en ;
    rdfs:comment """This property associates a publication, i.e. an instance of F3 Manifestation Product Type, with an instance of F24 Publication Expression, which all exemplars of that publication should carry, as long as they are recognised as complete exemplars of that publication. Typically, this property is observed on one exemplar of a publication, and extrapolated to all other exemplars of the same publication. This logical inference is an induction along the path that can be modelled as: F3 Manifestation Product Type R7i has example F5 Item R6 carries F24 Publication Expression.
It can happen that a given exemplar, or a subset of exemplars, originally produced, or intended to be produced with that characteristic, accidentally lacks part of the publication expression. This fact should be recorded as a property of F5 Item, and not of F3 Manifestation Product Type.
"""@en .

<http://iflastandards.info/ns/fr/frbr/frbroo/CLR6i_should_be_carried_by> rdfs:label "should be carried by"@en ;
    rdfs:comment """
"""@en .

<http://iflastandards.info/ns/fr/frbr/frbroo/R10_has_member> rdfs:label "has member"@en ;
    rdfs:comment """This property associates an instance of F15 Complex Work with an instance of F1 Work that forms part of it. 
"""@en .

<http://iflastandards.info/ns/fr/frbr/frbroo/R10i_is_member_of> rdfs:label "is member of"@en ;
    rdfs:comment """
"""@en .

<http://iflastandards.info/ns/fr/frbr/frbroo/R11_has_issuing_rule> rdfs:label "has issuing rule"@en ;
    rdfs:comment """This property associates an instance of F18 Serial Work with the instance of E29 Design or Procedure that specifies the issuing policy planned by this Work, such as sequencing pattern, expected frequency and expected regularity.
This property is a shortcut of the full path: F18 Serial Work R23i was realised through F30 Publication Event P16 used specific object E29 Design or Procedure.
"""@en .

<http://iflastandards.info/ns/fr/frbr/frbroo/R11i_is_issuing_rule_of> rdfs:label "is issuing rule of"@en ;
    rdfs:comment """
"""@en .

<http://iflastandards.info/ns/fr/frbr/frbroo/R12_is_realised_in> rdfs:label "is realised in"@en ;
    rdfs:comment """This property associates an instance of F20 Performance Work with an instance of F25 Performance Plan that consists of signs (words, figures, etc.) which express the directions the instance of F20 Performance Work consists of.
"""@en .

<http://iflastandards.info/ns/fr/frbr/frbroo/R12i_realises> rdfs:label "realises"@en ;
    rdfs:comment """
"""@en .

<http://iflastandards.info/ns/fr/frbr/frbroo/R13_is_realised_in> rdfs:label "is realised in"@en ;
    rdfs:comment """This property associates an instance of F21 Recording Work with an instance of F26 Recording realising the instance of F21 Recording Work.
This is a shortcut of the more elaborated path through R22 was realised through, F29 Recording Event and R21 created, which should be used when information about the recording event is available.
"""@en .

<http://iflastandards.info/ns/fr/frbr/frbroo/R13i_realises> rdfs:label "realises"@en ;
    rdfs:comment """
"""@en .

<http://iflastandards.info/ns/fr/frbr/frbroo/R15_has_fragment> rdfs:label "has fragment"@en ;
    rdfs:comment """This property associates the fragment of an expression and the expression of which it is a fragment.
"""@en .

<http://iflastandards.info/ns/fr/frbr/frbroo/R15i_is_fragment_of> rdfs:label "is fragment of"@en ;
    rdfs:comment """
"""@en .

<http://iflastandards.info/ns/fr/frbr/frbroo/R16_initiated> rdfs:label "initiated"@en ;
    rdfs:comment """This property associates the first conception of a work and the work itself that ensued from a given initial idea.
It marks the origin of the causality chain that results in a work’s coming into existence.
"""@en .

<http://iflastandards.info/ns/fr/frbr/frbroo/R16i_was_initiated_by> rdfs:label "was initiated by"@en ;
    rdfs:comment """
"""@en .

<http://iflastandards.info/ns/fr/frbr/frbroo/R17_created> rdfs:label "created"@en ;
    rdfs:comment """This property associates the expression that was first externalised during a particular creation event with that particular creation event.
"""@en .

<http://iflastandards.info/ns/fr/frbr/frbroo/R17i_was_created_by> rdfs:label "was created by"@en ;
    rdfs:comment """
"""@en .

<http://iflastandards.info/ns/fr/frbr/frbroo/R18_created> rdfs:label "created"@en ;
    rdfs:comment """This property associates an instance of F28 Expression Creation with the first physical objects in which the resulting instance of F2 Expression was embodied.
"""@en .

<http://iflastandards.info/ns/fr/frbr/frbroo/R18i_was_created_by> rdfs:label "was created by"@en ;
    rdfs:comment """
"""@en .

<http://iflastandards.info/ns/fr/frbr/frbroo/R19_created_a_realization_of> rdfs:label "created a realization of"@en ;
    rdfs:comment """This property associates an instance of F28 Expression Creation with the corresponding instance of F14 Individual Work or an instance of F15 Complex Work of which the corresponding instance of F14 Individual Work is a member.
"""@en .

<http://iflastandards.info/ns/fr/frbr/frbroo/R19i_was_realised_through> rdfs:label "was realised through"@en ;
    rdfs:comment """
"""@en .

<http://iflastandards.info/ns/fr/frbr/frbroo/R1_is_logical_successor_of> rdfs:label "is logical successor of"@en ;
    rdfs:comment """This property associates an instance of F1 Work which logically continues the content of another instance of F1 Work with the latter.
"""@en .

<http://iflastandards.info/ns/fr/frbr/frbroo/R1i_has_successor> rdfs:label "has successor"@en ;
    rdfs:comment """
"""@en .

<http://iflastandards.info/ns/fr/frbr/frbroo/R20_recorded> rdfs:label "recorded"@en ;
    rdfs:comment """This property associates an instance of F29 Recording Event with the instance of E2 Temporal Entity which was captured.
"""@en .

<http://iflastandards.info/ns/fr/frbr/frbroo/R20i_was_recorded_through> rdfs:label "was recorded through"@en ;
    rdfs:comment """
"""@en .

<http://iflastandards.info/ns/fr/frbr/frbroo/R21_created> rdfs:label "created"@en ;
    rdfs:comment """This property associates an instance of F29 Recording Event with the instance of F26 Recording that was created.
"""@en .

<http://iflastandards.info/ns/fr/frbr/frbroo/R21i_was_created_through> rdfs:label "was created through"@en ;
    rdfs:comment """
"""@en .

<http://iflastandards.info/ns/fr/frbr/frbroo/R22_created_a_realization_of> rdfs:label "created a realization of"@en ;
    rdfs:comment """This property associates an instance of F29 Recording Event with the instance of F21 Recording Work it realised.
"""@en .

<http://iflastandards.info/ns/fr/frbr/frbroo/R22i_was_realised_through> rdfs:label "was realised through"@en ;
    rdfs:comment """
"""@en .

<http://iflastandards.info/ns/fr/frbr/frbroo/R23_created_a_realization_of> rdfs:label "created a realization of"@en ;
    rdfs:comment """This property associates an instance of F30 Publication Event with the instance of F19 Publication Work it realised.
"""@en .

<http://iflastandards.info/ns/fr/frbr/frbroo/R23i_was_realised_through> rdfs:label "was realised through"@en ;
    rdfs:comment """
"""@en .

<http://iflastandards.info/ns/fr/frbr/frbroo/R24_created> rdfs:label "created"@en ;
    rdfs:comment """This property associates the instance of F24 Publication Expression that was created during a particular F30 Publication Event with that F30 Publication Event.
"""@en .

<http://iflastandards.info/ns/fr/frbr/frbroo/R24i_was_created_through> rdfs:label "was created through"@en ;
    rdfs:comment """
"""@en .

<http://iflastandards.info/ns/fr/frbr/frbroo/R25_performed> rdfs:label "performed"@en ;
    rdfs:comment """This property associates an instance of F31 Performance with the instance of F25 Performance Plan to which all those participating in the performance were supposed to conform.
"""@en .

<http://iflastandards.info/ns/fr/frbr/frbroo/R25i_was_performed_in> rdfs:label "was performed in"@en ;
    rdfs:comment """
"""@en .

<http://iflastandards.info/ns/fr/frbr/frbroo/R26_produced_things_of_type> rdfs:label "produced things of type"@en ;
    rdfs:comment """This property associates an instance of F32 Carrier Production Event with the instance of F3 Manifestation Product Type it produced items of.
"""@en .

<http://iflastandards.info/ns/fr/frbr/frbroo/R26i_was_produced_by> rdfs:label "was produced by"@en ;
    rdfs:comment """
"""@en .

<http://iflastandards.info/ns/fr/frbr/frbroo/R27_used_as_source_material> rdfs:label "used as source material"@en ;
    rdfs:comment """This property associates an instance of F32 Carrier Production Event with the set of signs provided by the publisher to be carried by all of the produced items.
"""@en .

<http://iflastandards.info/ns/fr/frbr/frbroo/R27i_was_used_by> rdfs:label "was used by"@en ;
    rdfs:comment """
"""@en .

<http://iflastandards.info/ns/fr/frbr/frbroo/R28_produced> rdfs:label "produced"@en ;
    rdfs:comment """This property associates an instance of F32 Carrier Production Event with any one of the produced items (i.e., the instances of F5 Item or F53 Material Copy).
"""@en .

<http://iflastandards.info/ns/fr/frbr/frbroo/R28i_was_produced_by> rdfs:label "was produced by"@en ;
    rdfs:comment """
"""@en .

<http://iflastandards.info/ns/fr/frbr/frbroo/R29_reproduced> rdfs:label "reproduced"@en ;
    rdfs:comment """This property associates an instance of F33 Reproduction Event with an instance of E84 Information Carrier it reproduces.
"""@en .

<http://iflastandards.info/ns/fr/frbr/frbroo/R29i_was_reproduced_by> rdfs:label "was reproduced by"@en ;
    rdfs:comment """
"""@en .

<http://iflastandards.info/ns/fr/frbr/frbroo/R2_is_derivative_of> rdfs:label "is derivative of"@en ;
    rdfs:comment """This property associates an instance of F1 Work which modifies the content of another instance of F1 Work with the latter. The property R2.1 has type of this property allows for specifying the kind of derivation, such as adaptation, summarisation etc.
"""@en .

<http://iflastandards.info/ns/fr/frbr/frbroo/R2i_has_derivative> rdfs:label "has derivative"@en ;
    rdfs:comment """
"""@en .

<http://iflastandards.info/ns/fr/frbr/frbroo/R30_produced> rdfs:label "produced"@en ;
    rdfs:comment """This property associates an instance of F33 Reproduction Event with an instance of E84 Information Carrier it produces.
"""@en .

<http://iflastandards.info/ns/fr/frbr/frbroo/R30i_was_produced_by> rdfs:label "was produced by"@en ;
    rdfs:comment """
"""@en .

<http://iflastandards.info/ns/fr/frbr/frbroo/R31_is_reproduction_of> rdfs:label "is reproduction of"@en ;
    rdfs:comment """This property associates an instance of E84 Information Carrier which is a reproduction of another instance of E84 Information Carrier with the latter. It is considered that a reproduction of multiple originals resulting in a single product requires a merging of those objects prior to the reproduction. Therefore an Information Carrier is regarded to be a reproduction of one and only one original. This property is a shortcut of the more fully developed path from E84 Information Carrier through R30 produced (was produced by), F33 Reproduction Event R29 reproduced (was reproduced by) to E84 Information Carrier.
"""@en .

<http://iflastandards.info/ns/fr/frbr/frbroo/R31i_has_reproduction> rdfs:label "has reproduction"@en ;
    rdfs:comment """
"""@en .

<http://iflastandards.info/ns/fr/frbr/frbroo/R32_is_warranted_by> rdfs:label "is warranted by"@en ;
    rdfs:comment """This property associates an instance of F35 Nomen Use Statement with an instance of F52 Name Use Activity which provides evidence for the use of the particular nomen in the stated sense. The association between this name use activity and a source for it may be described by the property P70 documents (is documented in).
"""@en .

<http://iflastandards.info/ns/fr/frbr/frbroo/R32i_warrants> rdfs:label "warrants"@en ;
    rdfs:comment """
"""@en .

<http://iflastandards.info/ns/fr/frbr/frbroo/R34_has_validity_period> rdfs:label "has validity period"@en ;
    rdfs:comment """This property associates an instance of F34 KOS with the instance of E52 Time-Span describing the period for which the particular KOS Expression was regarded as valid by its maintainers. Each change of validity status of a nomen use statement within a KOS should be associated with a release change of the KOS. The individual time-span of a validity state of a nomen would be the union of the time-spans of the KOS in which the Nomen was declared to have the particular validity status (provisional, accepted, obsolete etc...).
"""@en .

<http://iflastandards.info/ns/fr/frbr/frbroo/R34i_is_validity_period_of> rdfs:label "is validity period of"@en ;
    rdfs:comment """
"""@en .

<http://iflastandards.info/ns/fr/frbr/frbroo/R35_specified_by> rdfs:label "specified by"@en ;
    rdfs:comment """This property associates an instance of F35 Nomen Use Statement with an instance of F34 KOS in which the Nomen Use Statement has a given status. The property R35.1 allows for specifying the particular status of the nomen use statement within the KOS. An instance of R35 is specified by should have only one status.
"""@en .

<http://iflastandards.info/ns/fr/frbr/frbroo/R35i_specifies> rdfs:label "specifies"@en ;
    rdfs:comment """
"""@en .

<http://iflastandards.info/ns/fr/frbr/frbroo/R36_uses_script_conversion> rdfs:label "uses script conversion"@en ;
    rdfs:comment """This property associates an instance of F35 Nomen Use Statement with the instance of F36 Script Conversion that was used to create the Nomen referred to in the Nomen Use Statement. The source of this conversion may or may not be explicitly mentioned. Is shortcut of: F35 Nomen Use Statement R17 was created by (created) F28 Expression Creation P33 used specific technique (was used by) E29 Design or Procedure.
"""@en .

<http://iflastandards.info/ns/fr/frbr/frbroo/R36i_is_script_conversion_used_in> rdfs:label "is script conversion used in"@en ;
    rdfs:comment """This property associates an instance of F35 Nomen Use Statement with the instance of F12 Nomen for which it declares usage.
"""@en .

<http://iflastandards.info/ns/fr/frbr/frbroo/R37_states_as_nomen> rdfs:label "states as nomen"@en ;
    rdfs:comment """
"""@en .

<http://iflastandards.info/ns/fr/frbr/frbroo/R37i_is_stated_as_nomen_in> rdfs:label "is stated as nomen in"@en ;
    rdfs:comment """
"""@en .

<http://iflastandards.info/ns/fr/frbr/frbroo/R38_refers_to_thema> rdfs:label "refers to thema"@en ;
    rdfs:comment """This property associates an instance of F35 Nomen Use Statement with the instance of E1 CRM Entity for which it declares the usage of a nomen.
"""@en .

<http://iflastandards.info/ns/fr/frbr/frbroo/R38i_is_thema_of> rdfs:label "is thema of"@en ;
    rdfs:comment """
"""@en .

<http://iflastandards.info/ns/fr/frbr/frbroo/R39_is_intended_for> rdfs:label "is intended for"@en ;
    rdfs:comment """This property associates an instance of F35 Nomen Use Statement with an instance of E74 Group which is the target audience for which the associated nomen use is intended. To indicate that the associated nomen is declared as preferred in all contexts, the instance of E74 Group is ‘mankind’.
"""@en .

<http://iflastandards.info/ns/fr/frbr/frbroo/R39i_is_target_audience_in> rdfs:label "is target audience in"@en ;
    rdfs:comment """
"""@en .

<http://iflastandards.info/ns/fr/frbr/frbroo/R3_is_realised_in> rdfs:label "is realised in"@en ;
    rdfs:comment """This property associates an instance of F22 Self-Contained Expression with an instance of F1 Work.
This property expresses the association that exists between an expression (F22) and the work that this expression conveys. The semantics of the association will be different depending on what specific subtype of F1 Work the work is an instance of. If the work is an instance of F14 Individual Work, the F22 Self-Contained Expression completely conveys the individual work. If the work is an instance of F15 Complex Work, the F22 Self-Contained Expression conveys an alternative member of the complex work.
Our factual knowledge of how a given work is realised into an expression is often limited and this property makes it possible to express the association between instances of F22 Self-Contained Expression and the work it conveys without using the more developed paths.
The property R3.1 has type: E55 Type allows for specifying the role played by the referred to expression in the overall bibliographic history of the work (e.g., ‘progenitor expression’, on which all other expressions of the same work are based; ‘reference for canonical citations’, in the sense of the HuCit ontology developed by Matteo Romanello and Michele Pasin; ‘earliest draft’, ‘intermediate draft’, ‘final clean draft’, ‘princeps edition’, etc.).
"""@en .

<http://iflastandards.info/ns/fr/frbr/frbroo/R3i_realises> rdfs:label "realises"@en ;
    rdfs:comment """
"""@en .

<http://iflastandards.info/ns/fr/frbr/frbroo/R40_has_representative_expression> rdfs:label "has representative expression"@en ;
    rdfs:comment """This property identifies an instance of F22 Self-Contained Expression that has been chosen as the most characteristic expression of the instance of F1 Work of which it is an expression. There is no other semantic implication to this notion of being characteristic than to be an adequate candidate to uniquely identify the Work realized by it. Prototypically, this is the instance of F22 Self-Contained Expression that is deemed characteristic of an instance of F15 Complex Work.
Typically, any expression that is not regarded as “representative” for the work it expresses, would require a controlled access point, with qualifiers specifying the differences between that expression and a representative expression, although this may not always be done in practice. The title of a Work may not be one taken from a representative expression.
A given work can have more than one representative expression, provided the differences between these expressions are not deemed “substantial.” If the anticipated needs of users are not considered to call for bibliographic distinctions between variant expressions of a work, then even expressions that differ significantly from each other can be regarded as equally representative for the work. (See FRBR: Final Report, p. 19-20).
A given expression can be deemed representative for a work with regard to some of its aspects (e.g., the text contained in an edition the title proper of which reads ‘The tragicall historie of HAMLET Prince of Denmarke’, and the language of that text), and not representative for it with regard to some other aspects (e.g., the title proper ‘The tragicall historie of HAMLET Prince of Denmarke’ itself, which, being different from the title that is regarded as “representative” for Shakespeare’s work, will require the use of a controlled access point).
R40 has representative expression is a shortcut of the more developed path F1 Work R50i was assigned by F42 Representative Expression Assignment R51 assigned F2 Expression.

"""@en .

<http://iflastandards.info/ns/fr/frbr/frbroo/R40i_is_representative_expression_for> rdfs:label "is representative expression for"@en ;
    rdfs:comment """
"""@en .

<http://iflastandards.info/ns/fr/frbr/frbroo/R41_has_rep_manifestation_product_type> rdfs:label "has rep manifestation product type"@en ;
    rdfs:comment """This property identifies an instance of F3 Manifestation Product Type that has been chosen as the most characteristic Manifestation Product Type of the instance of F2 Expression of which it is a manifestation.
Identifying an instance of F3 Manifestation Product Type that is representative for an instance of F2 Expression makes it possible in turn to identify an instance of F2 Expression that is representative for an instance of F1 Work, and to decide what should be regarded as the title of the work.
The title of an Expression may not be one taken from a representative Manifestation Product Type or Manifestation Singleton.
A given expression can have more than one Representative Manifestation Product Type.
R41 has representative manifestation product type is a shortcut of the more developed path F2 Expression R48i was assigned by F41 Representative Manifestation Assignment R49 assigned F3 Manifestation Product Type.

"""@en .

<http://iflastandards.info/ns/fr/frbr/frbroo/R41i_is_rep_manifestation_product_type_for> rdfs:label "is rep manifestation product type for"@en ;
    rdfs:comment """
"""@en .

<http://iflastandards.info/ns/fr/frbr/frbroo/R42_is_representative_manifestation_singleton_for> rdfs:label "is representative manifestation singleton for"@en ;
    rdfs:comment """This property identifies an instance of Manifestation Singleton that has been declared as the unique representative for an instance of F2 Expression by some bibliographic agency.
This property identifies an instance of F4 Manifestation Singleton that has been chosen as the most characteristic Manifestation Singleton of the instance of F2 Expression of which it is a manifestation.
Identifying an instance of F4 Manifestation Singleton that is representative for an instance of F2 Expression makes it possible in turn to identify an instance of F2 Expression that is representative for an instance of F1 Work, and to decide what should be regarded as the title of the work.
The title of an Expression may not be one taken from a representative Manifestation Product Type or Manifestation Singleton.
A given expression can have more than one representative Manifestation Singleton.
It is a shortcut for the more developed path: F2 Expression R48i was assigned by F41 Representative Manifestation Assignment R53 assigned F4 Manifestation Singleton.

"""@en .

<http://iflastandards.info/ns/fr/frbr/frbroo/R42i_has_representative_manifestation_singleton> rdfs:label "has representative manifestation singleton"@en ;
    rdfs:comment """
"""@en .

<http://iflastandards.info/ns/fr/frbr/frbroo/R43_carried_out_by> rdfs:label "carried out by"@en ;
    rdfs:comment """This property associates a bibliographic agency (represented by one or more of its cataloguers) and the assigning of which Manifestation (i.e., which instance of F3 Manifestation Product Type or F4 Manifestation Singleton) is representative for a given expression.
In cataloguing practice, such a relationship is usually just implicit. However, it can become explicit, for example when a bibliographic agency creates an authority record for a given work and fills the “Source” field with information about the publication that contains the expression that was used by the bibliographic agency to establish the controlled access point for the work realised in that expression.
"""@en .

<http://iflastandards.info/ns/fr/frbr/frbroo/R43i_performed> rdfs:label "performed"@en ;
    rdfs:comment """
"""@en .

<http://iflastandards.info/ns/fr/frbr/frbroo/R44_carried_out_by> rdfs:label "carried out by"@en ;
    rdfs:comment """This property associates a bibliographic agency (represented by one or more of its cataloguers) and the assigning of which expression is representative for a given Work.
In cataloguing practice, such a relationship is usually just implicit. However, it can become explicit, for example when a bibliographic agency creates an authority record for a given work and fills the “Source” field with information about the publication that contains the expression that was used by the bibliographic agency to establish the controlled access point for the work realised in that expression.

"""@en .

<http://iflastandards.info/ns/fr/frbr/frbroo/R44i_performed> rdfs:label "performed"@en ;
    rdfs:comment """
"""@en .

<http://iflastandards.info/ns/fr/frbr/frbroo/R45_assigned_to> rdfs:label "assigned to"@en ;
    rdfs:comment """This property identifies the entity to which an actor, such as a bibliographic agency, assigned an instance of F13 Identifier.
"""@en .

<http://iflastandards.info/ns/fr/frbr/frbroo/R45i_was_assigned_by> rdfs:label "was assigned by"@en ;
    rdfs:comment """
"""@en .

<http://iflastandards.info/ns/fr/frbr/frbroo/R46_assigned_to> rdfs:label "assigned to"@en ;
    rdfs:comment """This property associates the instance of F13 Identifier assigned to an instance of E1 CRM Entity and the event of assigning it.
"""@en .

<http://iflastandards.info/ns/fr/frbr/frbroo/R46i_was_assigned_by> rdfs:label "was assigned by"@en ;
    rdfs:comment """
"""@en .

<http://iflastandards.info/ns/fr/frbr/frbroo/R48_assigned_to> rdfs:label "assigned to"@en ;
    rdfs:comment """This property associates the event of assigning a representative instance of F3 Manifestation Product Type or F4 Manifestation Singleton with the expression to which it was assigned.
"""@en .

<http://iflastandards.info/ns/fr/frbr/frbroo/R48i_was_assigned_by> rdfs:label "was assigned by"@en ;
    rdfs:comment """
"""@en .

<http://iflastandards.info/ns/fr/frbr/frbroo/R49_assigned> rdfs:label "assigned"@en ;
    rdfs:comment """This property associates the event of assigning a representative instance of F3 Manifestation Product Type with the F3 Manifestation Product Type which has been assigned.
"""@en .

<http://iflastandards.info/ns/fr/frbr/frbroo/R49i_was_assigned_by> rdfs:label "was assigned by"@en ;
    rdfs:comment """
"""@en .

<http://iflastandards.info/ns/fr/frbr/frbroo/R4_carriers_provided_by> rdfs:label "carriers provided by"@en ;
    rdfs:comment """This property associates a publication, i.e. an instance of F3 Manifestation Product Type, with an instance of F2 Expression, which all exemplars of that publication should carry, as long as they are recognised as complete exemplars of that publication. Typically, this property is observed on one exemplar of a publication, and extrapolated to all other exemplars of the same publication.
This property is a shortcut of: F2 Expression P165i is incorporated in F24 Publication Expression CLR6i should be carried by F3 Manifestation Product Type.
"""@en .

<http://iflastandards.info/ns/fr/frbr/frbroo/R4i_comprises_carriers_of> rdfs:label "comprises carriers of"@en ;
    rdfs:comment """
"""@en .

<http://iflastandards.info/ns/fr/frbr/frbroo/R50_assigned_to> rdfs:label "assigned to"@en ;
    rdfs:comment """This property associates the event of assigning a representative instance of F2 Expression with the instance of F15 Complex Work to which it was assigned.
"""@en .

<http://iflastandards.info/ns/fr/frbr/frbroo/R50i_was_assigned_by> rdfs:label "was assigned by"@en ;
    rdfs:comment """
"""@en .

<http://iflastandards.info/ns/fr/frbr/frbroo/R51_assigned> rdfs:label "assigned"@en ;
    rdfs:comment """This property associates the event of assigning a representative instance of F2 Expression with the F2 Expression which has been assigned.
"""@en .

<http://iflastandards.info/ns/fr/frbr/frbroo/R51i_was_assigned_by> rdfs:label "was assigned by"@en ;
    rdfs:comment """
"""@en .

<http://iflastandards.info/ns/fr/frbr/frbroo/R52_used_rule> rdfs:label "used rule"@en ;
    rdfs:comment """This property associates the event of assigning an instance of F13 Identifier with the instructions followed by an actor, such as a Bibliographic Agency, in creating that identifier.
"""@en .

<http://iflastandards.info/ns/fr/frbr/frbroo/R52i_was_the_rule_used_in> rdfs:label "was the rule used in"@en ;
    rdfs:comment """
"""@en .

<http://iflastandards.info/ns/fr/frbr/frbroo/R53_assigned> rdfs:label "assigned"@en ;
    rdfs:comment """This property associates the event of assigning a representative instance of F4 Manifestation Singleton with the F4 Manifestation Singleton which has been assigned.
"""@en .

<http://iflastandards.info/ns/fr/frbr/frbroo/R53i_was_assigned_by> rdfs:label "was assigned by"@en ;
    rdfs:comment """
"""@en .

<http://iflastandards.info/ns/fr/frbr/frbroo/R54_has_nomen_language> rdfs:label "has nomen language"@en ;
    rdfs:comment """This property associates an instance of F35 Nomen Use Statement with an instance of E56 Language which is a target language for the associated nomen use.
"""@en .

<http://iflastandards.info/ns/fr/frbr/frbroo/R54i_is_language_of_nomen_in> rdfs:label "is language of nomen in"@en ;
    rdfs:comment """
"""@en .

<http://iflastandards.info/ns/fr/frbr/frbroo/R55_has_nomen_form> rdfs:label "has nomen form"@en ;
    rdfs:comment """This property associates an instance of F35 Nomen Use Statement with the instance of E55 Type that characterizes the Nomen referred to in the Nomen Use Statement, such as abbreviation, full name etc. In the case of abbreviations, the source of this form may or may not be explicitly mentioned.
"""@en .

<http://iflastandards.info/ns/fr/frbr/frbroo/R55i_is_nomen_form_in> rdfs:label "is nomen form in"@en ;
    rdfs:comment """
"""@en .

<http://iflastandards.info/ns/fr/frbr/frbroo/R56_has_related_use> rdfs:label "has related use"@en ;
    rdfs:comment """This property associates an instance of F35 Nomen Use Statement with another instance of F35 Nomen Use Statement which has a related use in some context, such as alternative, lexical variant, replacing former use etc. The property R56.1 allows for specifying the particular kind of the nomen use statement relationship.
"""@en .

<http://iflastandards.info/ns/fr/frbr/frbroo/R56i_is_related_use_for> rdfs:label "is related use for"@en ;
    rdfs:comment """
"""@en .

<http://iflastandards.info/ns/fr/frbr/frbroo/R57_is_based_on> rdfs:label "is based on"@en ;
    rdfs:comment """This property associates an instance of F38 Character with an instance of E39 Actor that the character is motivated by or is intended to represent. An instance of F38 Character may be based on a combination of features taken from several actors. This property is a shortcut of the more fully developed path from E28 Conceptual Object, restricted to F38 Character, through the inverse of P94 has created (was created by), E65 Creation P17 was motivated by (motivated) to E1 CRM Entity restricted to E39 Actor.
"""@en .

<http://iflastandards.info/ns/fr/frbr/frbroo/R57i_is_basis_for> rdfs:label "is basis for"@en ;
    rdfs:comment """
"""@en .

<http://iflastandards.info/ns/fr/frbr/frbroo/R58_has_fictional_member> rdfs:label "has fictional member"@en ;
    rdfs:comment """This property associates an instance of F38 Character representing a group with another instance of F38 Character that is presented in relevant fiction as a member of the fictional group.
"""@en .

<http://iflastandards.info/ns/fr/frbr/frbroo/R58i_is_fictional_member_of> rdfs:label "is fictional member of"@en ;
    rdfs:comment """
"""@en .

<http://iflastandards.info/ns/fr/frbr/frbroo/R59_had_typical_subject> rdfs:label "had typical subject"@en ;
    rdfs:comment """This property associates an instance of F51 Pursuit with the instance of E1 CRM Entity that is the typical subject of the associated activity, such as an area of expertise in which the actor is engaged or was engaged.
"""@en .

<http://iflastandards.info/ns/fr/frbr/frbroo/R59i_was_typical_subject_of> rdfs:label "was typical subject of"@en ;
    rdfs:comment """
"""@en .

<http://iflastandards.info/ns/fr/frbr/frbroo/R5_has_component> rdfs:label "has component"@en ;
    rdfs:comment """This property associates an F2 Expression X with a structural component Y that conveys in itself the complete concept of a work that is member of (R10) the overall work realized by X.
It does not cover the relationship that exists between pre-existing expressions that are re-used in a new, larger expression and that new, larger expression. Such a relationship is modelled by P165 incorporates.
"""@en .

<http://iflastandards.info/ns/fr/frbr/frbroo/R5i_is_component_of> rdfs:label "is component of"@en ;
    rdfs:comment """
"""@en .

<http://iflastandards.info/ns/fr/frbr/frbroo/R60_used_to_use_language> rdfs:label "used to use language"@en ;
    rdfs:comment """This property associates an instance of F51 Pursuit with the instance of E56 Language that was characteristically used for the products of the associated activity.
The property R60.1 has type of use allows for specifying a particular form of use.
"""@en .

<http://iflastandards.info/ns/fr/frbr/frbroo/R60i_was_language_used_by> rdfs:label "was language used by"@en ;
    rdfs:comment """
"""@en .

<http://iflastandards.info/ns/fr/frbr/frbroo/R61_occured_in_kind_of_context> rdfs:label "occured in kind of context"@en ;
    rdfs:comment """This property associates an instance of F52 Name Use Activity with the instance of E55 Type that characterises the kind of role or context within which the associated name was used.
"""@en .

<http://iflastandards.info/ns/fr/frbr/frbroo/R61i_was_kind_of_context_for> rdfs:label "was kind of context for"@en ;
    rdfs:comment """
"""@en .

<http://iflastandards.info/ns/fr/frbr/frbroo/R62_was_used_for_membership_in> rdfs:label "was used for membership in"@en ;
    rdfs:comment """This property associates an instance of F52 Name Use Activity with the instance of E74 Group that characterises the context within which the associated name was used for membership in that group.
"""@en .

<http://iflastandards.info/ns/fr/frbr/frbroo/R62i_was_context_for> rdfs:label "was context for"@en ;
    rdfs:comment """
"""@en .

<http://iflastandards.info/ns/fr/frbr/frbroo/R63_named> rdfs:label "named"@en ;
    rdfs:comment """This property associates an instance of F52 Name Use Activity with the instance of E1 CRM Entity that the associated name was used for.
"""@en .

<http://iflastandards.info/ns/fr/frbr/frbroo/R63i_was_named_by> rdfs:label "was named by"@en ;
    rdfs:comment """
"""@en .

<http://iflastandards.info/ns/fr/frbr/frbroo/R64_used_name> rdfs:label "used name"@en ;
    rdfs:comment """This property associates an instance of F52 Name Use Activity with the instance of E41 Appellation that was used for the associated entity.
"""@en .

<http://iflastandards.info/ns/fr/frbr/frbroo/R64i_was_name_used_by> rdfs:label "was name used by"@en ;
    rdfs:comment """
"""@en .

<http://iflastandards.info/ns/fr/frbr/frbroo/R65_recorded_aspects_of> rdfs:label "recorded aspects of"@en ;
    rdfs:comment """This property associates an instance of F29 Recording Event with an instance of E18 Physical Thing some of whose features, at the time of recording, were recorded in that process.
"""@en .

<http://iflastandards.info/ns/fr/frbr/frbroo/R65i_had_aspects_recorded_through> rdfs:label "had aspects recorded through"@en ;
    rdfs:comment """
"""@en .

<http://iflastandards.info/ns/fr/frbr/frbroo/R66_included_performed_version_of> rdfs:label "included performed version of"@en ;
    rdfs:comment """This property associates an instance of F31 Performance with a product of the mind that was performed in the course of that instance of F31 Performance.
According to the level of knowledge available about the performance, the range of this property can actually be specialised as either an instance of F1 Work (if nothing is known as to which specific expression of the work was performed), or of F2 Expression (if there is a reasonable amount of certainty as to which specific expression—e.g., a well identified translation of a play—of the work was performed).
In addition to being a subproperty of P16 used specific object (was used for), this property also is a shortcut of the fully developed path that goes from F31 Performance to F1 Work through: R25 performed F25 Performance Plan P165 incorporates F22 Self-Contained Expression R3i realises. In this fully developed path, the specific instance of F22 Self-Contained Expression can be precisely identified and described for its own sake, or it can just be known to have necessarily existed.

"""@en .

<http://iflastandards.info/ns/fr/frbr/frbroo/R66i_had_a_performed_version_through> rdfs:label "had a performed version through"@en ;
    rdfs:comment """
"""@en .

<http://iflastandards.info/ns/fr/frbr/frbroo/R6_carries> rdfs:label "carries"@en ;
    rdfs:comment """This property associates an instance of F54 Utilised Information Carrier with the unique instance of F24 Publication Expression it carries.
"""@en .

<http://iflastandards.info/ns/fr/frbr/frbroo/R6i_is_carried_by> rdfs:label "is carried by"@en ;
    rdfs:comment """
"""@en .

<http://iflastandards.info/ns/fr/frbr/frbroo/R7_is_example_of> rdfs:label "is example of"@en ;
    rdfs:comment """This property associates a publication with one of its exemplars.
It is a shortcut of the more developed path: F5 Item R28i was produced by F32 Carrier Production R26 produced things of type (was produced by): F3 Manifestation Product Type.
"""@en .

<http://iflastandards.info/ns/fr/frbr/frbroo/R7i_has_example> rdfs:label "has example"@en ;
    rdfs:comment """
"""@en .

<http://iflastandards.info/ns/fr/frbr/frbroo/R8_consists_of> rdfs:label "consists of"@en ;
    rdfs:comment """This property associates an instance of F13 Identifier with one of the non-syntactic instances of E90 Symbolic Object which form part of it.
"""@en .

<http://iflastandards.info/ns/fr/frbr/frbroo/R8i_forms_part_of> rdfs:label "forms part of"@en ;
    rdfs:comment """
"""@en .

<http://iflastandards.info/ns/fr/frbr/frbroo/R9_is_realised_in> rdfs:label "is realised in"@en ;
    rdfs:comment """This property associates an F14 Individual Work with the unique F22 Self-Contained Expression that completely conveys it.
It is a shortcut for the more developed path: F14 Individual Work R19i was realised through F28 Expression Creation R17 created F22 Self-Contained Expression.
"""@en .

<http://iflastandards.info/ns/fr/frbr/frbroo/R9i_realises> rdfs:label "realises"@en ;
    rdfs:comment """
"""@en .

<http://postdata.linhd.uned.es/kos/scheme-category> a owl:NamedIndividual .

<http://postdata.linhd.uned.es/ontology/POSTDATA-literaryAnalysis.owl/dataType#vc-typeOfIntertextuality> a rdfs:Datatype .

<http://postdata.linhd.uned.es/ontology/POSTDATA-literaryAnalysis.owl/vc-figureCategory> a rdfs:Datatype .

<http://postdata.linhd.uned.es/ontology/postdata-core#additionalFile> a owl:DatatypeProperty ;
    rdfs:label "additional File"@en ;
    rdfs:comment """A file (XML, PFD, plain text) which contains the Redaction and, likely, other type of analytical information.

Taking as example the poem "Amadís de Gaula a Don Quijote de la Mancha": Redaction could be an XML-TEI file (for example, the TEI annotated text of ADSO corpus (https://github.com/bncolorado/CorpusSonetosSigloDeOro/blob/master/Cervantes/Cervantes_1.xml)), whereas "additionalFile" could be another file containing a plain text version of the same poem."""@en ;
    rdfs:domain <http://postdata.linhd.uned.es/ontology/postdata-core#Redaction> ;
    rdfs:isDefinedBy "http://postdata.linhd.uned.es/ontology/postdata-core/" ;
    rdfs:range xsd:anyURI .

<http://postdata.linhd.uned.es/ontology/postdata-core#additionalName> a owl:DatatypeProperty ;
    rdfs:label "additional Name"@en ;
    rdfs:comment """An additional name, such as a nickname, epithet, or alias, or any other descriptive phrase used within a personal name.

Taking as example the writer Charlotte Brontë, an "additionalName" would be her alias: "Currell Bell"."""@en ;
    rdfs:domain <http://postdata.linhd.uned.es/ontology/postdata-core#Person> ;
    rdfs:isDefinedBy "http://postdata.linhd.uned.es/ontology/postdata-core/" ;
    rdfs:range xsd:string .

<http://postdata.linhd.uned.es/ontology/postdata-core#alternativeName> a owl:DatatypeProperty ;
    rdfs:label "alternative Name"@en ;
    rdfs:comment """Alternative name that references the current Person. A person may have zero or several alternative names.

Taking as example the character "Aldonza Lorenzo" from the Quixote, an "alternativeName" could be "Dulcinea"."""@en ;
    rdfs:domain <http://postdata.linhd.uned.es/ontology/postdata-core#Person> ;
    rdfs:isDefinedBy "http://postdata.linhd.uned.es/ontology/postdata-core/" ;
    rdfs:range xsd:string .

<http://postdata.linhd.uned.es/ontology/postdata-core#alternativeTitle> a owl:DatatypeProperty ;
    rdfs:label "alternative Title"@en ;
    rdfs:comment """Alternative title, that is, other known denominations of a Poetic Work or a Redaction.

Taking as example the "Poema de Mio Cid", an "alternativeTitle" would be "Cantar de Mio Cid"."""@en ;
    rdfs:domain [ a owl:Class ;
            owl:unionOf ( <http://postdata.linhd.uned.es/ontology/postdata-core#PoeticWork> <http://postdata.linhd.uned.es/ontology/postdata-core#Redaction> ) ] ;
    rdfs:isDefinedBy "http://postdata.linhd.uned.es/ontology/postdata-core/" ;
    rdfs:range xsd:string .

<http://postdata.linhd.uned.es/ontology/postdata-core#audienceEducationLevel> a owl:DatatypeProperty ;
    rdfs:label "audience Education Level"@en ;
    rdfs:comment """Level of education of the recipients of a text/song.

Taking as example the play "La segunda Celestina" (Agustín de Salazar), "audienceEducationLevel" would be a learned audience."""@en ;
    rdfs:domain <http://postdata.linhd.uned.es/ontology/postdata-core#Redaction> ;
    rdfs:isDefinedBy "http://postdata.linhd.uned.es/ontology/postdata-core/" ;
    rdfs:range xsd:string .

<http://postdata.linhd.uned.es/ontology/postdata-core#biography> a owl:DatatypeProperty ;
    rdfs:label "biography"@en ;
    rdfs:comment """An account of a person's life written, composed, or produced by another.

Taking as example the poet Antonio Machado, "biography" could be: "Antonio Cipriano José María y Francisco de Santa Ana Machado y Ruiz (26 July 1875 – 22 February 1939), known as Antonio Machado, was a Spanish poet and one of the leading figures of the Spanish literary movement known as the Generation of '98. His work, initially modernist, evolved towards an intimate form of symbolism with romantic traits. He gradually developed a style characterised by both an engagement with humanity on one side and an almost Taoist contemplation of existence on the other, a synthesis that according to Machado echoed the most ancient popular wisdom. In Gerardo Diego's words, Machado "spoke in verse and lived in poetry."" (example extracted from Wikipedia)."""@en ;
    rdfs:domain <http://postdata.linhd.uned.es/ontology/postdata-core#Person> ;
    rdfs:isDefinedBy "http://postdata.linhd.uned.es/ontology/postdata-core/" ;
    rdfs:range xsd:string ;
    rdfs:subPropertyOf <http://purl.org/vocab/bio/0.1/biography> .

<http://postdata.linhd.uned.es/ontology/postdata-core#characterIn> a owl:ObjectProperty ;
    rdfs:label "character In"@en ;
    rdfs:comment "This property points to the text in which the current instance of Person or Organisation is a character."@en ;
    rdfs:domain <http://postdata.linhd.uned.es/ontology/postdata-core#Agent> ;
    rdfs:isDefinedBy "http://postdata.linhd.uned.es/ontology/postdata-core/" ;
    rdfs:range <http://postdata.linhd.uned.es/ontology/postdata-core#Redaction> ;
    owl:inverseOf <http://postdata.linhd.uned.es/ontology/postdata-core#hasCharacter> .

<http://postdata.linhd.uned.es/ontology/postdata-core#commentary> a owl:DatatypeProperty ;
    rdfs:label "commentary"@en ;
    rdfs:comment """An explanatory series of notes or comments; an explanatory essay or treatise on a text.

Taking as Opus example "Versos" by Fernando de Herrera, the comments Francisco de Quevedo wrote on his own edition along the text of the poems would form the "commentary"."""@en ;
    rdfs:domain [ a owl:Class ;
            owl:unionOf ( <http://postdata.linhd.uned.es/ontology/postdata-core#PoeticWork> <http://postdata.linhd.uned.es/ontology/postdata-core#Redaction> ) ] ;
    rdfs:isDefinedBy "http://postdata.linhd.uned.es/ontology/postdata-core/" ;
    rdfs:range xsd:string .

<http://postdata.linhd.uned.es/ontology/postdata-core#deathPlace> a owl:ObjectProperty ;
    rdfs:label "death Place"@en ;
    rdfs:comment "This property points to the instance of Place where the Person died"@en ;
    rdfs:domain <http://postdata.linhd.uned.es/ontology/postdata-core#Person> ;
    rdfs:isDefinedBy "http://postdata.linhd.uned.es/ontology/postdata-core/" ;
    rdfs:range <http://postdata.linhd.uned.es/ontology/postdata-core#Place> ;
    owl:inverseOf <http://postdata.linhd.uned.es/ontology/postdata-core#deathPlaceOf> .

<http://postdata.linhd.uned.es/ontology/postdata-core#dedicatedTo> a owl:ObjectProperty ;
    rdfs:label "dedicated To"@en ;
    rdfs:comment "This property points to a Person to whom the current text was dedicated. This means that a Redaction includes a dedicated text to another person in an explicit way (frequently at the beginning of the text)."@en ;
    rdfs:domain <http://postdata.linhd.uned.es/ontology/postdata-core#Redaction> ;
    rdfs:isDefinedBy "http://postdata.linhd.uned.es/ontology/postdata-core/" ;
    rdfs:range <http://postdata.linhd.uned.es/ontology/postdata-core#Person> ;
    owl:inverseOf <http://postdata.linhd.uned.es/ontology/postdata-core#hasDedication> .

<http://postdata.linhd.uned.es/ontology/postdata-core#depictedIn> a owl:ObjectProperty ;
    rdfs:label "depicted In"@en ;
    rdfs:comment "This property points to the work (instance of PoeticWork) or a redaction which depicts the Role at hand in relation to its contents. When the Role at hand is related to the agents that participated in the transmission of the work (e.g. sponsor), this property points to the entity affected by the current function"@en ;
    rdfs:domain <http://postdata.linhd.uned.es/ontology/postdata-core#Role> ;
    rdfs:isDefinedBy "http://postdata.linhd.uned.es/ontology/postdata-core/" ;
    rdfs:range [ a owl:Class ;
            owl:unionOf ( <http://postdata.linhd.uned.es/ontology/postdata-core#PoeticWork> <http://postdata.linhd.uned.es/ontology/postdata-core#Redaction> ) ] .

<http://postdata.linhd.uned.es/ontology/postdata-core#editorOf> a owl:ObjectProperty ;
    rdfs:label "editor Of"@en ;
    rdfs:comment "This property points to an instance of Redaction which was edited by the the current Person"@en ;
    rdfs:domain <http://postdata.linhd.uned.es/ontology/postdata-core#Person> ;
    rdfs:isDefinedBy "http://postdata.linhd.uned.es/ontology/postdata-core/" ;
    rdfs:range <http://postdata.linhd.uned.es/ontology/postdata-core#Redaction> ;
    owl:inverseOf <http://postdata.linhd.uned.es/ontology/postdata-core#hasEditor> .

<http://postdata.linhd.uned.es/ontology/postdata-core#ethnicity> a owl:DatatypeProperty ;
    rdfs:label "ethnicity" ;
    rdfs:comment """An ethnic group; a social group that shares a common and distinctive culture, religion, language, or the like.

Taking as Person example the poet "Antonio Enríquez Gómez", his "ethnicity" would be "crypto-Jewish"."""@en ;
    rdfs:domain <http://postdata.linhd.uned.es/ontology/postdata-core#Person> ;
    rdfs:isDefinedBy "http://postdata.linhd.uned.es/ontology/postdata-core/" ;
    rdfs:range xsd:string .

<http://postdata.linhd.uned.es/ontology/postdata-core#firstPartOf> a owl:ObjectProperty ;
    rdfs:comment "This property points to the container (an instance of Redaction) of which the item at hand is its first part"@en,
        "first Part of"@en ;
    rdfs:domain <http://postdata.linhd.uned.es/ontology/postdata-core#TextUnit> ;
    rdfs:isDefinedBy "http://postdata.linhd.uned.es/ontology/postdata-core/" ;
    rdfs:range <http://postdata.linhd.uned.es/ontology/postdata-core#Redaction> ;
    rdfs:subPropertyOf <http://www.ontologydesignpatterns.org/cp/owl/partof.owl#isPartOf> ;
    owl:inverseOf <http://postdata.linhd.uned.es/ontology/postdata-core#hasFirstPart> .

<http://postdata.linhd.uned.es/ontology/postdata-core#function> a owl:DatatypeProperty ;
    rdfs:label "function"@en ;
    rdfs:comment """Purpose of the work (e.g. prayer, spell, curse). A Poetic Work or Redaction may have several functions associated.

Taking as example the poem "Cantico delle creature" by San Francesco d’Assisi, "function" would be "prayer"."""@en ;
    rdfs:domain [ a owl:Class ;
            owl:unionOf ( <http://postdata.linhd.uned.es/ontology/postdata-core#PoeticWork> <http://postdata.linhd.uned.es/ontology/postdata-core#Redaction> ) ] ;
    rdfs:isDefinedBy "http://postdata.linhd.uned.es/ontology/postdata-core/" ;
    rdfs:range xsd:string ;
    rdfs:subPropertyOf owl:topDataProperty .

<http://postdata.linhd.uned.es/ontology/postdata-core#genName> a owl:DatatypeProperty ;
    rdfs:label "genName"@en ;
    rdfs:comment """It contains a name component used to distinguish otherwise similar names on the basis of the relative ages or generations of the persons named.

Taking as example the person "Felipe II", "genName" is "II"."""@en ;
    rdfs:domain <http://postdata.linhd.uned.es/ontology/postdata-core#Person> ;
    rdfs:isDefinedBy "http://postdata.linhd.uned.es/ontology/postdata-core/" ;
    rdfs:range xsd:string .

<http://postdata.linhd.uned.es/ontology/postdata-core#hasMember> a owl:ObjectProperty ;
    rdfs:label "has Member"@en ;
    rdfs:comment "This property points to a Person that belongs to the Organisation"@en ;
    rdfs:domain <http://postdata.linhd.uned.es/ontology/postdata-core#Organisation> ;
    rdfs:isDefinedBy "http://postdata.linhd.uned.es/ontology/postdata-core/" ;
    rdfs:range <http://postdata.linhd.uned.es/ontology/postdata-core#Person> ;
    owl:inverseOf <http://postdata.linhd.uned.es/ontology/postdata-core#isMemberOf> .

<http://postdata.linhd.uned.es/ontology/postdata-core#hasTextUnit> a owl:ObjectProperty ;
    rdfs:label "hasTextUnit"@en ;
    rdfs:comment "A text unit in an ordered list."@en ;
    rdfs:domain <http://postdata.linhd.uned.es/ontology/postdata-core#OrderedTextUnitList> ;
    rdfs:isDefinedBy "http://postdata.linhd.uned.es/ontology/postdata-core/" ;
    rdfs:range <http://postdata.linhd.uned.es/ontology/postdata-core#TextUnit> ;
    rdfs:subPropertyOf <http://purl.org/ontology/olo/core#slot> .

<http://postdata.linhd.uned.es/ontology/postdata-core#involves> a owl:ObjectProperty ;
    rdfs:label "involves"@en ;
    rdfs:comment "This property points to an Organisation, Person or Place which are related to the current instance of Event"@en ;
    rdfs:domain <http://postdata.linhd.uned.es/ontology/postdata-core#Event> ;
    rdfs:isDefinedBy "http://postdata.linhd.uned.es/ontology/postdata-core/" ;
    rdfs:range [ a owl:Class ;
            owl:unionOf ( <http://postdata.linhd.uned.es/ontology/postdata-core#Agent> <http://postdata.linhd.uned.es/ontology/postdata-core#Place> ) ] ;
    owl:inverseOf <http://postdata.linhd.uned.es/ontology/postdata-core#isInvolvedIn> .

<http://postdata.linhd.uned.es/ontology/postdata-core#isAnonymous> a owl:DatatypeProperty ;
    rdfs:label "is Anonymous"@en ;
    rdfs:comment """In case the identity of current instance of Creator is unknown.

Taking as example the creator of "Libro de Alexandre", "isAnonymous" is True because the author is unknown to this day."""@en ;
    rdfs:domain <http://postdata.linhd.uned.es/ontology/postdata-core#CreatorRole> ;
    rdfs:isDefinedBy "http://postdata.linhd.uned.es/ontology/postdata-core/" ;
    rdfs:range xsd:boolean .

<http://postdata.linhd.uned.es/ontology/postdata-core#isCalligram> a owl:DatatypeProperty ;
    rdfs:label "is Calligram"@en ;
    rdfs:comment """Whether it is a calligram, that is, a text visually arranged in a way that it forms an image associated with the text contents.

Taking as example the (calligram) poem "La Colombe poignardée et le Jet d’eau" by Apollinaire, "is Calligram" value is True."""@en ;
    rdfs:domain <http://postdata.linhd.uned.es/ontology/postdata-core#PoeticWork> ;
    rdfs:isDefinedBy "http://postdata.linhd.uned.es/ontology/postdata-core/" ;
    rdfs:range xsd:boolean .

<http://postdata.linhd.uned.es/ontology/postdata-core#isFictional> a owl:DatatypeProperty ;
    rdfs:label "is Fictional"@en ;
    rdfs:comment """Whether the person under analysis is a fictional character.

Taking as example the character "Don Quijote de la Mancha" will have a True value for "is Fictional" property."""@en ;
    rdfs:domain <http://postdata.linhd.uned.es/ontology/postdata-core#Person> ;
    rdfs:isDefinedBy "http://postdata.linhd.uned.es/ontology/postdata-core/" ;
    rdfs:range xsd:boolean ;
    rdfs:subPropertyOf owl:topDataProperty .

<http://postdata.linhd.uned.es/ontology/postdata-core#isRealisedThrough> a owl:ObjectProperty ;
    rdfs:label "is Realised Through"@en ;
    rdfs:comment "This property points to a text (an instance of Redaction) which is one of the materialisations of the work under analysis"@en ;
    rdfs:domain <http://postdata.linhd.uned.es/ontology/postdata-core#PoeticWork> ;
    rdfs:isDefinedBy "http://postdata.linhd.uned.es/ontology/postdata-core/" ;
    rdfs:range <http://postdata.linhd.uned.es/ontology/postdata-core#Redaction> ;
    owl:inverseOf <http://postdata.linhd.uned.es/ontology/postdata-core#realises> .

<http://postdata.linhd.uned.es/ontology/postdata-core#isRecordedBy> a owl:ObjectProperty ;
    rdfs:label "is Recorded By"@en ;
    rdfs:comment "This property points to the specific location in the text of the bibliographic item  (an instance of Location) that registers the current event"@en ;
    rdfs:domain <http://postdata.linhd.uned.es/ontology/postdata-core#Event> ;
    rdfs:isDefinedBy "http://postdata.linhd.uned.es/ontology/postdata-core/" ;
    rdfs:range <http://postdata.linhd.uned.es/ontology/postdata-transmission#Location> .

<http://postdata.linhd.uned.es/ontology/postdata-core#isSong> a owl:DatatypeProperty ;
    rdfs:label "is Song"@en ;
    rdfs:comment """Whether the Redaction was composed to be sung.

Taking as example the poetic work "Chanson de Roland", "is Song" is True because the work is part of a genre which was sang."""@en ;
    rdfs:domain [ a owl:Class ;
            owl:unionOf ( <http://postdata.linhd.uned.es/ontology/postdata-core#PoeticWork> <http://postdata.linhd.uned.es/ontology/postdata-core#Redaction> ) ] ;
    rdfs:isDefinedBy "http://postdata.linhd.uned.es/ontology/postdata-core/" ;
    rdfs:range xsd:boolean .

<http://postdata.linhd.uned.es/ontology/postdata-core#isWrongAttribution> a owl:DatatypeProperty ;
    rdfs:label "is Wrong Attribution"@en ;
    rdfs:comment """In case the identity of the current instance of Creator is certainly a wrong attribution. This is applied to the Creator Role associated to a Redaction.

Taking as example the poem "Muere lentamente" (by Martha Madeiros) which is erroneously attributed to Pablo Neruda, in the case Neruda is indicated as the author, "is Wrong Attribution" would be True."""@en ;
    rdfs:domain <http://postdata.linhd.uned.es/ontology/postdata-core#CreatorRole> ;
    rdfs:isDefinedBy "http://postdata.linhd.uned.es/ontology/postdata-core/" ;
    rdfs:range xsd:boolean .

<http://postdata.linhd.uned.es/ontology/postdata-core#keyword> a owl:DatatypeProperty ;
    rdfs:label "keyword"@en ;
    rdfs:comment """A significant or descriptive word. Usually, a word used as a reference point for finding other words or information.

Taking as example the theatre play "Othello" by Shakespeare, one possible "keyword" is "jealousy"."""@en ;
    rdfs:domain [ a owl:Class ;
            owl:unionOf ( <http://postdata.linhd.uned.es/ontology/postdata-core#PoeticWork> <http://postdata.linhd.uned.es/ontology/postdata-core#Redaction> ) ] ;
    rdfs:isDefinedBy "http://postdata.linhd.uned.es/ontology/postdata-core/" ;
    rdfs:range xsd:string .

<http://postdata.linhd.uned.es/ontology/postdata-core#language> a owl:DatatypeProperty ;
    rdfs:label "language"@en ;
    rdfs:comment """Language of the text. There might be several languages used in a Poetic Work or Redaction.

For example the "language" of "Romancero gitano" by Lorca, is "Spanish" (xsd:string). It could also be represented with the associated langauge code "es" (xsd:language)"""@en ;
    rdfs:domain [ a owl:Class ;
            owl:unionOf ( <http://postdata.linhd.uned.es/ontology/postdata-core#PoeticWork> <http://postdata.linhd.uned.es/ontology/postdata-core#Redaction> ) ] ;
    rdfs:isDefinedBy "http://postdata.linhd.uned.es/ontology/postdata-core/" ;
    rdfs:range [ a rdfs:Datatype ;
            owl:unionOf ( xsd:language xsd:string ) ] .

<http://postdata.linhd.uned.es/ontology/postdata-core#layout> a owl:DatatypeProperty ;
    rdfs:label "layout"@en ;
    rdfs:comment """The arrangement of textual materials (images included) on a page.

Taking as example "The Waste Land and Other Poems" by T.S. Eliot, edition by Broadview press, printed in 2011, the "the layout" can be described in the following way: "the text is left aligned, written in one column. Each stanza is followed by a blank space dividing it from the following stanza. The number of lines is displayed by a number marking every five lines which is aligned to the right edge of the page. Every page contains on average 30-40 lines"."""@en ;
    rdfs:domain <http://postdata.linhd.uned.es/ontology/postdata-core#Redaction> ;
    rdfs:isDefinedBy "http://postdata.linhd.uned.es/ontology/postdata-core/" ;
    rdfs:range xsd:string .

<http://postdata.linhd.uned.es/ontology/postdata-core#literaryTradition> a owl:DatatypeProperty ;
    rdfs:label "literary Tradition"@en ;
    rdfs:comment """The literary tradition assigned to a Poetic Work. There might be several values for this property.

Taking as example the theatre play "La vida es sueño" by Calderón de la Barca, "literary Tradition" is "Baroque"."""@en ;
    rdfs:domain <http://postdata.linhd.uned.es/ontology/postdata-core#PoeticWork> ;
    rdfs:isDefinedBy "http://postdata.linhd.uned.es/ontology/postdata-core/" ;
    rdfs:range xsd:string .

<http://postdata.linhd.uned.es/ontology/postdata-core#name> a owl:DatatypeProperty ;
    rdfs:label "name"@en ;
    rdfs:comment """Contains a proper noun or noun phrase that refers the current item.

Taking as example the full name of Federico García Lorca, "name" would be "Federico del Sagrado Corazón de Jesús García Lorca"."""@en ;
    rdfs:domain <http://postdata.linhd.uned.es/ontology/postdata-core#Person> ;
    rdfs:isDefinedBy "http://postdata.linhd.uned.es/ontology/postdata-core/" ;
    rdfs:range xsd:string ;
    rdfs:subPropertyOf <http://xmlns.com/foaf/0.1/name> .

<http://postdata.linhd.uned.es/ontology/postdata-core#nationality> a owl:DatatypeProperty ;
    rdfs:label "nationality"@en ;
    rdfs:comment """An ethnic group forming a part of one or more political nations.

Taking as example, the poet “Antonio Machado”, his “nationality” would be “Spanish”."""@en ;
    rdfs:domain <http://postdata.linhd.uned.es/ontology/postdata-core#Person> ;
    rdfs:isDefinedBy "http://postdata.linhd.uned.es/ontology/postdata-core/" ;
    rdfs:range xsd:string .

<http://postdata.linhd.uned.es/ontology/postdata-core#note> a owl:DatatypeProperty ;
    rdfs:label "note"@en ;
    rdfs:comment "Comment or explanation referred to a Place, Poetic Work, Redaction or Person"@en ;
    rdfs:domain [ a owl:Class ;
            owl:unionOf ( <http://postdata.linhd.uned.es/ontology/postdata-core#Place> <http://postdata.linhd.uned.es/ontology/postdata-core#PoeticWork> <http://postdata.linhd.uned.es/ontology/postdata-core#Redaction> <http://xmlns.com/foaf/0.1/Person> ) ] ;
    rdfs:isDefinedBy "http://postdata.linhd.uned.es/ontology/postdata-core/" ;
    rdfs:range xsd:string ;
    rdfs:subPropertyOf <http://purl.org/net/nknouf/ns/bibtex#hasNote> .

<http://postdata.linhd.uned.es/ontology/postdata-core#portrait> a owl:DatatypeProperty ;
    rdfs:label "portrait"@en ;
    rdfs:comment "URL to a digital image file that depicts the person"@en ;
    rdfs:domain <http://postdata.linhd.uned.es/ontology/postdata-core#Person> ;
    rdfs:isDefinedBy "http://postdata.linhd.uned.es/ontology/postdata-core/" ;
    rdfs:range xsd:anyURI .

<http://postdata.linhd.uned.es/ontology/postdata-core#positionName> a owl:DatatypeProperty ;
    rdfs:label "position Name"@en ;
    rdfs:comment "Contains a name component which indicates that the referent has a particular role or position in society, such as an official title or rank"@en ;
    rdfs:domain <http://postdata.linhd.uned.es/ontology/postdata-core#Person> ;
    rdfs:isDefinedBy "http://postdata.linhd.uned.es/ontology/postdata-core/" ;
    rdfs:range xsd:string ;
    rdfs:subPropertyOf owl:topDataProperty .

<http://postdata.linhd.uned.es/ontology/postdata-core#sampleText> a owl:DatatypeProperty ;
    rdfs:label "sample Text"@en ;
    rdfs:comment "Excerpt"@en ;
    rdfs:domain <http://postdata.linhd.uned.es/ontology/postdata-core#Redaction> ;
    rdfs:isDefinedBy "http://postdata.linhd.uned.es/ontology/postdata-core/" ;
    rdfs:range xsd:string .

<http://postdata.linhd.uned.es/ontology/postdata-core#subtitle> a owl:DatatypeProperty,
        owl:FunctionalProperty ;
    rdfs:label "subtitle"@en ;
    rdfs:comment "A secondary, usually explanatory title"@en ;
    rdfs:domain [ a owl:Class ;
            owl:unionOf ( <http://postdata.linhd.uned.es/ontology/postdata-core#PoeticWork> <http://postdata.linhd.uned.es/ontology/postdata-core#Redaction> ) ] ;
    rdfs:isDefinedBy "http://postdata.linhd.uned.es/ontology/postdata-core/" ;
    rdfs:range xsd:string ;
    rdfs:subPropertyOf <http://purl.org/spar/fabio/hasSubtitle> .

<http://postdata.linhd.uned.es/ontology/postdata-core#theme> a owl:DatatypeProperty ;
    rdfs:label "theme"@en ;
    rdfs:comment "Subject of a Poetic Work"@en ;
    rdfs:domain <http://postdata.linhd.uned.es/ontology/postdata-core#PoeticWork> ;
    rdfs:isDefinedBy "http://postdata.linhd.uned.es/ontology/postdata-core/" ;
    rdfs:range xsd:string .

<http://postdata.linhd.uned.es/ontology/postdata-core#typeOfCharacter> a owl:ObjectProperty ;
    rdfs:label "type Of Character"@en ;
    rdfs:comment "Type of character (eg. “main”, “antagonist”, etc.). The values are specified in a controlled vocabulary"@en ;
    rdfs:domain <http://postdata.linhd.uned.es/ontology/postdata-core#Role> ;
    rdfs:isDefinedBy "http://postdata.linhd.uned.es/ontology/postdata-core/" ;
    rdfs:range [ a owl:Restriction ;
            owl:hasValue <http://postdata.linhd.uned.es/kos/character-type> ;
            owl:onProperty skos:inScheme ],
        skos:Concept .

<http://postdata.linhd.uned.es/ontology/postdata-core#typeOfEvent> a owl:DatatypeProperty ;
    rdfs:label "type of Event"@en ;
    rdfs:comment "Type of event, for instance its modality (real, fictional...)"@en ;
    rdfs:domain <http://postdata.linhd.uned.es/ontology/postdata-core#Event> ;
    rdfs:isDefinedBy "http://postdata.linhd.uned.es/ontology/postdata-core/" ;
    rdfs:range xsd:string .

<http://postdata.linhd.uned.es/ontology/postdata-core#typeOfPlace> a owl:DatatypeProperty ;
    rdfs:label "type of Place"@en ;
    rdfs:comment "Type of place (e.g. fictional)"@en ;
    rdfs:domain <http://postdata.linhd.uned.es/ontology/postdata-core#Place> ;
    rdfs:isDefinedBy "http://postdata.linhd.uned.es/ontology/postdata-core/" ;
    rdfs:range xsd:string ;
    rdfs:subPropertyOf owl:topDataProperty .

<http://postdata.linhd.uned.es/ontology/postdata-core#typeOfRedaction> a owl:DatatypeProperty ;
    rdfs:label "type of Redaction"@en ;
    rdfs:comment """The type of the text provided in the Redaction
Eg.: Diplomatic edition, critical edition, translation"""@en ;
    rdfs:domain <http://postdata.linhd.uned.es/ontology/postdata-core#Redaction> ;
    rdfs:isDefinedBy "http://postdata.linhd.uned.es/ontology/postdata-core/" ;
    rdfs:range xsd:string .

<http://postdata.linhd.uned.es/ontology/postdata-core#unidentifiedSource> a owl:DatatypeProperty ;
    rdfs:label "unidentified Source"@en ;
    rdfs:comment "There are references that mentioned a PrimarySource for the text at hand but the real textual artefact has not been identified"@en ;
    rdfs:domain [ a owl:Class ;
            owl:unionOf ( <http://postdata.linhd.uned.es/ontology/postdata-core#PoeticWork> <http://postdata.linhd.uned.es/ontology/postdata-core#Redaction> ) ] ;
    rdfs:isDefinedBy "http://postdata.linhd.uned.es/ontology/postdata-core/" ;
    rdfs:range xsd:string .

<http://postdata.linhd.uned.es/ontology/postdata-dates> a owl:Ontology ;
    ns11:license "https://creativecommons.org/licenses/by/4.0/"@en ;
    dc:contributors """Alvaro Pérez (LINHD_POSTDATA-UNED)  
https://www.linkedin.com/in/álvaro-pérez-pozo-ab241154/"""@en,
        """Bruno Sartini (Bolonia University)
https://orcid.org/0000-0002-9152-4402"""@en,
        """Javier de la Rosa (LINHD_POSTDATA-UNED)
https://www.linkedin.com/in/versae/"""@en,
        """Oscar Corcho (Universidad Politécnica de Madrid)
http://orcid.org/0000-0002-9260-0753"""@en ;
    dc:creator """Helena Bermúdez Sabel 
https://orcid.org/0000-0001-7782-206X"""@en,
        """Mª Luisa Díez Platas 
https://orcid.org/0000-0002-9416-3147"""@en ;
    dc:date "2019-05-23"@en ;
    dc:description "This ontology coverage the classes and properties for dating the poetic opus and its manifestations"@en ;
    dc:title "postdata-dates ontology"@en ;
    terms:publisher """POSTDATA Project “This project has received funding from the European Research Council (ERC) under the European Union’s Horizon 2020 research and innovation programme (grant agreement Nº [679528])”
        Principal Investigator. Elena González Blanco -- <https://orcid.org/0000-0002-0448-1812>
        Technical Director. Salvador Ros Muñoz -- <https://orcid.org/0000-0001-6330-4958>"""@en ;
    vann:preferredNamespacePrefix "pddates"@en ;
    owl:versionInfo "V1.0" .

<http://postdata.linhd.uned.es/ontology/postdata-dates#ClosedIntervalExpression> a owl:Class ;
    rdfs:label "ClosedInterval"@en ;
    rdfs:comment "Exactly specified date range"@en ;
    rdfs:isDefinedBy "http://postdata.linhd.uned.es/ontology/postdata-dates" ;
    rdfs:subClassOf [ a owl:Restriction ;
            owl:allValuesFrom xsd:date ;
            owl:onProperty <http://schema.org/endDate> ],
        [ a owl:Restriction ;
            owl:allValuesFrom xsd:date ;
            owl:onProperty <http://schema.org/startDate> ],
        <http://postdata.linhd.uned.es/ontology/postdata-dates#IntervalExpression> .

<http://postdata.linhd.uned.es/ontology/postdata-dates#dateContent> a owl:DatatypeProperty ;
    rdfs:label "dateContent"@en ;
    rdfs:comment "Value of the date as xds: dates"@en ;
    rdfs:domain <http://postdata.linhd.uned.es/ontology/postdata-dates#ExactDateExpression> ;
    rdfs:isDefinedBy "http://postdata.linhd.uned.es/ontology/postdata-dates"@en ;
    rdfs:range xsd:date .

<http://postdata.linhd.uned.es/ontology/postdata-dates#dateNote> a owl:DatatypeProperty ;
    rdfs:label "dateNote"@en ;
    rdfs:comment "Comments in relation to a stated date"@en ;
    rdfs:domain <http://postdata.linhd.uned.es/ontology/postdata-dates#DateEntity> ;
    rdfs:isDefinedBy "http://postdata.linhd.uned.es/ontology/postdata-dates" ;
    rdfs:range xsd:string ;
    rdfs:subPropertyOf owl:topDataProperty .

<http://postdata.linhd.uned.es/ontology/postdata-dates#isExpressedAs> a owl:ObjectProperty ;
    rdfs:label "isExpressedAs"@en ;
    rdfs:comment "Property that associates with an Date Entity its form of expression"@en ;
    rdfs:domain <http://postdata.linhd.uned.es/ontology/postdata-dates#DateEntity> ;
    rdfs:isDefinedBy "http://postdata.linhd.uned.es/ontology/postdata-dates" ;
    rdfs:range <http://postdata.linhd.uned.es/ontology/postdata-dates#DateExpression> .

<http://postdata.linhd.uned.es/ontology/postdata-dates#notAfter> a owl:DatatypeProperty ;
    rdfs:label "notAfter"@en ;
    rdfs:comment "In uncertain dates, it specifies the latest possible date"@en ;
    rdfs:domain <http://postdata.linhd.uned.es/ontology/postdata-dates#OpenedIntervalExpression> ;
    rdfs:isDefinedBy "http://postdata.linhd.uned.es/ontology/postdata-dates" ;
    rdfs:range xsd:date ;
    rdfs:subPropertyOf owl:topDataProperty .

<http://postdata.linhd.uned.es/ontology/postdata-dates#notBefore> a owl:DatatypeProperty ;
    rdfs:label "notBefore"@en ;
    rdfs:comment "In uncertain dates, it specifies the earliest possible date"@en ;
    rdfs:domain <http://postdata.linhd.uned.es/ontology/postdata-dates#OpenedIntervalExpression> ;
    rdfs:isDefinedBy "http://postdata.linhd.uned.es/ontology/postdata-dates" ;
    rdfs:range xsd:date ;
    rdfs:subPropertyOf owl:topDataProperty .

<http://postdata.linhd.uned.es/ontology/postdata-literaryAnalysisElements> a owl:Ontology ;
    dc:contributors """Alvaro Pérez (LINHD_POSTDATA-UNED)
https://www.linkedin.com/in/álvaro-pérez-pozo-ab241154/"""@en,
        """Bruno Sartini (Bolonia University)
https://orcid.org/0000-0002-9152-4402"""@en,
        """Javier de la Rosa (LINHD_POSTDATA-UNED)
https://www.linkedin.com/in/versae/"""@en,
        """Oscar Corcho (Universidad Politécnica de Madrid)
http://orcid.org/0000-0002-9260-0753"""@en ;
    dc:creator """Mª Luisa Díez Platas 
https://orcid.org/0000-0002-9416-3147"""@en ;
    dc:description "This ontology supports the information necessary for the literary analysis of a poetic work. It focuses especially on rhetorical figures or figure of speech such as tropes and schemes."@en ;
    dc:title "postdata-literaryAnalysisElements ontology"@en ;
    terms:publisher "POSTDATA Project",
        """POSTDATA Project

“This project has received funding from the European Research Council (ERC) under the European Union’s Horizon 2020 research and innovation programme (grant agreement Nº [679528])”
Principal Investigator. Elena González Blanco -- https://orcid.org/0000-0002-0448-1812
Technical Director. Salvador Ros Muñoz -- https://orcid.org/0000-0001-6330-4958"""@en ;
    vann:preferredNamespacePrefix "postdata" ;
    owl:imports <http://postdata.linhd.uned.es/ontology/postdata-core>,
        <http://www.ontologydesignpatterns.org/cp/owl/partof.owl> ;
    owl:versionInfo "V1.0" ;
    ns1:license "https://creativecommons.org/licenses/by/4.0/"@en .

<http://postdata.linhd.uned.es/ontology/postdata-literaryAnalysisElements#UnitOfRhetoricalDevice> a owl:Class .

<http://postdata.linhd.uned.es/ontology/postdata-literaryAnalysisElements#hasAcrostic> a owl:ObjectProperty ;
    rdfs:label "hasAcrostic"@en ;
    rdfs:comment "This property points to the Acrostic contained in the current instance of the Redaction"@en ;
    rdfs:domain <http://postdata.linhd.uned.es/ontology/postdata-core#Redaction> ;
    rdfs:isDefinedBy "http://postdata.linhd.uned.es/ontology/postdata-literaryAnalysisElements/"@en ;
    rdfs:range <http://postdata.linhd.uned.es/ontology/postdata-literaryAnalysisElements#Acrostic> ;
    owl:inverseOf <http://postdata.linhd.uned.es/ontology/postdata-literaryAnalysisElements#isContainedIn> .

<http://postdata.linhd.uned.es/ontology/postdata-literaryAnalysisElements#hasContemporaryRelation> a owl:ObjectProperty ;
    rdfs:label "hasContemporaryRelation"@en ;
    rdfs:comment "This property points to the work under analysis (Redaction) with which the current cultural product, that is contemporary to it, has some kind of intertextual relationship"@en ;
    rdfs:domain <http://postdata.linhd.uned.es/ontology/postdata-literaryAnalysisElements#Intertextuality> ;
    rdfs:isDefinedBy "http://postdata.linhd.uned.es/ontology/postdata-literaryAnalysisElements/"@en ;
    rdfs:range <http://postdata.linhd.uned.es/ontology/postdata-core#Redaction> ;
    owl:inverseOf <http://postdata.linhd.uned.es/ontology/postdata-literaryAnalysisElements#isRelatedContemporaneouslyWith> .

<http://postdata.linhd.uned.es/ontology/postdata-literaryAnalysisElements#hasDerivedWork> a owl:ObjectProperty ;
    rdfs:label "hasDerivedWork"@en ;
    rdfs:comment "This property points to a cultural product (Intertextuality) which was based on the work under analysis"@en ;
    rdfs:domain <http://postdata.linhd.uned.es/ontology/postdata-core#Redaction> ;
    rdfs:isDefinedBy "http://postdata.linhd.uned.es/ontology/postdata-literaryAnalysisElements/"@en ;
    rdfs:range <http://postdata.linhd.uned.es/ontology/postdata-literaryAnalysisElements#Intertextuality> ;
    owl:inverseOf <http://postdata.linhd.uned.es/ontology/postdata-literaryAnalysisElements#isDerivedFrom> .

<http://postdata.linhd.uned.es/ontology/postdata-literaryAnalysisElements#hasRelationsWith> a owl:ObjectProperty ;
    rdfs:label "hasRelationsWith"@en ;
    rdfs:comment "This property points to the text under analysis (Redaction) with which the current cultural product has a generic intertextual relationship"@en ;
    rdfs:domain <http://postdata.linhd.uned.es/ontology/postdata-core#Redaction> ;
    rdfs:isDefinedBy "http://postdata.linhd.uned.es/ontology/postdata-literaryAnalysisElements/"@en ;
    rdfs:range <http://postdata.linhd.uned.es/ontology/postdata-literaryAnalysisElements#Intertextuality> ;
    owl:inverseOf <http://postdata.linhd.uned.es/ontology/postdata-literaryAnalysisElements#isRelatedWith> .

<http://postdata.linhd.uned.es/ontology/postdata-literaryAnalysisElements#hasSmallerUnits> a owl:ObjectProperty ;
    rdfs:label "hasSmallerUnits"@en ;
    rdfs:comment "The current instance of Figure of Speech can be decompounded in smaller units for a more granular anlysis (e.g. a kenning made of other kennings)"@en ;
    rdfs:domain <http://postdata.linhd.uned.es/ontology/postdata-literaryAnalysisElements#FigureOfSpeech> ;
    rdfs:isDefinedBy "http://postdata.linhd.uned.es/ontology/postdata-literaryAnalysisElements/"@en ;
    rdfs:range <http://postdata.linhd.uned.es/ontology/postdata-literaryAnalysisElements#FigureOfSpeech> ;
    owl:inverseOf <http://postdata.linhd.uned.es/ontology/postdata-literaryAnalysisElements#isSmallerUnitOf> .

<http://postdata.linhd.uned.es/ontology/postdata-literaryAnalysisElements#isAbecedarius> a owl:DatatypeProperty ;
    rdfs:label "isAbecedarius"@en ;
    rdfs:comment "Whether the composition is an abecedarius, that is an acrostic in which the first letter of every word, strophe or verse follows the order of the alphabet"@en ;
    rdfs:domain <http://postdata.linhd.uned.es/ontology/postdata-literaryAnalysisElements#Acrostic> ;
    rdfs:isDefinedBy "http://postdata.linhd.uned.es/ontology/postdata-literaryAnalysisElements/"@en ;
    rdfs:range xsd:boolean .

<http://postdata.linhd.uned.es/ontology/postdata-literaryAnalysisElements#isPresentIn> a owl:ObjectProperty ;
    rdfs:label "isPresentIn"@en ;
    rdfs:comment "This property points to the lines (instance of Line) or word (instance of Word) which contains the current item under analysis"@en ;
    rdfs:domain <http://postdata.linhd.uned.es/ontology/postdata-literaryAnalysisElements#FigureOfSpeech> ;
    rdfs:isDefinedBy "http://postdata.linhd.uned.es/ontology/postdata-literaryAnalysisElements/"@en ;
    rdfs:range <http://postdata.linhd.uned.es/ontology/postdata-structuralElements#Line> .

<http://postdata.linhd.uned.es/ontology/postdata-literaryAnalysisElements#isReferencedIn> a owl:ObjectProperty ;
    rdfs:label "isReferencedIn"@en ;
    rdfs:comment "This property points to the Acrostic in which the current instance of Person of Place is referenced"@en ;
    rdfs:isDefinedBy "http://postdata.linhd.uned.es/ontology/postdata-literaryAnalysisElements/"@en ;
    rdfs:range <http://postdata.linhd.uned.es/ontology/postdata-literaryAnalysisElements#Acrostic> ;
    owl:inverseOf <http://postdata.linhd.uned.es/ontology/postdata-literaryAnalysisElements#refersTo> .

<http://postdata.linhd.uned.es/ontology/postdata-literaryAnalysisElements#isSource> a owl:ObjectProperty ;
    rdfs:label "isSource"@en ;
    rdfs:comment "This property points to the text under analysis (Redaction) from which the current cultural product has derived"@en ;
    rdfs:domain <http://postdata.linhd.uned.es/ontology/postdata-literaryAnalysisElements#Intertextuality> ;
    rdfs:isDefinedBy "http://postdata.linhd.uned.es/ontology/postdata-literaryAnalysisElements/"@en ;
    rdfs:range <http://postdata.linhd.uned.es/ontology/postdata-core#Redaction> ;
    owl:inverseOf <http://postdata.linhd.uned.es/ontology/postdata-literaryAnalysisElements#usesAsSource> .

<http://postdata.linhd.uned.es/ontology/postdata-literaryAnalysisElements#locus> a owl:DatatypeProperty ;
    rdfs:label "locus"@en ;
    dc:creator "mluisadiez" ;
    rdfs:comment "The particular position of the item at hand in relation to the PrimarySource or in a text"@en ;
    rdfs:domain <http://postdata.linhd.uned.es/ontology/postdata-literaryAnalysisElements#Intertextuality> ;
    rdfs:isDefinedBy "http://postdata.linhd.uned.es/ontology/postdata-literaryAnalysisElements"@en ;
    rdfs:range xsd:string ;
    rdfs:subPropertyOf owl:topDataProperty .

<http://postdata.linhd.uned.es/ontology/postdata-literaryAnalysisElements#rhetoricalOperation> a owl:ObjectProperty ;
    rdfs:label "rethoricalOperation"@en ;
    rdfs:comment "Classification categories of speech figures in relation to rhetorical operations: addition, omission, transposition and permutation"@en ;
    rdfs:domain <http://postdata.linhd.uned.es/ontology/postdata-literaryAnalysisElements#FigureOfSpeech> ;
    rdfs:isDefinedBy "http://postdata.linhd.uned.es/ontology/postdata-literaryAnalysisElements/"@en ;
    rdfs:range [ a owl:Restriction ;
            owl:hasValue <http://postdata.linhd.uned.es/kos/rhetorical-operation> ;
            owl:onProperty skos:inScheme ],
        skos:Concept .

<http://postdata.linhd.uned.es/ontology/postdata-literaryAnalysisElements#schemeVariety> a owl:ObjectProperty ;
    rdfs:label "schemeCategory"@en ;
    rdfs:comment "Categorisation of the scheme"@en ;
    rdfs:domain <http://postdata.linhd.uned.es/ontology/postdata-literaryAnalysisElements#Scheme> ;
    rdfs:isDefinedBy "http://postdata.linhd.uned.es/ontology/postdata-literaryAnalysisElements/"@en ;
    rdfs:range [ a owl:Restriction ;
            owl:hasValue <http://postdata.linhd.uned.es/kos/scheme-variety> ;
            owl:onProperty skos:inScheme ],
        skos:Concept ;
    rdfs:subPropertyOf <http://postdata.linhd.uned.es/ontology/postdata-literaryAnalysisElements#figureVariety> .

<http://postdata.linhd.uned.es/ontology/postdata-literaryAnalysisElements#tropeVariety> a owl:ObjectProperty ;
    rdfs:label "tropeCategory"@en ;
    rdfs:comment "Categorisation of the trope"@en ;
    rdfs:domain <http://postdata.linhd.uned.es/ontology/postdata-literaryAnalysisElements#Trope> ;
    rdfs:isDefinedBy "http://postdata.linhd.uned.es/ontology/postdata-literaryAnalysisElements/"@en ;
    rdfs:range [ a owl:Restriction ;
            owl:hasValue <http://postdata.linhd.uned.es/kos/trope-variety> ;
            owl:onProperty skos:inScheme ],
        skos:Concept ;
    rdfs:subPropertyOf <http://postdata.linhd.uned.es/ontology/postdata-literaryAnalysisElements#figureVariety> .

<http://postdata.linhd.uned.es/ontology/postdata-literaryAnalysisElements#typeOfIntertextuality> a owl:ObjectProperty ;
    rdfs:label "typeOfIntertextuality"@en ;
    rdfs:comment "Categorisation of the work under analysis depending on the relationship between this work and other texts. E.g. “contrafactum”, “de seguir”, etc."@en ;
    rdfs:domain <http://postdata.linhd.uned.es/ontology/postdata-literaryAnalysisElements#Intertextuality> ;
    rdfs:isDefinedBy "http://postdata.linhd.uned.es/ontology/postdata-literaryAnalysisElements/"@en ;
    rdfs:range [ a owl:Restriction ;
            owl:hasValue <http://postdata.linhd.uned.es/kos/type-of-intertextuality> ;
            owl:onProperty skos:inScheme ],
        skos:Concept .

<http://postdata.linhd.uned.es/ontology/postdata-prosodicElements> a owl:Ontology ;
    dc:contributors """Alvaro Pérez (LINHD_POSTDATA-UNED)
https://www.linkedin.com/in/álvaro-pérez-pozo-ab241154/"""@en,
        """Bruno Sartini (Bolonia University)
https://orcid.org/0000-0002-9152-4402"""@en,
        """Javier de la Rosa (LINHD_POSTDATA-UNED)
https://www.linkedin.com/in/versae/"""@en,
        """Oscar Corcho (Universidad Politécnica de Madrid)
http://orcid.org/0000-0002-9260-0753"""@en ;
    dc:creator """Helena Bermúdez Sabel 
https://orcid.org/0000-0001-7782-206X"""@en,
        """Mª Luisa Díez Platas 
https://orcid.org/0000-0002-9416-3147"""@en ;
    dc:date "2019-07-12"@en ;
    dc:description """This ontology contains the classes and properties necessary to structure the information of a prosodic analysis, that is to say, the information obtained from the study of the meters and the forms of versification.
In poetry, the metric is the basic rhythmic structure of the verses of a poetic work."""@en ;
    dc:title "postdata-structural ontology"@en ;
    terms:publisher "POSTDATA Project",
        """POSTDATA Project

“This project has received funding from the European Research Council (ERC) under the European Union’s Horizon 2020 research and innovation programme (grant agreement Nº [679528])”
Principal Investigator. Elena González Blanco -- https://orcid.org/0000-0002-0448-1812
Technical Director. Salvador Ros Muñoz -- https://orcid.org/0000-0001-6330-4958"""@en ;
    vann:preferredNamespacePrefix "pdprosodic"@en ;
    owl:imports <http://postdata.linhd.uned.es/ontology/postdata-structuralElements#> ;
    owl:versionInfo "V1.0" ;
    ns1:license "https://creativecommons.org/licenses/by/4.0/"@en .

<http://postdata.linhd.uned.es/ontology/postdata-prosodicElements#affectsFirst> a owl:ObjectProperty ;
    rdfs:label "affectsFirst"@en ;
    rdfs:comment "This property points to the first of the words affected by a metaplasm"@en ;
    rdfs:domain <http://postdata.linhd.uned.es/ontology/postdata-prosodicElements#Metaplasm> ;
    rdfs:isDefinedBy "http://postdata.linhd.uned.es/ontology/postdata-prosodicElements"@en .

<http://postdata.linhd.uned.es/ontology/postdata-prosodicElements#analyses> a owl:ObjectProperty ;
    rdfs:label "analyses"@en ;
    rdfs:comment "This property points to an instance of Redaction, Line or Stanza in which a WorkPattern, StanzaPattern or LinePattern presents analytical information about the work as a whole, the stanzas or the lines,  respectively."@en ;
    rdfs:domain <http://postdata.linhd.uned.es/ontology/postdata-prosodicElements#Pattern> ;
    rdfs:isDefinedBy "http://postdata.linhd.uned.es/ontology/postdata-prosodicElements"@en ;
    owl:inverseOf <http://postdata.linhd.uned.es/ontology/postdata-prosodicElements#isAnalysedThrough> .

<http://postdata.linhd.uned.es/ontology/postdata-prosodicElements#clausulaScheme> a owl:DatatypeProperty ;
    rdfs:label "clausulaScheme"@en ;
    dc:creator "mluisadiez" ;
    rdfs:comment "Pattern of clausulae, that is, the ending of a line determined by the number of unstressed syllables following the last stressed one."@en ;
    rdfs:domain <http://postdata.linhd.uned.es/ontology/postdata-prosodicElements#StanzaPattern> ;
    rdfs:isDefinedBy "http://postdata.linhd.uned.es/ontology/postdata-prosodicElements"@en ;
    rdfs:range xsd:string ;
    rdfs:subPropertyOf owl:topDataProperty .

<http://postdata.linhd.uned.es/ontology/postdata-prosodicElements#corresponds> a owl:ObjectProperty ;
    rdfs:label "corresponds"@en ;
    rdfs:comment "This property points to the instance of Rhyme whose rhyming word is described by the current instance of RhymeMatch"@en ;
    rdfs:domain <http://postdata.linhd.uned.es/ontology/postdata-prosodicElements#RhymeMatch> ;
    rdfs:isDefinedBy "http://postdata.linhd.uned.es/ontology/postdata-prosodicElements"@en ;
    rdfs:range <http://postdata.linhd.uned.es/ontology/postdata-prosodicElements#Rhyme> ;
    owl:inverseOf <http://postdata.linhd.uned.es/ontology/postdata-prosodicElements#matches> .

<http://postdata.linhd.uned.es/ontology/postdata-prosodicElements#employs> a owl:ObjectProperty ;
    rdfs:label "employs"@en ;
    rdfs:comment "This propery points to a Symbol used in metrical notation being defined"@en ;
    rdfs:domain <http://postdata.linhd.uned.es/ontology/postdata-prosodicElements#MetricalEncoding> ;
    rdfs:isDefinedBy "http://postdata.linhd.uned.es/ontology/postdata-prosodicElements"@en ;
    rdfs:range <http://postdata.linhd.uned.es/ontology/postdata-prosodicElements#Symbol> ;
    owl:inverseOf <http://postdata.linhd.uned.es/ontology/postdata-prosodicElements#isEmployedIn> .

<http://postdata.linhd.uned.es/ontology/postdata-prosodicElements#ending> a owl:DatatypeProperty ;
    rdfs:label "ending"@en ;
    dc:creator "mluisadiez" ;
    dc:date "2018-06-16T18:39:21+00:00"^^xsd:dateTime ;
    rdfs:comment "Contents from the last stressed vowel of the rhyme to its end"@en ;
    rdfs:domain <http://postdata.linhd.uned.es/ontology/postdata-prosodicElements#Rhyme> ;
    rdfs:isDefinedBy "http://postdata.linhd.uned.es/ontology/postdata-prosodicElements"@en ;
    rdfs:range xsd:string ;
    rdfs:subPropertyOf owl:topDataProperty .

<http://postdata.linhd.uned.es/ontology/postdata-prosodicElements#finalConsonant> a owl:DatatypeProperty ;
    rdfs:label "finalConsonant"@en ;
    dc:creator "mluisadiez" ;
    dc:date "2018-06-16T18:39:21+00:00"^^xsd:dateTime ;
    rdfs:comment "Last consonant of rhyming word" ;
    rdfs:domain <http://postdata.linhd.uned.es/ontology/postdata-prosodicElements#Rhyme> ;
    rdfs:isDefinedBy "http://postdata.linhd.uned.es/ontology/postdata-prosodicElements"@en ;
    rdfs:range xsd:string ;
    rdfs:subPropertyOf owl:topDataProperty .

<http://postdata.linhd.uned.es/ontology/postdata-prosodicElements#footType> a owl:ObjectProperty ;
    rdfs:label "footType"@en ;
    rdfs:comment "Type of foot (e.g. iamb)"@en ;
    rdfs:domain <http://postdata.linhd.uned.es/ontology/postdata-prosodicElements#Foot> ;
    rdfs:isDefinedBy "http://postdata.linhd.uned.es/ontology/postdata-prosodicElements"@en ;
    rdfs:range [ a owl:Restriction ;
            owl:hasValue <http://postdata.linhd.uned.es/kos/foot-type> ;
            owl:onProperty skos:inScheme ],
        skos:Concept .

<http://postdata.linhd.uned.es/ontology/postdata-prosodicElements#hasFirstFoot> a owl:ObjectProperty ;
    rdfs:label "hasFirstFoot"@en ;
    dc:creator "mluisadiez" ;
    dc:date "2018-06-16T20:30:43+00:00"^^xsd:dateTime ;
    rdfs:comment "This property points to the first Foot of the line" ;
    rdfs:domain <http://postdata.linhd.uned.es/ontology/postdata-prosodicElements#LinePattern> ;
    rdfs:isDefinedBy "http://postdata.linhd.uned.es/ontology/postdata-prosodicElements"@en ;
    rdfs:range <http://postdata.linhd.uned.es/ontology/postdata-prosodicElements#Foot> ;
    rdfs:subPropertyOf owl:topObjectProperty ;
    owl:inverseOf <http://postdata.linhd.uned.es/ontology/postdata-prosodicElements#isFirstFoot> .

<http://postdata.linhd.uned.es/ontology/postdata-prosodicElements#hasFirstUnit> a owl:ObjectProperty ;
    rdfs:label "hasFirstUnit"@en ;
    rdfs:comment "This property points to the firt unit in which the foot is divided (an instance of FootDivision)"@en ;
    rdfs:domain <http://postdata.linhd.uned.es/ontology/postdata-prosodicElements#Foot> ;
    rdfs:isDefinedBy "http://postdata.linhd.uned.es/ontology/postdata-prosodicElements"@en ;
    rdfs:range <http://postdata.linhd.uned.es/ontology/postdata-prosodicElements#FootDivision> ;
    owl:inverseOf <http://postdata.linhd.uned.es/ontology/postdata-prosodicElements#isFirstUnit> .

<http://postdata.linhd.uned.es/ontology/postdata-prosodicElements#hasMetaplasm> a owl:DatatypeProperty ;
    rdfs:label "hasMetaplasm"@en ;
    rdfs:comment "If the line, word or syllable is affected by a metaplasm"@en ;
    rdfs:isDefinedBy "http://postdata.linhd.uned.es/ontology/postdata-prosodicElements"@en ;
    rdfs:range xsd:boolean ;
    rdfs:subPropertyOf owl:topDataProperty .

<http://postdata.linhd.uned.es/ontology/postdata-prosodicElements#hasRefrain> a owl:DatatypeProperty ;
    rdfs:label "hasRefrain"@en ;
    dc:creator "mluisadiez" ;
    dc:date "2018-06-16T18:39:21+00:00"^^xsd:dateTime ;
    rdfs:comment "Whether the work has a refrain" ;
    rdfs:domain <http://postdata.linhd.uned.es/ontology/postdata-prosodicElements#WorkPattern> ;
    rdfs:range xsd:boolean ;
    rdfs:subPropertyOf owl:topDataProperty .

<http://postdata.linhd.uned.es/ontology/postdata-prosodicElements#hasRhymeWord> a owl:ObjectProperty ;
    rdfs:label "hasRhymeWord"@en ;
    dc:creator "mluisadiez" ;
    dc:date "2018-06-16T20:30:43+00:00"^^xsd:dateTime ;
    rdfs:comment "This property points to the instance of Word for a further linguistic analysis/division by words"@en ;
    rdfs:domain <http://postdata.linhd.uned.es/ontology/postdata-prosodicElements#Rhyme> ;
    rdfs:isDefinedBy "http://postdata.linhd.uned.es/ontology/postdata-prosodicElements"@en ;
    rdfs:range <http://postdata.linhd.uned.es/ontology/postdata-structuralElements#Word> ;
    rdfs:subPropertyOf owl:topObjectProperty ;
    owl:inverseOf <http://postdata.linhd.uned.es/ontology/postdata-prosodicElements#isRhymeWord> .

<http://postdata.linhd.uned.es/ontology/postdata-prosodicElements#initialPhonemesPattern> a owl:DatatypeProperty ;
    rdfs:label "initialPhonemesPattern"@en ;
    dc:creator "mluisadiez" ;
    rdfs:comment "Initial phonemes of each word in a line, in alphabetical order to show sound repetitions"@en ;
    rdfs:domain <http://postdata.linhd.uned.es/ontology/postdata-prosodicElements#LinePattern> ;
    rdfs:isDefinedBy "http://postdata.linhd.uned.es/ontology/postdata-prosodicElements"@en ;
    rdfs:range xsd:string ;
    rdfs:subPropertyOf owl:topDataProperty .

<http://postdata.linhd.uned.es/ontology/postdata-prosodicElements#interStrophicRelations> a owl:DatatypeProperty ;
    rdfs:label "interStrophicRelations"@en ;
    dc:creator "mluisadiez" ;
    dc:date "2018-06-16T18:39:21+00:00"^^xsd:dateTime ;
    rdfs:comment "Type of technique used to related stanzas by the repetition of sounds" ;
    rdfs:domain <http://postdata.linhd.uned.es/ontology/postdata-prosodicElements#WorkPattern> ;
    rdfs:isDefinedBy "http://postdata.linhd.uned.es/ontology/postdata-prosodicElements"@en ;
    rdfs:range xsd:string ;
    rdfs:subPropertyOf owl:topDataProperty .

<http://postdata.linhd.uned.es/ontology/postdata-prosodicElements#isAffectedBy> a owl:ObjectProperty ;
    rdfs:label "isAffectedBy"@en ;
    rdfs:comment "Refers to the metaplasm that affects a word or syllable"@en ;
    rdfs:isDefinedBy "http://postdata.linhd.uned.es/ontology/postdata-prosodicElements"@en .

<http://postdata.linhd.uned.es/ontology/postdata-prosodicElements#isCatalectic> a owl:DatatypeProperty ;
    rdfs:label "isCatalectic"@en ;
    dc:creator "mluisadiez" ;
    rdfs:comment "Whether the instance at hand is the last foot of the line or hemistich and is lacking one syllable"@en ;
    rdfs:domain <http://postdata.linhd.uned.es/ontology/postdata-prosodicElements#Foot> ;
    rdfs:isDefinedBy "http://postdata.linhd.uned.es/ontology/postdata-prosodicElements"@en ;
    rdfs:range xsd:boolean ;
    rdfs:subPropertyOf owl:topDataProperty .

<http://postdata.linhd.uned.es/ontology/postdata-prosodicElements#isEcho> a owl:DatatypeProperty ;
    rdfs:label "isEcho"@en ;
    dc:creator "mluisadiez" ;
    dc:date "2018-06-16T18:39:21+00:00"^^xsd:dateTime ;
    rdfs:comment "Whether the word in a rhyming pair under analysis is the first one (false) or the second (true)"@en ;
    rdfs:domain <http://postdata.linhd.uned.es/ontology/postdata-prosodicElements#Rhyme> ;
    rdfs:isDefinedBy "http://postdata.linhd.uned.es/ontology/postdata-prosodicElements"@en ;
    rdfs:range xsd:boolean ;
    rdfs:subPropertyOf owl:topDataProperty .

<http://postdata.linhd.uned.es/ontology/postdata-prosodicElements#isEchoOf> a owl:ObjectProperty ;
    rdfs:label "isEchoOf"@en ;
    rdfs:comment "This property points to a following Word (echo) that that rhymes with the current instance of Word"@en ;
    rdfs:domain <http://postdata.linhd.uned.es/ontology/postdata-structuralElements#Word> ;
    rdfs:isDefinedBy "http://postdata.linhd.uned.es/ontology/postdata-prosodicElements"@en ;
    rdfs:range <http://postdata.linhd.uned.es/ontology/postdata-structuralElements#Word> .

<http://postdata.linhd.uned.es/ontology/postdata-prosodicElements#isFormedWith> a owl:ObjectProperty ;
    rdfs:label "isFormedWith"@en ;
    rdfs:comment "A metric syllable produced by the effect of a metaplasm, is formed by one or more syllables of a word."@en ;
    rdfs:domain <http://postdata.linhd.uned.es/ontology/postdata-prosodicElements#MetricalSyllable> ;
    rdfs:isDefinedBy "http://postdata.linhd.uned.es/ontology/postdata-prosodicElements"@en ;
    rdfs:range <http://postdata.linhd.uned.es/ontology/postdata-structuralElements#Syllable> .

<http://postdata.linhd.uned.es/ontology/postdata-prosodicElements#isHypermetre> a owl:DatatypeProperty ;
    rdfs:label "isHypermetre"@en ;
    dc:creator "mluisadiez" ;
    dc:date "2018-06-16T18:39:21+00:00"^^xsd:dateTime ;
    rdfs:comment "It has one or more syllables in addition to those found in a standard metrical unit or line of verse"@en ;
    rdfs:domain <http://postdata.linhd.uned.es/ontology/postdata-prosodicElements#LinePattern> ;
    rdfs:isDefinedBy "http://postdata.linhd.uned.es/ontology/postdata-prosodicElements"@en ;
    rdfs:range xsd:boolean ;
    rdfs:subPropertyOf owl:topDataProperty .

<http://postdata.linhd.uned.es/ontology/postdata-prosodicElements#isHypermetrical> a owl:DatatypeProperty ;
    rdfs:label "isHypermetrical"@en ;
    dc:creator "mluisadiez" ;
    rdfs:comment "Whether the instance at hand is the last foot of the line or hemistich and it contains extra syllables"@en ;
    rdfs:domain <http://postdata.linhd.uned.es/ontology/postdata-prosodicElements#Foot> ;
    rdfs:isDefinedBy "http://postdata.linhd.uned.es/ontology/postdata-prosodicElements"@en ;
    rdfs:range xsd:boolean ;
    rdfs:subPropertyOf owl:topDataProperty .

<http://postdata.linhd.uned.es/ontology/postdata-prosodicElements#isHypometre> a owl:DatatypeProperty ;
    rdfs:label "isHypometre"@en ;
    dc:creator "mluisadiez" ;
    dc:date "2018-06-16T18:39:21+00:00"^^xsd:dateTime ;
    rdfs:comment "It has one or more syllables less than to those found in a standard metrical unit or line of verse"@en ;
    rdfs:domain <http://postdata.linhd.uned.es/ontology/postdata-prosodicElements#LinePattern> ;
    rdfs:isDefinedBy "http://postdata.linhd.uned.es/ontology/postdata-prosodicElements"@en ;
    rdfs:range xsd:boolean ;
    rdfs:subPropertyOf owl:topDataProperty .

<http://postdata.linhd.uned.es/ontology/postdata-prosodicElements#isIrregular> a owl:DatatypeProperty ;
    rdfs:label "isIrregular"@en ;
    dc:creator "mluisadiez" ;
    rdfs:comment "Whether in comparison to the other lines, the current foot breaks a regular pattern"@en ;
    rdfs:domain <http://postdata.linhd.uned.es/ontology/postdata-prosodicElements#Foot> ;
    rdfs:isDefinedBy "http://postdata.linhd.uned.es/ontology/postdata-prosodicElements"@en ;
    rdfs:range xsd:boolean ;
    rdfs:subPropertyOf owl:topDataProperty .

<http://postdata.linhd.uned.es/ontology/postdata-prosodicElements#isIsometric> a owl:DatatypeProperty ;
    rdfs:label "isIsometric"@en ;
    dc:creator "mluisadiez" ;
    dc:date "2018-06-16T18:39:21+00:00"^^xsd:dateTime ;
    rdfs:comment "Whether the work is monometric, that is, if all lines have the same metrical analysis" ;
    rdfs:domain <http://postdata.linhd.uned.es/ontology/postdata-prosodicElements#WorkPattern> ;
    rdfs:isDefinedBy "http://postdata.linhd.uned.es/ontology/postdata-prosodicElements"@en ;
    rdfs:range xsd:boolean ;
    rdfs:subPropertyOf owl:topDataProperty .

<http://postdata.linhd.uned.es/ontology/postdata-prosodicElements#isIsostrophic> a owl:DatatypeProperty ;
    rdfs:label "isIsostrophic"@en ;
    dc:creator "mluisadiez" ;
    dc:date "2018-06-16T18:39:21+00:00"^^xsd:dateTime ;
    rdfs:comment "Whether all stanzas are metrically equivalent" ;
    rdfs:domain <http://postdata.linhd.uned.es/ontology/postdata-prosodicElements#WorkPattern> ;
    rdfs:isDefinedBy "http://postdata.linhd.uned.es/ontology/postdata-prosodicElements"@en ;
    rdfs:range xsd:boolean ;
    rdfs:subPropertyOf owl:topDataProperty .

<http://postdata.linhd.uned.es/ontology/postdata-prosodicElements#isPresentIn> a owl:ObjectProperty ;
    rdfs:label "isPresentIn"@en ;
    rdfs:comment "This property points to the text (instance of Redaction, Line or Stanza) which contains the current item under analysis"@en ;
    rdfs:domain <http://postdata.linhd.uned.es/ontology/postdata-prosodicElements#Rhyme> ;
    rdfs:isDefinedBy "http://postdata.linhd.uned.es/ontology/postdata-prosodicElements"@en ;
    rdfs:range [ a owl:Class ;
            owl:unionOf ( <http://postdata.linhd.uned.es/ontology/postdata-core#Redaction> <http://postdata.linhd.uned.es/ontology/postdata-structuralElements#Line> <http://postdata.linhd.uned.es/ontology/postdata-structuralElements#Stanza> ) ] ;
    owl:inverseOf <http://postdata.linhd.uned.es/ontology/postdata-prosodicElements#presents> .

<http://postdata.linhd.uned.es/ontology/postdata-prosodicElements#isRegular> a owl:DatatypeProperty ;
    rdfs:label "isRegular"@en ;
    dc:creator "mluisadiez" ;
    dc:date "2018-06-16T18:39:21+00:00"^^xsd:dateTime ;
    rdfs:comment "Regular metrics"@en ;
    rdfs:domain <http://postdata.linhd.uned.es/ontology/postdata-prosodicElements#LinePattern> ;
    rdfs:isDefinedBy "http://postdata.linhd.uned.es/ontology/postdata-prosodicElements"@en ;
    rdfs:range xsd:boolean ;
    rdfs:subPropertyOf owl:topDataProperty .

<http://postdata.linhd.uned.es/ontology/postdata-prosodicElements#isStressed> a owl:DatatypeProperty ;
    rdfs:label "isStressed"@en ;
    rdfs:comment "If the syllable or a metricla syllable has accent"@en ;
    rdfs:isDefinedBy "http://postdata.linhd.uned.es/ontology/postdata-prosodicElements"@en ;
    rdfs:range xsd:boolean .

<http://postdata.linhd.uned.es/ontology/postdata-prosodicElements#isUnissonant> a owl:DatatypeProperty ;
    rdfs:label "isUnissonant"@en ;
    dc:creator "mluisadiez" ;
    dc:date "2018-06-16T18:39:21+00:00"^^xsd:dateTime ;
    rdfs:comment "Whether all stanzas have the same rhyme" ;
    rdfs:domain <http://postdata.linhd.uned.es/ontology/postdata-prosodicElements#WorkPattern> ;
    rdfs:isDefinedBy "http://postdata.linhd.uned.es/ontology/postdata-prosodicElements"@en ;
    rdfs:range xsd:boolean ;
    rdfs:subPropertyOf owl:topDataProperty .

<http://postdata.linhd.uned.es/ontology/postdata-prosodicElements#isUsedBy> a owl:ObjectProperty ;
    rdfs:label "isUsedBy"@en ;
    rdfs:comment "This property points to an instance of LinePattern, StanzaPattern or WorkPattern which uses the convention defined in the current instance of MetricalEncoding"@en ;
    rdfs:domain <http://postdata.linhd.uned.es/ontology/postdata-prosodicElements#MetricalEncoding> ;
    rdfs:isDefinedBy "http://postdata.linhd.uned.es/ontology/postdata-prosodicElements"@en ;
    rdfs:range <http://postdata.linhd.uned.es/ontology/postdata-prosodicElements#Pattern> ;
    owl:inverseOf <http://postdata.linhd.uned.es/ontology/postdata-prosodicElements#uses> .

<http://postdata.linhd.uned.es/ontology/postdata-prosodicElements#label> a owl:DatatypeProperty ;
    rdfs:label "label"@en ;
    dc:creator "mluisadiez" ;
    dc:date "2018-06-16T18:39:21+00:00"^^xsd:dateTime ;
    rdfs:comment "String used to identify the item at hand (usually, “a”, “b”, “c”, etc.)"@en ;
    rdfs:domain <http://postdata.linhd.uned.es/ontology/postdata-prosodicElements#Rhyme> ;
    rdfs:isDefinedBy "http://postdata.linhd.uned.es/ontology/postdata-prosodicElements"@en ;
    rdfs:range xsd:string ;
    rdfs:subPropertyOf owl:topDataProperty .

<http://postdata.linhd.uned.es/ontology/postdata-prosodicElements#metricalCategory> a owl:ObjectProperty ;
    rdfs:label "metricalCategory"@en ;
    rdfs:comment "Major category to identify the metrical type (e.g. fixed forms vs strophic)"@en ;
    rdfs:domain <http://postdata.linhd.uned.es/ontology/postdata-prosodicElements#WorkPattern> ;
    rdfs:isDefinedBy "http://postdata.linhd.uned.es/ontology/postdata-prosodicElements"@en ;
    rdfs:range [ a owl:Restriction ;
            owl:hasValue <http://postdata.linhd.uned.es/kos/metrical-category> ;
            owl:onProperty skos:inScheme ],
        skos:Concept .

<http://postdata.linhd.uned.es/ontology/postdata-prosodicElements#metricalComplexity> a owl:ObjectProperty ;
    rdfs:label "metricalComplexity"@en ;
    rdfs:comment "Categorisation depending on the number of syllables: usually, less or more than eight"@en ;
    rdfs:domain <http://postdata.linhd.uned.es/ontology/postdata-prosodicElements#WorkPattern> ;
    rdfs:isDefinedBy "http://postdata.linhd.uned.es/ontology/postdata-prosodicElements"@en ;
    rdfs:range [ a owl:Restriction ;
            owl:hasValue <http://postdata.linhd.uned.es/kos/metrical-complexity> ;
            owl:onProperty skos:inScheme ],
        skos:Concept .

<http://postdata.linhd.uned.es/ontology/postdata-prosodicElements#metricalContext> a owl:ObjectProperty ;
    rdfs:label "metricalContext"@en ;
    rdfs:comment "Categorisation depending on whether all lines have the same number of syllables"@en ;
    rdfs:domain <http://postdata.linhd.uned.es/ontology/postdata-prosodicElements#WorkPattern> ;
    rdfs:isDefinedBy "http://postdata.linhd.uned.es/ontology/postdata-prosodicElements"@en ;
    rdfs:range [ a owl:Restriction ;
            owl:hasValue <http://postdata.linhd.uned.es/kos/metrical-context> ;
            owl:onProperty skos:inScheme ],
        skos:Concept .

<http://postdata.linhd.uned.es/ontology/postdata-prosodicElements#metricalSymbol> a owl:DatatypeProperty ;
    rdfs:label "metricalSymbol"@en ;
    rdfs:comment "Symbol use to define a feature in a metrical pattern"@en ;
    rdfs:domain <http://postdata.linhd.uned.es/ontology/postdata-prosodicElements#Symbol> ;
    rdfs:isDefinedBy "http://postdata.linhd.uned.es/ontology/postdata-prosodicElements"@en ;
    rdfs:range xsd:string .

<http://postdata.linhd.uned.es/ontology/postdata-prosodicElements#metricalSymbolExplanation> a owl:DatatypeProperty ;
    rdfs:label "metricalSymbolExplanation"@en ;
    rdfs:comment "Meaning of the symbol used in a metrical pattern"@en ;
    rdfs:domain <http://postdata.linhd.uned.es/ontology/postdata-prosodicElements#Symbol> ;
    rdfs:isDefinedBy "http://postdata.linhd.uned.es/ontology/postdata-prosodicElements"@en ;
    rdfs:range xsd:string .

<http://postdata.linhd.uned.es/ontology/postdata-prosodicElements#metricalTypeDescription> a owl:DatatypeProperty ;
    rdfs:label "metricalTypeDescription"@en ;
    dc:creator "mluisadiez" ;
    dc:date "2018-06-16T18:39:21+00:00"^^xsd:dateTime ;
    rdfs:comment "Commentary on the categorisation attending to metrics" ;
    rdfs:domain <http://postdata.linhd.uned.es/ontology/postdata-prosodicElements#WorkPattern> ;
    rdfs:isDefinedBy "http://postdata.linhd.uned.es/ontology/postdata-prosodicElements"@en ;
    rdfs:range xsd:string ;
    rdfs:subPropertyOf owl:topDataProperty .

<http://postdata.linhd.uned.es/ontology/postdata-prosodicElements#nextFoot> a owl:ObjectProperty ;
    rdfs:label "nextFoot"@en ;
    dc:creator "mluisadiez" ;
    dc:date "2018-06-16T20:30:43+00:00"^^xsd:dateTime ;
    rdfs:comment "This property points to the next instance of Foot"@en ;
    rdfs:domain <http://postdata.linhd.uned.es/ontology/postdata-prosodicElements#Foot> ;
    rdfs:isDefinedBy "http://postdata.linhd.uned.es/ontology/postdata-prosodicElements"@en ;
    rdfs:range <http://postdata.linhd.uned.es/ontology/postdata-prosodicElements#Foot> ;
    rdfs:subPropertyOf owl:topObjectProperty ;
    owl:inverseOf <http://postdata.linhd.uned.es/ontology/postdata-prosodicElements#previousFoot> .

<http://postdata.linhd.uned.es/ontology/postdata-prosodicElements#nextFootAfterCaesura> a owl:ObjectProperty ;
    rdfs:label "nextFootAfterCaesura"@en ;
    dc:creator "mluisadiez" ;
    dc:date "2018-06-16T20:30:43+00:00"^^xsd:dateTime ;
    rdfs:comment "This property points to the next instance of Foot when this is positioned after a caesura"@en ;
    rdfs:domain <http://postdata.linhd.uned.es/ontology/postdata-prosodicElements#Foot> ;
    rdfs:isDefinedBy "http://postdata.linhd.uned.es/ontology/postdata-prosodicElements"@en ;
    rdfs:range <http://postdata.linhd.uned.es/ontology/postdata-prosodicElements#Foot> ;
    rdfs:subPropertyOf owl:topObjectProperty ;
    owl:inverseOf <http://postdata.linhd.uned.es/ontology/postdata-prosodicElements#previousFootBeforeCaesura> .

<http://postdata.linhd.uned.es/ontology/postdata-prosodicElements#nextUnit> a owl:ObjectProperty ;
    rdfs:label "nextUnit"@en ;
    rdfs:comment "This property points to the next unit that forms the foot (an instance of FootDivision)"@en ;
    rdfs:domain <http://postdata.linhd.uned.es/ontology/postdata-prosodicElements#FootDivision> ;
    rdfs:isDefinedBy "http://postdata.linhd.uned.es/ontology/postdata-prosodicElements"@en ;
    rdfs:range <http://postdata.linhd.uned.es/ontology/postdata-prosodicElements#FootDivision> ;
    owl:inverseOf <http://postdata.linhd.uned.es/ontology/postdata-prosodicElements#previousUnit> .

<http://postdata.linhd.uned.es/ontology/postdata-prosodicElements#numberOfFeet> a owl:DatatypeProperty ;
    rdfs:label "numberOfFeet"@en ;
    dc:creator "mluisadiez" ;
    dc:date "2018-06-16T18:39:21+00:00"^^xsd:dateTime ;
    rdfs:comment "Number of feet"@en ;
    rdfs:domain <http://postdata.linhd.uned.es/ontology/postdata-prosodicElements#LinePattern> ;
    rdfs:isDefinedBy "http://postdata.linhd.uned.es/ontology/postdata-prosodicElements"@en ;
    rdfs:range xsd:positiveInteger ;
    rdfs:subPropertyOf owl:topDataProperty .

<http://postdata.linhd.uned.es/ontology/postdata-prosodicElements#numberOfLines> a owl:DatatypeProperty ;
    rdfs:label "numberOfLines"@en ;
    dc:creator "mluisadiez" ;
    dc:date "2018-06-16T18:39:21+00:00"^^xsd:dateTime ;
    rdfs:comment "Number of lines in item" ;
    rdfs:domain <http://postdata.linhd.uned.es/ontology/postdata-prosodicElements#StanzaPattern> ;
    rdfs:isDefinedBy "http://postdata.linhd.uned.es/ontology/postdata-prosodicElements"@en ;
    rdfs:range xsd:positiveInteger ;
    rdfs:subPropertyOf owl:topDataProperty .

<http://postdata.linhd.uned.es/ontology/postdata-prosodicElements#numberOfMorae> a owl:DatatypeProperty ;
    rdfs:label "numberOfMorae"@en ;
    dc:creator "mluisadiez" ;
    rdfs:comment "The number of morae the foot contains"@en ;
    rdfs:domain <http://postdata.linhd.uned.es/ontology/postdata-prosodicElements#Foot> ;
    rdfs:isDefinedBy "http://postdata.linhd.uned.es/ontology/postdata-prosodicElements"@en ;
    rdfs:range xsd:positiveInteger ;
    rdfs:subPropertyOf owl:topDataProperty .

<http://postdata.linhd.uned.es/ontology/postdata-prosodicElements#numberOfStanzas> a owl:DatatypeProperty ;
    rdfs:label "numberOfStanzas"@en ;
    dc:creator "mluisadiez" ;
    dc:date "2018-06-16T18:39:21+00:00"^^xsd:dateTime ;
    rdfs:comment "Number of stanzas" ;
    rdfs:domain <http://postdata.linhd.uned.es/ontology/postdata-prosodicElements#WorkPattern> ;
    rdfs:isDefinedBy "http://postdata.linhd.uned.es/ontology/postdata-prosodicElements"@en ;
    rdfs:range xsd:positiveInteger ;
    rdfs:subPropertyOf owl:topDataProperty .

<http://postdata.linhd.uned.es/ontology/postdata-prosodicElements#numberOfSyllables> a owl:DatatypeProperty ;
    rdfs:label "numberOfSyllables"@en ;
    dc:creator "mluisadiez" ;
    dc:date "2018-06-16T18:39:21+00:00"^^xsd:dateTime ;
    rdfs:comment "The exact number of syllables, that is, without paying attention to any metrical phenomena that may affect the counting"@en ;
    rdfs:domain <http://postdata.linhd.uned.es/ontology/postdata-prosodicElements#LinePattern> ;
    rdfs:isDefinedBy "http://postdata.linhd.uned.es/ontology/postdata-prosodicElements"@en ;
    rdfs:range xsd:positiveInteger ;
    rdfs:subPropertyOf owl:topDataProperty .

<http://postdata.linhd.uned.es/ontology/postdata-prosodicElements#phonemePattern> a owl:DatatypeProperty ;
    rdfs:label "phonemePattern"@en ;
    dc:creator "mluisadiez" ;
    dc:date "2018-06-16T18:39:21+00:00"^^xsd:dateTime ;
    rdfs:comment "All phonemes in a line represented by their nearest written equivalents. They could be arranged in alphabetical order to show sound repetitions"@en ;
    rdfs:domain <http://postdata.linhd.uned.es/ontology/postdata-prosodicElements#LinePattern> ;
    rdfs:isDefinedBy "http://postdata.linhd.uned.es/ontology/postdata-prosodicElements"@en ;
    rdfs:range xsd:string ;
    rdfs:subPropertyOf owl:topDataProperty .

<http://postdata.linhd.uned.es/ontology/postdata-prosodicElements#phonemePatternByManner> a owl:DatatypeProperty ;
    rdfs:label "phonemePatternByManner"@en ;
    dc:creator "mluisadiez" ;
    dc:date "2018-06-16T18:39:21+00:00"^^xsd:dateTime ;
    rdfs:comment "All phonemes in a line represented by manner of articulation. They could be arranged in alphabetical order to show sound repetitions. The coding scheme presented in one of the databases stands for the different manners of articulation of consonants, and at the same time groups together front and back vowels"@en ;
    rdfs:domain <http://postdata.linhd.uned.es/ontology/postdata-prosodicElements#LinePattern> ;
    rdfs:isDefinedBy "http://postdata.linhd.uned.es/ontology/postdata-prosodicElements"@en ;
    rdfs:range xsd:string ;
    rdfs:subPropertyOf owl:topDataProperty .

<http://postdata.linhd.uned.es/ontology/postdata-prosodicElements#phoneticTranscription> a owl:DatatypeProperty ;
    rdfs:label "phoneticTranscription"@en ;
    dc:creator "mluisadiez" ;
    dc:date "2018-06-16T18:39:21+00:00"^^xsd:dateTime ;
    rdfs:comment "Phonetic transcription"@en ;
    rdfs:domain <http://postdata.linhd.uned.es/ontology/postdata-prosodicElements#LinePattern> ;
    rdfs:isDefinedBy "http://postdata.linhd.uned.es/ontology/postdata-prosodicElements"@en ;
    rdfs:range xsd:string ;
    rdfs:subPropertyOf owl:topDataProperty .

<http://postdata.linhd.uned.es/ontology/postdata-prosodicElements#prefinalConsonants> a owl:DatatypeProperty ;
    rdfs:label "prefinalConsonants"@en ;
    dc:creator "mluisadiez" ;
    dc:date "2018-06-16T18:39:21+00:00"^^xsd:dateTime ;
    rdfs:comment "Consonants between the stressed vowel and the last consonant"@en ;
    rdfs:domain <http://postdata.linhd.uned.es/ontology/postdata-prosodicElements#Rhyme> ;
    rdfs:isDefinedBy "http://postdata.linhd.uned.es/ontology/postdata-prosodicElements"@en ;
    rdfs:range xsd:string ;
    rdfs:subPropertyOf owl:topDataProperty .

<http://postdata.linhd.uned.es/ontology/postdata-prosodicElements#rhymeCategory> a owl:DatatypeProperty ;
    rdfs:label "rhymeCategory"@en ;
    dc:creator "mluisadiez" ;
    dc:date "2018-06-16T18:39:21+00:00"^^xsd:dateTime ;
    rdfs:comment "Categorisation of the item at hand"@en ;
    rdfs:domain <http://postdata.linhd.uned.es/ontology/postdata-prosodicElements#Rhyme> ;
    rdfs:isDefinedBy "http://postdata.linhd.uned.es/ontology/postdata-prosodicElements"@en ;
    rdfs:range xsd:string ;
    rdfs:subPropertyOf owl:topDataProperty .

<http://postdata.linhd.uned.es/ontology/postdata-prosodicElements#rhymeDispositionType> a owl:ObjectProperty ;
    rdfs:label "rhymeDispositionType"@en ;
    rdfs:comment "Categorisation of the stanza according to the diposition of the rhymes (eg. “cross”, “pair”)"@en ;
    rdfs:domain <http://postdata.linhd.uned.es/ontology/postdata-prosodicElements#StanzaPattern> ;
    rdfs:isDefinedBy "http://postdata.linhd.uned.es/ontology/postdata-prosodicElements"@en ;
    rdfs:range [ a owl:Restriction ;
            owl:hasValue <http://postdata.linhd.uned.es/kos/rhymeDisposition-type> ;
            owl:onProperty skos:inScheme ],
        skos:Concept .

<http://postdata.linhd.uned.es/ontology/postdata-prosodicElements#rhymeGrapheme> a owl:DatatypeProperty ;
    rdfs:label "rhymeGrapheme"@en ;
    dc:creator "mluisadiez" ;
    dc:date "2018-06-16T18:39:21+00:00"^^xsd:dateTime ;
    rdfs:comment "Grapheme that represents the rhyming sounds"@en ;
    rdfs:domain <http://postdata.linhd.uned.es/ontology/postdata-prosodicElements#Rhyme> ;
    rdfs:isDefinedBy "http://postdata.linhd.uned.es/ontology/postdata-prosodicElements"@en ;
    rdfs:range xsd:string ;
    rdfs:subPropertyOf owl:topDataProperty .

<http://postdata.linhd.uned.es/ontology/postdata-prosodicElements#rhymePhoneme> a owl:DatatypeProperty ;
    rdfs:label "rhymePhoneme"@en ;
    dc:creator "mluisadiez" ;
    dc:date "2018-06-16T18:39:21+00:00"^^xsd:dateTime ;
    rdfs:comment "Phonetic transcription of the rhyming sounds"@en ;
    rdfs:domain <http://postdata.linhd.uned.es/ontology/postdata-prosodicElements#Rhyme> ;
    rdfs:isDefinedBy "http://postdata.linhd.uned.es/ontology/postdata-prosodicElements"@en ;
    rdfs:range xsd:string ;
    rdfs:subPropertyOf owl:topDataProperty .

<http://postdata.linhd.uned.es/ontology/postdata-prosodicElements#rhymeTypeProportion> a owl:DatatypeProperty ;
    rdfs:label "rhymeTypeProportion"@en ;
    dc:creator "mluisadiez" ;
    dc:date "2018-06-16T18:39:21+00:00"^^xsd:dateTime ;
    rdfs:comment "Proportion of the feminine/masculine rhymes of the poem" ;
    rdfs:domain <http://postdata.linhd.uned.es/ontology/postdata-prosodicElements#WorkPattern> ;
    rdfs:isDefinedBy "http://postdata.linhd.uned.es/ontology/postdata-prosodicElements"@en ;
    rdfs:range xsd:string ;
    rdfs:subPropertyOf owl:topDataProperty .

<http://postdata.linhd.uned.es/ontology/postdata-prosodicElements#rhymesWith> a owl:ObjectProperty ;
    rdfs:label "rhymesWith"@en ;
    rdfs:comment "This property points to an instance of Line that rhymes with the current Line under analysis"@en ;
    rdfs:domain <http://postdata.linhd.uned.es/ontology/postdata-structuralElements#Line> ;
    rdfs:isDefinedBy "http://postdata.linhd.uned.es/ontology/postdata-prosodicElements"@en ;
    rdfs:range <http://postdata.linhd.uned.es/ontology/postdata-structuralElements#Line> .

<http://postdata.linhd.uned.es/ontology/postdata-prosodicElements#scannedLine> a owl:DatatypeProperty ;
    rdfs:label "scannedLine"@en ;
    dc:creator "mluisadiez" ;
    dc:date "2018-06-16T18:39:21+00:00"^^xsd:dateTime ;
    rdfs:comment "A line metrically analysed, marked up in terms of syllable division and accent"@en ;
    rdfs:domain <http://postdata.linhd.uned.es/ontology/postdata-prosodicElements#LinePattern> ;
    rdfs:isDefinedBy "http://postdata.linhd.uned.es/ontology/postdata-prosodicElements"@en ;
    rdfs:range xsd:string ;
    rdfs:subPropertyOf owl:topDataProperty .

<http://postdata.linhd.uned.es/ontology/postdata-prosodicElements#scheme> a owl:DatatypeProperty ;
    rdfs:label "scheme"@en ;
    rdfs:comment "Abstraction that represents the outline of the unit through a pattern. E.g. “ox(o)“ to represent the type of syllables"@en ;
    rdfs:domain <http://postdata.linhd.uned.es/ontology/postdata-prosodicElements#Foot> ;
    rdfs:isDefinedBy "http://postdata.linhd.uned.es/ontology/postdata-prosodicElements"@en ;
    rdfs:range xsd:string .

<http://postdata.linhd.uned.es/ontology/postdata-prosodicElements#stressPosition> a owl:DatatypeProperty ;
    rdfs:label "stressPosition"@en ;
    rdfs:comment "Position of the stressed syllable from the end of the word"@en ;
    rdfs:domain <http://postdata.linhd.uned.es/ontology/postdata-structuralElements#Word> ;
    rdfs:isDefinedBy "http://postdata.linhd.uned.es/ontology/postdata-prosodicElements"@en ;
    rdfs:range xsd:integer .

<http://postdata.linhd.uned.es/ontology/postdata-prosodicElements#successIn> a owl:ObjectProperty ;
    rdfs:label "successIn"@en ;
    rdfs:comment "A metaplasm is presented in Line"@en ;
    rdfs:domain <http://postdata.linhd.uned.es/ontology/postdata-prosodicElements#Metaplasm> ;
    rdfs:range <http://postdata.linhd.uned.es/ontology/postdata-structuralElements#Line> .

<http://postdata.linhd.uned.es/ontology/postdata-prosodicElements#syllabicMetricalScheme> a owl:DatatypeProperty .

<http://postdata.linhd.uned.es/ontology/postdata-prosodicElements#typeOfMetaplasm> a owl:ObjectProperty ;
    rdfs:label "typeOfMetaplasm"@en ;
    rdfs:comment "Type of Metaplasm"@en ;
    rdfs:domain <http://postdata.linhd.uned.es/ontology/postdata-prosodicElements#Metaplasm> ;
    rdfs:range [ a owl:Restriction ;
            owl:hasValue <http://postdata.linhd.uned.es/kos/metaplasm-type> ;
            owl:onProperty skos:inScheme ],
        skos:Concept .

<http://postdata.linhd.uned.es/ontology/postdata-prosodicElements#typeOfRhymeMatching> a owl:ObjectProperty ;
    rdfs:label "typeOfRhymeMatching"@en ;
    rdfs:comment "Explain the degree in which the different rhyming sounds match (e.g. assonant, consonant, perfect, imperfect, half-rhyme...)"@en ;
    rdfs:domain <http://postdata.linhd.uned.es/ontology/postdata-prosodicElements#RhymeMatch> ;
    rdfs:isDefinedBy "http://postdata.linhd.uned.es/ontology/postdata-prosodicElements"@en ;
    rdfs:range [ a owl:Restriction ;
            owl:hasValue <http://postdata.linhd.uned.es/kos/rhymeMatching-type> ;
            owl:onProperty skos:inScheme ],
        skos:Concept .

<http://postdata.linhd.uned.es/ontology/postdata-prosodicElements#unitType> a owl:ObjectProperty ;
    rdfs:label "unitType"@en ;
    rdfs:comment "The type of unit that defines the foot division"@en ;
    rdfs:domain <http://postdata.linhd.uned.es/ontology/postdata-prosodicElements#FootDivision> ;
    rdfs:isDefinedBy "http://postdata.linhd.uned.es/ontology/postdata-prosodicElements"@en ;
    rdfs:range [ a owl:Restriction ;
            owl:hasValue <http://postdata.linhd.uned.es/kos/footUnit-type> ;
            owl:onProperty skos:inScheme ] .

<http://postdata.linhd.uned.es/ontology/postdata-prosodicElements#vc-audience> a rdfs:Datatype .

<http://postdata.linhd.uned.es/ontology/postdata-prosodicElements#vc-audienceEducationLevel> a rdfs:Datatype .

<http://postdata.linhd.uned.es/ontology/postdata-prosodicElements#vc-authorEducationLevel> a rdfs:Datatype .

<http://postdata.linhd.uned.es/ontology/postdata-prosodicElements#vc-birthDateCertainty> a rdfs:Datatype .

<http://postdata.linhd.uned.es/ontology/postdata-prosodicElements#vc-birthPlaceCertainty> a rdfs:Datatype .

<http://postdata.linhd.uned.es/ontology/postdata-prosodicElements#vc-certainty> a rdfs:Datatype .

<http://postdata.linhd.uned.es/ontology/postdata-prosodicElements#vc-clausula> a rdfs:Datatype .

<http://postdata.linhd.uned.es/ontology/postdata-prosodicElements#vc-clausulaSchemaType> a rdfs:Datatype .

<http://postdata.linhd.uned.es/ontology/postdata-prosodicElements#vc-dateCertainty> a rdfs:Datatype .

<http://postdata.linhd.uned.es/ontology/postdata-prosodicElements#vc-feetType> a rdfs:Datatype .

<http://postdata.linhd.uned.es/ontology/postdata-prosodicElements#vc-figureCategory> a rdfs:Datatype .

<http://postdata.linhd.uned.es/ontology/postdata-prosodicElements#vc-footType> a rdfs:Datatype .

<http://postdata.linhd.uned.es/ontology/postdata-prosodicElements#vc-function> a rdfs:Datatype .

<http://postdata.linhd.uned.es/ontology/postdata-prosodicElements#vc-gender> a rdfs:Datatype .

<http://postdata.linhd.uned.es/ontology/postdata-prosodicElements#vc-genre> a rdfs:Datatype .

<http://postdata.linhd.uned.es/ontology/postdata-prosodicElements#vc-metricalCategory> a rdfs:Datatype .

<http://postdata.linhd.uned.es/ontology/postdata-prosodicElements#vc-metricalComplexity> a rdfs:Datatype .

<http://postdata.linhd.uned.es/ontology/postdata-prosodicElements#vc-metricalContext> a rdfs:Datatype .

<http://postdata.linhd.uned.es/ontology/postdata-prosodicElements#vc-metricalType> a rdfs:Datatype .

<http://postdata.linhd.uned.es/ontology/postdata-prosodicElements#vc-poeticType> a rdfs:Datatype .

<http://postdata.linhd.uned.es/ontology/postdata-prosodicElements#vc-religiousAffiliation> a rdfs:Datatype .

<http://postdata.linhd.uned.es/ontology/postdata-prosodicElements#vc-rhymeCategory> a rdfs:Datatype .

<http://postdata.linhd.uned.es/ontology/postdata-prosodicElements#vc-rhymeDispositionType> a rdfs:Datatype .

<http://postdata.linhd.uned.es/ontology/postdata-prosodicElements#vc-roleFunction> a rdfs:Datatype .

<http://postdata.linhd.uned.es/ontology/postdata-prosodicElements#vc-script> a rdfs:Datatype .

<http://postdata.linhd.uned.es/ontology/postdata-prosodicElements#vc-socialStatus> a rdfs:Datatype .

<http://postdata.linhd.uned.es/ontology/postdata-prosodicElements#vc-typeOfBibliographicItem> a rdfs:Datatype .

<http://postdata.linhd.uned.es/ontology/postdata-prosodicElements#vc-typeOfCharacter> a rdfs:Datatype .

<http://postdata.linhd.uned.es/ontology/postdata-prosodicElements#vc-typeOfDesignation> a rdfs:Datatype .

<http://postdata.linhd.uned.es/ontology/postdata-prosodicElements#vc-typeOfEdition> a rdfs:Datatype .

<http://postdata.linhd.uned.es/ontology/postdata-prosodicElements#vc-typeOfEvent> a rdfs:Datatype .

<http://postdata.linhd.uned.es/ontology/postdata-prosodicElements#vc-typeOfIntertextuality> a rdfs:Datatype .

<http://postdata.linhd.uned.es/ontology/postdata-prosodicElements#vc-typeOfMusicalNotation> a rdfs:Datatype .

<http://postdata.linhd.uned.es/ontology/postdata-prosodicElements#vc-typeOfParatext> a rdfs:Datatype .

<http://postdata.linhd.uned.es/ontology/postdata-prosodicElements#vc-typeOfPlace> a rdfs:Datatype .

<http://postdata.linhd.uned.es/ontology/postdata-prosodicElements#vc-typeOfRedaction> a rdfs:Datatype .

<http://postdata.linhd.uned.es/ontology/postdata-prosodicElements#vc-typeOfRhymeMatching> a rdfs:Datatype .

<http://postdata.linhd.uned.es/ontology/postdata-prosodicElements#vc-typeOfStanza> a rdfs:Datatype .

<http://postdata.linhd.uned.es/ontology/postdata-prosodicElements#vc-typeOfStanzaEdition> a rdfs:Datatype .

<http://postdata.linhd.uned.es/ontology/postdata-prosodicElements#vc-unitType> a rdfs:Datatype .

<http://postdata.linhd.uned.es/ontology/postdata-prosodicElements#vc-versificationType> a rdfs:Datatype .

<http://postdata.linhd.uned.es/ontology/postdata-prosodicElements#vc-writingTechnique> a rdfs:Datatype .

<http://postdata.linhd.uned.es/ontology/postdata-prosodicElements#versificationType> a owl:ObjectProperty ;
    rdfs:label "versificationType"@en ;
    rdfs:comment "Type of metre: accentual verse, accentual-syllabic verse, syllabic verse, quantitative verse, etc."@en ;
    rdfs:domain <http://postdata.linhd.uned.es/ontology/postdata-prosodicElements#WorkPattern> ;
    rdfs:isDefinedBy "http://postdata.linhd.uned.es/ontology/postdata-prosodicElements"@en ;
    rdfs:range [ a owl:Restriction ;
            owl:hasValue <http://postdata.linhd.uned.es/kos/versification-type> ;
            owl:onProperty skos:inScheme ],
        skos:Concept .

<http://postdata.linhd.uned.es/ontology/postdata-prosodicElements#vowelTypeScheme> a owl:DatatypeProperty ;
    rdfs:label "vowelTypeScheme"@en ;
    dc:creator "mluisadiez" ;
    dc:date "2018-06-16T18:39:21+00:00"^^xsd:dateTime ;
    rdfs:comment "Linguistic properties of the vowels of the line"@en ;
    rdfs:domain <http://postdata.linhd.uned.es/ontology/postdata-prosodicElements#LinePattern> ;
    rdfs:isDefinedBy "http://postdata.linhd.uned.es/ontology/postdata-prosodicElements"@en ;
    rdfs:range xsd:string ;
    rdfs:subPropertyOf owl:topDataProperty .

<http://postdata.linhd.uned.es/ontology/postdata-structuralElements#Punctuation> a owl:Class ;
    rdfs:label "Punctuation"@en ;
    dc:creator "mluisadiez" ;
    rdfs:comment "Specific markings, signs and symbols that are used in and around sentences to give them structure and to allow for correct understanding and comprehension"@en ;
    rdfs:isDefinedBy "http://postdata.linhd.uned.es/ontology/postdata-structuralElements" ;
    rdfs:subClassOf [ a owl:Restriction ;
            owl:onDataRange xsd:string ;
            owl:onProperty <http://postdata.linhd.uned.es/ontology/postdata-structuralElements#content> ;
            owl:qualifiedCardinality "1"^^xsd:nonNegativeInteger ],
        <http://postdata.linhd.uned.es/ontology/postdata-structuralElements#Token> .

<http://postdata.linhd.uned.es/ontology/postdata-structuralElements#belongsToLine> a owl:ObjectProperty ;
    rdfs:label "belongsToLine"@en ;
    rdfs:comment "This property refers to the Line (viewed as a list of tokens) the token belongs to."@en ;
    rdfs:domain <http://postdata.linhd.uned.es/ontology/postdata-structuralElements#Token> ;
    rdfs:isDefinedBy "http://postdata.linhd.uned.es/ontology/postdata-structuralElements"@en ;
    rdfs:range <http://postdata.linhd.uned.es/ontology/postdata-structuralElements#Line> ;
    rdfs:subPropertyOf <http://purl.org/ontology/olo/core#ordered_list> ;
    owl:inverseOf <http://postdata.linhd.uned.es/ontology/postdata-structuralElements#hasToken> .

<http://postdata.linhd.uned.es/ontology/postdata-structuralElements#belongsToLineList> a owl:ObjectProperty ;
    rdfs:label "belongsToLineList"@en ;
    rdfs:comment "This property refers to the OrderedLineList , associated with a Redaction; the Line belongs to."@en ;
    rdfs:domain <http://postdata.linhd.uned.es/ontology/postdata-structuralElements#Line> ;
    rdfs:isDefinedBy "http://postdata.linhd.uned.es/ontology/postdata-structuralElements"@en ;
    rdfs:range <http://postdata.linhd.uned.es/ontology/postdata-structuralElements#OrderedLineList> ;
    rdfs:subPropertyOf <http://purl.org/ontology/olo/core#ordered_list> ;
    owl:inverseOf <http://postdata.linhd.uned.es/ontology/postdata-structuralElements#hasLineItem> .

<http://postdata.linhd.uned.es/ontology/postdata-structuralElements#belongsToStanza> a owl:ObjectProperty ;
    rdfs:label "belongsToStanza"@en ;
    rdfs:comment "This property refers to the Stanza (viewed as a list of lines) theLine belongs to."@en ;
    rdfs:domain <http://postdata.linhd.uned.es/ontology/postdata-structuralElements#Line> ;
    rdfs:isDefinedBy "http://postdata.linhd.uned.es/ontology/postdata-structuralElements"@en ;
    rdfs:range <http://postdata.linhd.uned.es/ontology/postdata-structuralElements#Stanza> ;
    rdfs:subPropertyOf <http://purl.org/ontology/olo/core#ordered_list> ;
    owl:inverseOf <http://postdata.linhd.uned.es/ontology/postdata-structuralElements#hasLine> .

<http://postdata.linhd.uned.es/ontology/postdata-structuralElements#belongsToStanzaList> a owl:ObjectProperty ;
    rdfs:label "belongsToStanzaList"@en ;
    rdfs:comment "This property refers to the OrderedStanzaList , associated with a Redaction; the Stanza belongs to."@en ;
    rdfs:domain <http://postdata.linhd.uned.es/ontology/postdata-structuralElements#Stanza> ;
    rdfs:isDefinedBy "http://postdata.linhd.uned.es/ontology/postdata-structuralElements"@en ;
    rdfs:range <http://postdata.linhd.uned.es/ontology/postdata-structuralElements#OrderedStanzaList> ;
    rdfs:subPropertyOf <http://purl.org/ontology/olo/core#ordered_list> ;
    owl:inverseOf <http://postdata.linhd.uned.es/ontology/postdata-structuralElements#hasStanzaItem> .

<http://postdata.linhd.uned.es/ontology/postdata-structuralElements#belongsToWord> a owl:ObjectProperty ;
    rdfs:label "belongsToWord"@en ;
    rdfs:comment "This property refers to the Word (viewed as a list of syllables) the Syllable belongs to."@en ;
    rdfs:domain <http://postdata.linhd.uned.es/ontology/postdata-structuralElements#Syllable> ;
    rdfs:isDefinedBy "http://postdata.linhd.uned.es/ontology/postdata-structuralElements"@en ;
    rdfs:range <http://postdata.linhd.uned.es/ontology/postdata-structuralElements#Word> ;
    rdfs:subPropertyOf <http://purl.org/ontology/olo/core#ordered_list> ;
    owl:inverseOf <http://postdata.linhd.uned.es/ontology/postdata-structuralElements#hasSyllable> .

<http://postdata.linhd.uned.es/ontology/postdata-structuralElements#coda> a owl:DatatypeProperty ;
    rdfs:label "coda"@en ;
    dc:creator "mluisadiez" ;
    rdfs:comment "Sound or sounds that follow the nucleus" ;
    rdfs:domain <http://postdata.linhd.uned.es/ontology/postdata-structuralElements#Syllable> ;
    rdfs:isDefinedBy "http://postdata.linhd.uned.es/ontology/postdata-structuralElements"@en ;
    rdfs:range xsd:string ;
    rdfs:subPropertyOf owl:topDataProperty .

<http://postdata.linhd.uned.es/ontology/postdata-structuralElements#containsMentionToAgent> a owl:ObjectProperty ;
    rdfs:label "containsMentionToAgent"@en ;
    rdfs:comment "Agent  that is mentioned on the line"@en ;
    rdfs:isDefinedBy "http://postdata.linhd.uned.es/ontology/postdata-structuralElements"@en ;
    rdfs:range <http://postdata.linhd.uned.es/ontology/postdata-core#Agent> ;
    rdfs:subPropertyOf <http://postdata.linhd.uned.es/ontology/postdata-structuralElements#containsMentionTo> .

<http://postdata.linhd.uned.es/ontology/postdata-structuralElements#containsMentionToPlace> a owl:ObjectProperty ;
    rdfs:label "containsMentionToPlace"@en ;
    rdfs:comment "Place that is mentioned on the line"@en ;
    rdfs:isDefinedBy "http://postdata.linhd.uned.es/ontology/postdata-structuralElements"@en ;
    rdfs:range <http://postdata.linhd.uned.es/ontology/postdata-core#Place> ;
    rdfs:subPropertyOf <http://postdata.linhd.uned.es/ontology/postdata-structuralElements#containsMentionTo> .

<http://postdata.linhd.uned.es/ontology/postdata-structuralElements#firstHemistich> a owl:DatatypeProperty ;
    rdfs:label "firstHemistich"@en ;
    rdfs:comment "This property points to the first division of the line (an instance of Line), such as the first hemistich"@en ;
    rdfs:domain <http://postdata.linhd.uned.es/ontology/postdata-structuralElements#Line> ;
    rdfs:isDefinedBy "http://postdata.linhd.uned.es/ontology/postdata-structuralElements"@en ;
    rdfs:range xsd:string .

<http://postdata.linhd.uned.es/ontology/postdata-structuralElements#hasFirstStanza> a owl:ObjectProperty ;
    rdfs:label "hasFirstStanza"@en ;
    rdfs:comment "This property points to the first group of lines (an instance of Stanza) which form the current element under analysis"@en ;
    rdfs:domain [ a owl:Class ;
            owl:unionOf ( <http://postdata.linhd.uned.es/ontology/postdata-core#Redaction> <http://postdata.linhd.uned.es/ontology/postdata-structuralElements#OrderedStanzaList> ) ] ;
    rdfs:isDefinedBy "http://postdata.linhd.uned.es/ontology/postdata-structuralElements"@en ;
    rdfs:range <http://postdata.linhd.uned.es/ontology/postdata-structuralElements#Stanza> ;
    owl:inverseOf <http://postdata.linhd.uned.es/ontology/postdata-structuralElements#isFirstStanza> .

<http://postdata.linhd.uned.es/ontology/postdata-structuralElements#hasFirstSyllable> a owl:ObjectProperty ;
    rdfs:domain <http://postdata.linhd.uned.es/ontology/postdata-structuralElements#Word> ;
    rdfs:range <http://postdata.linhd.uned.es/ontology/postdata-structuralElements#Syllable> ;
    owl:inverseOf <http://postdata.linhd.uned.es/ontology/postdata-structuralElements#isFirstSyllable> .

<http://postdata.linhd.uned.es/ontology/postdata-structuralElements#hasFirstToken> a owl:ObjectProperty ;
    rdfs:label "hasFirstToken"@en ;
    dc:creator "mluisadiez" ;
    rdfs:comment "This property points to one of the words (an instance of Punctuation or Word) which form the current element under analysis"@en ;
    rdfs:domain <http://postdata.linhd.uned.es/ontology/postdata-structuralElements#Line> ;
    rdfs:isDefinedBy "http://postdata.linhd.uned.es/ontology/postdata-structuralElements"@en ;
    rdfs:range <http://postdata.linhd.uned.es/ontology/postdata-structuralElements#Token> ;
    rdfs:subPropertyOf owl:topObjectProperty ;
    owl:inverseOf <http://postdata.linhd.uned.es/ontology/postdata-structuralElements#isFirstToken> .

<http://postdata.linhd.uned.es/ontology/postdata-structuralElements#hasLastStanza> a owl:ObjectProperty ;
    rdfs:label "hasLastStanza"@en ;
    rdfs:comment "This property points to the last Stanza  which form the current element under analysis"@en ;
    rdfs:domain [ a owl:Class ;
            owl:unionOf ( <http://postdata.linhd.uned.es/ontology/postdata-core#Redaction> <http://postdata.linhd.uned.es/ontology/postdata-structuralElements#OrderedStanzaList> ) ] ;
    rdfs:isDefinedBy "http://postdata.linhd.uned.es/ontology/postdata-structuralElements"@en ;
    rdfs:range <http://postdata.linhd.uned.es/ontology/postdata-structuralElements#Stanza> ;
    rdfs:subPropertyOf owl:topObjectProperty ;
    owl:inverseOf <http://postdata.linhd.uned.es/ontology/postdata-structuralElements#isLastStanza> .

<http://postdata.linhd.uned.es/ontology/postdata-structuralElements#hasLastSyllable> a owl:ObjectProperty ;
    rdfs:label "hasLastSyllable"@en ;
    rdfs:comment "This property points to the last Syllable which form the current element under analysis"@en ;
    rdfs:domain <http://postdata.linhd.uned.es/ontology/postdata-structuralElements#Word> ;
    rdfs:isDefinedBy "http://postdata.linhd.uned.es/ontology/postdata-structuralElements"@en ;
    rdfs:range <http://postdata.linhd.uned.es/ontology/postdata-structuralElements#Syllable> ;
    rdfs:subPropertyOf owl:topObjectProperty ;
    owl:inverseOf <http://postdata.linhd.uned.es/ontology/postdata-structuralElements#isLastSyllable> .

<http://postdata.linhd.uned.es/ontology/postdata-structuralElements#hasLastToken> a owl:ObjectProperty ;
    rdfs:label "hasLastToken"@en ;
    rdfs:comment "This property points to the last Token  which form the current element under analysis"@en ;
    rdfs:domain <http://postdata.linhd.uned.es/ontology/postdata-structuralElements#Line> ;
    rdfs:isDefinedBy "http://postdata.linhd.uned.es/ontology/postdata-structuralElements"@en ;
    rdfs:range <http://postdata.linhd.uned.es/ontology/postdata-structuralElements#Token> ;
    rdfs:subPropertyOf owl:topObjectProperty ;
    owl:inverseOf <http://postdata.linhd.uned.es/ontology/postdata-structuralElements#isLastToken> .

<http://postdata.linhd.uned.es/ontology/postdata-structuralElements#hasLineList> a owl:ObjectProperty ;
    rdfs:label "hasLineList"@en ;
    rdfs:comment "This property refers to the list of lines(the poem structured in lines) that the redaction contains to"@en ;
    rdfs:domain <http://postdata.linhd.uned.es/ontology/postdata-core#Redaction> ;
    rdfs:isDefinedBy "http://postdata.linhd.uned.es/ontology/postdata-structuralElements/"@en ;
    rdfs:range <http://postdata.linhd.uned.es/ontology/postdata-structuralElements#OrderedLineList> ;
    owl:inverseOf <http://postdata.linhd.uned.es/ontology/postdata-structuralElements#isLineListOfRedaction> .

<http://postdata.linhd.uned.es/ontology/postdata-structuralElements#hasStanzaList> a owl:ObjectProperty ;
    rdfs:label "hasStanzaList"@en ;
    rdfs:comment "This property refers to the list of stanzas (the poem structured in stanzas) that the redaction contains to"@en ;
    rdfs:domain <http://postdata.linhd.uned.es/ontology/postdata-core#Redaction> ;
    rdfs:isDefinedBy "http://postdata.linhd.uned.es/ontology/postdata-structuralElements/"@en ;
    rdfs:range <http://postdata.linhd.uned.es/ontology/postdata-structuralElements#OrderedStanzaList> ;
    owl:inverseOf <http://postdata.linhd.uned.es/ontology/postdata-structuralElements#isStanzaListOfRedaction> .

<http://postdata.linhd.uned.es/ontology/postdata-structuralElements#isCallOf> a owl:ObjectProperty ;
    rdfs:label "isCallOf"@en ;
    rdfs:comment "This property points to a previous Word (call) that rhymes with the current instance of Word"@en ;
    rdfs:domain <http://postdata.linhd.uned.es/ontology/postdata-structuralElements#Word> ;
    rdfs:isDefinedBy "http://postdata.linhd.uned.es/ontology/postdata-structuralElements"@en ;
    rdfs:range <http://postdata.linhd.uned.es/ontology/postdata-structuralElements#Word> .

<http://postdata.linhd.uned.es/ontology/postdata-structuralElements#isEchoOf> a owl:ObjectProperty ;
    rdfs:label "isEchoOf"@en ;
    rdfs:comment "This property points to a following Word (echo) that that rhymes with the current instance of Word"@en ;
    rdfs:domain <http://postdata.linhd.uned.es/ontology/postdata-structuralElements#Word> ;
    rdfs:isDefinedBy "http://postdata.linhd.uned.es/ontology/postdata-structuralElements"@en ;
    rdfs:range <http://postdata.linhd.uned.es/ontology/postdata-structuralElements#Word> .

<http://postdata.linhd.uned.es/ontology/postdata-structuralElements#isNotMetricStanza> a owl:DatatypeProperty ;
    rdfs:label "isNotMetricStanza"@en ;
    dc:creator "mluisadiez" ;
    rdfs:comment "If Stanza is a metrical unit, then this should be “no”. Otherwise (e.g. a section, a lai, etc.) it should be set to “yes”"@en ;
    rdfs:domain <http://postdata.linhd.uned.es/ontology/postdata-structuralElements#Stanza> ;
    rdfs:isDefinedBy "http://postdata.linhd.uned.es/ontology/postdata-structuralElements"@en ;
    rdfs:range xsd:boolean ;
    rdfs:subPropertyOf owl:topDataProperty .

<http://postdata.linhd.uned.es/ontology/postdata-structuralElements#isRefrainOmitted> a owl:DatatypeProperty ;
    rdfs:label "isRefrainOmitted"@en ;
    dc:creator "mluisadiez" ;
    rdfs:comment "Whether the copy of the refrain was omitted"@en ;
    rdfs:domain <http://postdata.linhd.uned.es/ontology/postdata-structuralElements#Stanza> ;
    rdfs:isDefinedBy "http://postdata.linhd.uned.es/ontology/postdata-structuralElements"@en ;
    rdfs:range xsd:boolean ;
    rdfs:subPropertyOf owl:topDataProperty .

<http://postdata.linhd.uned.es/ontology/postdata-structuralElements#isTheSameAs> a owl:ObjectProperty ;
    rdfs:label "isTheSameAs"@en ;
    dc:creator "mluisadiez" ;
    rdfs:comment "This property points to another instance of Stanza which belongs to another work or ensemble but that has the same contents as the current item at hand"@en ;
    rdfs:domain <http://postdata.linhd.uned.es/ontology/postdata-structuralElements#Stanza> ;
    rdfs:isDefinedBy "http://postdata.linhd.uned.es/ontology/postdata-structuralElements"@en ;
    rdfs:range <http://postdata.linhd.uned.es/ontology/postdata-structuralElements#Stanza> ;
    rdfs:subPropertyOf owl:topObjectProperty .

<http://postdata.linhd.uned.es/ontology/postdata-structuralElements#nextLine> a owl:ObjectProperty ;
    rdfs:label "nextLine"@en ;
    rdfs:comment "This property points to next Line of the Line under analysis, in a OrderedLineList or in a Stanza"@en ;
    rdfs:domain <http://postdata.linhd.uned.es/ontology/postdata-structuralElements#Line> ;
    rdfs:isDefinedBy "http://postdata.linhd.uned.es/ontology/postdata-structuralElements"@en ;
    rdfs:range <http://postdata.linhd.uned.es/ontology/postdata-structuralElements#Line> ;
    rdfs:subPropertyOf <http://purl.org/ontology/olo/core#next> ;
    owl:inverseOf <http://postdata.linhd.uned.es/ontology/postdata-structuralElements#previousLine> .

<http://postdata.linhd.uned.es/ontology/postdata-structuralElements#nextStanza> a owl:ObjectProperty ;
    rdfs:label "nextStanza"@en ;
    dc:creator "mluisadiez" ;
    rdfs:comment "This property points to  Stanza that follows the Stanza under analysis in a OrderedStanzaList"@en ;
    rdfs:domain <http://postdata.linhd.uned.es/ontology/postdata-structuralElements#Stanza> ;
    rdfs:isDefinedBy "http://postdata.linhd.uned.es/ontology/postdata-structuralElements"@en ;
    rdfs:range <http://postdata.linhd.uned.es/ontology/postdata-structuralElements#Stanza> ;
    rdfs:subPropertyOf <http://purl.org/ontology/olo/core#next> ;
    owl:inverseOf <http://postdata.linhd.uned.es/ontology/postdata-structuralElements#previousStanza> .

<http://postdata.linhd.uned.es/ontology/postdata-structuralElements#nextSyllable> a owl:ObjectProperty ;
    rdfs:label "nextSyllable"@en ;
    rdfs:comment "This property points to the Syllale that follows the Syllable under analysis in a Word"@en ;
    rdfs:domain <http://postdata.linhd.uned.es/ontology/postdata-structuralElements#Syllable> ;
    rdfs:isDefinedBy "http://postdata.linhd.uned.es/ontology/postdata-structuralElements"@en ;
    rdfs:range <http://postdata.linhd.uned.es/ontology/postdata-structuralElements#Syllable> ;
    rdfs:subPropertyOf <http://purl.org/ontology/olo/core#next> ;
    owl:inverseOf <http://postdata.linhd.uned.es/ontology/postdata-structuralElements#previousSyllable> .

<http://postdata.linhd.uned.es/ontology/postdata-structuralElements#nextToken> a owl:ObjectProperty ;
    rdfs:label "nextToken"@en ;
    dc:creator "mluisadiez" ;
    dc:date "2018-06-16T20:30:43+00:00"^^xsd:dateTime ;
    rdfs:comment "This property points to a Token that follows the current Token under analysis in a Line"@en,
        "This property points to an instance of Word that follows the current item under analysis"@en ;
    rdfs:domain <http://postdata.linhd.uned.es/ontology/postdata-structuralElements#Token> ;
    rdfs:range <http://postdata.linhd.uned.es/ontology/postdata-structuralElements#Token> ;
    rdfs:subPropertyOf <http://purl.org/ontology/olo/core#next> ;
    owl:inverseOf <http://postdata.linhd.uned.es/ontology/postdata-structuralElements#previousToken> .

<http://postdata.linhd.uned.es/ontology/postdata-structuralElements#nucleusType> a owl:ObjectProperty ;
    rdfs:label "nucleusType"@en ;
    rdfs:comment "Type of syllabic nucleus (linguistic typology)"@en ;
    rdfs:domain <http://postdata.linhd.uned.es/ontology/postdata-structuralElements#Syllable> ;
    rdfs:isDefinedBy "http://postdata.linhd.uned.es/ontology/postdata-structuralElements"@en ;
    rdfs:range [ a owl:Restriction ;
            owl:hasValue <http://postdata.linhd.uned.es/kos/nucleus-type> ;
            owl:onProperty skos:inScheme ],
        skos:Concept .

<http://postdata.linhd.uned.es/ontology/postdata-structuralElements#onset> a owl:DatatypeProperty ;
    rdfs:label "onset"@en ;
    dc:creator "mluisadiez" ;
    rdfs:comment "Sound or sounds occurring before the nucleus, a consonant or consonant cluster"@en ;
    rdfs:domain <http://postdata.linhd.uned.es/ontology/postdata-structuralElements#Syllable> ;
    rdfs:isDefinedBy "http://postdata.linhd.uned.es/ontology/postdata-structuralElements"@en ;
    rdfs:range xsd:string ;
    rdfs:subPropertyOf owl:topDataProperty .

<http://postdata.linhd.uned.es/ontology/postdata-structuralElements#partOfSpeech> a owl:ObjectProperty ;
    rdfs:label "partOfSpeech"@en ;
    rdfs:comment """A category of words (or, more generally, of lexical items) that have similar grammatical properties. 
Commonly listed  parts of speech are noun, verb, adjective, adverb, pronoun, preposition, conjunction, interjection, and sometimes numeral, article, or determiner."""@en ;
    rdfs:domain <http://postdata.linhd.uned.es/ontology/postdata-structuralElements#Word> ;
    rdfs:isDefinedBy "http://postdata.linhd.uned.es/ontology/postdata-structuralElements/"@en ;
    rdfs:range [ a owl:Restriction ;
            owl:hasValue <http://postdata.linhd.uned.es/kos/part-of-speech> ;
            owl:onProperty skos:inScheme ],
        skos:Concept ;
    rdfs:subPropertyOf owl:topObjectProperty .

<http://postdata.linhd.uned.es/ontology/postdata-structuralElements#positionInWord> a owl:DatatypeProperty ;
    rdfs:label "positionInWord"@en ;
    dc:creator "mluisadiez" ;
    rdfs:comment """Position of the syllable in the word 
Eg.: 3/4 (= third syllable in a four-syllable word)"""@en ;
    rdfs:domain <http://postdata.linhd.uned.es/ontology/postdata-structuralElements#Syllable> ;
    rdfs:isDefinedBy "http://postdata.linhd.uned.es/ontology/postdata-structuralElements"@en ;
    rdfs:range xsd:string ;
    rdfs:subPropertyOf owl:topDataProperty .

<http://postdata.linhd.uned.es/ontology/postdata-structuralElements#secondHemistich> a owl:DatatypeProperty ;
    rdfs:label "secondHemistich" ;
    rdfs:comment "This property points to the first division of the line (an instance of Line), such as the second hemistich" ;
    rdfs:domain <http://postdata.linhd.uned.es/ontology/postdata-structuralElements#Line> ;
    rdfs:isDefinedBy "http://postdata.linhd.uned.es/ontology/postdata-structuralElements" ;
    rdfs:range xsd:string .

<http://postdata.linhd.uned.es/ontology/postdata-structuralElements#sense> a owl:DatatypeProperty ;
    rdfs:label "sense"@en ;
    dc:creator "mluisadiez" ;
    rdfs:comment "One of the meanings of a word or phrase"@en ;
    rdfs:domain <http://postdata.linhd.uned.es/ontology/postdata-structuralElements#Word> ;
    rdfs:isDefinedBy "http://postdata.linhd.uned.es/ontology/postdata-structuralElements"@en ;
    rdfs:range xsd:string ;
    rdfs:subPropertyOf owl:topDataProperty .

<http://postdata.linhd.uned.es/ontology/postdata-structuralElements#stanzaNumber> a owl:DatatypeProperty ;
    rdfs:label "stanzaNumber"@en ;
    rdfs:comment "Position of the stanza inside the composition"@en ;
    rdfs:domain <http://postdata.linhd.uned.es/ontology/postdata-structuralElements#Stanza> ;
    rdfs:isDefinedBy "http://postdata.linhd.uned.es/ontology/postdata-structuralElements"@en ;
    rdfs:range xsd:positiveInteger ;
    rdfs:subPropertyOf <http://purl.org/ontology/olo/core#index> .

<http://postdata.linhd.uned.es/ontology/postdata-structuralElements#translation> a owl:DatatypeProperty ;
    rdfs:label "translation"@en ;
    dc:creator "mluisadiez" ;
    rdfs:comment "Translation of the word"@en ;
    rdfs:domain <http://postdata.linhd.uned.es/ontology/postdata-structuralElements#Word> ;
    rdfs:isDefinedBy "http://postdata.linhd.uned.es/ontology/postdata-structuralElements"@en ;
    rdfs:range xsd:string ;
    rdfs:subPropertyOf owl:topDataProperty .

<http://postdata.linhd.uned.es/ontology/postdata-structuralElements#typeOfStanza> a owl:ObjectProperty ;
    rdfs:label "typeOfStanza"@en ;
    rdfs:comment "Type of stanza, but not in relation to its metrics. E.g. tornada, refrain"@en ;
    rdfs:domain <http://postdata.linhd.uned.es/ontology/postdata-structuralElements#Stanza> ;
    rdfs:isDefinedBy "http://postdata.linhd.uned.es/ontology/postdata-structuralElements"@en ;
    rdfs:range [ a owl:Restriction ;
            owl:hasValue <http://postdata.linhd.uned.es/kos/stanza-type> ;
            owl:onProperty skos:inScheme ],
        skos:Concept .

<http://postdata.linhd.uned.es/ontology/postdata-structuralElements#typeOfStanzaEdition> a owl:ObjectProperty ;
    rdfs:label "typeOfStanzaEdition"@en ;
    rdfs:comment """The type of the text provided in the Stanza 
Eg.: Diplomatic edition, critical edition, translation"""@en ;
    rdfs:domain <http://postdata.linhd.uned.es/ontology/postdata-structuralElements#Stanza> ;
    rdfs:isDefinedBy "http://postdata.linhd.uned.es/ontology/postdata-structuralElements"@en ;
    rdfs:range [ a owl:Restriction ;
            owl:hasValue <http://postdata.linhd.uned.es/kos/stanzaEdition-type> ;
            owl:onProperty skos:inScheme ],
        skos:Concept .

<http://postdata.linhd.uned.es/ontology/postdata-structuralElements#weight> a owl:DatatypeProperty ;
    rdfs:label "weight"@en ;
    dc:creator "mluisadiez" ;
    rdfs:comment "Pattern according to the number and/or duration of segments in the syllabic rime, that is, the nucleus and coda"@en ;
    rdfs:domain <http://postdata.linhd.uned.es/ontology/postdata-structuralElements#Syllable> ;
    rdfs:isDefinedBy "pdstruct:positionInWord max 1 xsd:string"@en ;
    rdfs:range xsd:string ;
    rdfs:subPropertyOf owl:topDataProperty .

<http://postdata.linhd.uned.es/ontology/postdata-structuralElements#wordNumber> a owl:DatatypeProperty ;
    rdfs:label "wordNumber"@en ;
    rdfs:comment "Position of the word within the line to which it belongs"@en ;
    rdfs:domain <http://postdata.linhd.uned.es/ontology/postdata-structuralElements#Word> ;
    rdfs:isDefinedBy "http://postdata.linhd.uned.es/ontology/postdata-structuralElements"@en ;
    rdfs:range xsd:positiveInteger ;
    rdfs:subPropertyOf <http://purl.org/ontology/olo/core#index> .

dc:contributors a owl:AnnotationProperty .

dc:creator a owl:AnnotationProperty .

dc:date a owl:AnnotationProperty .

dc:description a owl:AnnotationProperty .

terms:abstract a owl:AnnotationProperty,
        owl:DatatypeProperty .

terms:publisher a owl:AnnotationProperty .

<http://purl.org/linguistics/gold/Syllable> a owl:Class .

vann:preferredNamespacePrefix a owl:AnnotationProperty .

<http://schema.org/image> a owl:AnnotationProperty .

<http://schema.org/url> a owl:DatatypeProperty .

owl:maxQualifiedCardinality a owl:AnnotationProperty .

ns1:license a owl:AnnotationProperty .

skos:definition a owl:AnnotationProperty .

skos:example a owl:AnnotationProperty .

skos:note a owl:AnnotationProperty .

<https://schema.org/latitude> a owl:DatatypeProperty ;
    rdfs:label "latitude"@en ;
    rdfs:comment "The latitude of a location. For example 37.42242 (WGS 84)."@en ;
    rdfs:domain <http://postdata.linhd.uned.es/ontology/postdata-core#Place> ;
    rdfs:range xsd:string .

<https://schema.org/longitude> a owl:DatatypeProperty ;
    rdfs:label "longitude"@en ;
    rdfs:comment "The longitude of a location. For example -122.08585 (WGS 84)."@en ;
    rdfs:domain <http://postdata.linhd.uned.es/ontology/postdata-core#Place> ;
    rdfs:range xsd:string .

<http://bakulf.github.io/raop/0.1#RethoricalDevice> a owl:Class .

<http://bakulf.github.io/raop/0.1#Word> a owl:Class .

<http://iflastandards.info/ns/fr/frbr/frbroo/F1> a owl:Class ;
    rdfs:label "Work"@en ;
    rdfs:comment "This class comprises the sums of concepts which appear in the course of the coherent evolution of an original idea into one or more expressions that are dominated by the original idea. The substance of Work is concepts. A Work may be elaborated by one or more Actors simultaneously or over time. A Work may have members that constitute components of the overall concept or that are alternatives to other members of the work. Members of a work may or may not represent the concept of the Work as a whole; for instance a translation reinterprets the whole, a volume of a trilogy represents a part of the concept. A Work can be either individual or complex. If it is individual its concept is completely realised in a single F22 Self-Contained Expression. If it is complex its concept is embedded in an F15 Complex Work. An F15 Complex Work consists of members that are either F15 Complex Works themselves or F14 Individual Works. The member relationship of Work is based on the members respecting the same concept, and should not be confused with the structural parts of an expression, that might be taken from other work(s). A Work is the product of an intellectual process of one or more persons, yet only indirect evidence about it is at our hands. This can be contextual information such as the existence of an order for a work, reflections of the creators themselves that are documented somewhere, and finally the expressions of the work created. As ideas normally take shape during discussion, elaboration and implementation, it is not reasonable to assume that a work starts with a complete concept. Moreover, it can be very difficult or impossible to define the whole of the concept of a work at some given time. The only objective evidence for such a notion can be based on a stage of expressions at a given time. In this sense, self-contained expressions serve as a kind of \"snap-shots\" of a work. A Work may aggregate expressions of other works into a new expression. For instance, an anthology of poems is regarded as a work in its own right that makes use of expressions of the individual poems that have been selected and ordered as part of an intellectual process. This does not make the contents of the aggregated expressions part of this work, but only parts of the resulting expression."@en ;
    rdfs:isDefinedBy <http://iflastandards.info/ns/fr/frbr/frbroo/> ;
    skos:definition "This class comprises the sums of concepts which appear in the course of the coherent evolution of an original idea into one or more expressions that are dominated by the original idea."@en .

<http://iflastandards.info/ns/fr/frbr/frbroo/F17> a owl:Class ;
    rdfs:label "Aggregation Work"@en ;
    rdfs:comment "This class comprises works whose essence is the selection and/or arrangement of expressions of one or more other works. This does not make the contents of the aggregated expressions part of this work, but only part of the resulting expression. F17 Aggregation Work may include additional original parts. An expression of a work may include expressions of other works within it. For instance, an anthology of poems is regarded as a work in its own right that makes use of expressions of the individual poems that have been selected and ordered as part of an intellectual process. A new version of an aggregate work does not make the resulting complex work an aggregate work as well. The inclusion of expressions from a complex work in an aggregation work does not make the aggregation work itself complex."@en ;
    rdfs:isDefinedBy <http://iflastandards.info/ns/fr/frbr/frbroo/> .

<http://iflastandards.info/ns/fr/frbr/frbroo/F22> a owl:Class ;
    rdfs:label "Self Contained Expression"@en ;
    rdfs:comment "This class comprises the immaterial realisations of individual works at a particular time that are regarded as a complete whole. The quality of wholeness reflects the intention of its creator that this expression should convey the concept of the work. Such a whole can in turn be part of a larger whole. Inherent to the notion of work is the completion of recognisable outcomes of the work. These outcomes, i.e. the Self-Contained Expressions, are regarded as the symbolic equivalents of Individual Works, which form the atoms of a complex work. A Self-Contained Expression may contain expressions or parts of expressions from other work, such as citations or items collected in anthologies. Even though they are incorporated in the Self-Contained Expression, they are not regarded as becoming members of the expressed container work by their inclusion in the expression, but are rather regarded as foreign or referred elements. F22 Self-Contained Expression can be distinguished from F23 Expression Fragment in that an F23 Expression Fragment was not intended by its creator to make sense by itself. Normally creators would characterise an outcome of a work as finished. In other cases, one could recognise an outcome of a work as complete from the elaboration or logical coherence of its content, or if there is any historical knowledge about the creator deliberately or accidentally never finishing (completing) that particular expression. In all those cases, one would regard an expression as self-contained."@en ;
    rdfs:isDefinedBy <http://iflastandards.info/ns/fr/frbr/frbroo/> ;
    skos:definition "This class comprises the immaterial realisations of individual works at a particular time that are regarded as a complete whole."@en .

<http://postdata.linhd.uned.es/kos/character-type> a owl:NamedIndividual,
        skos:ConceptScheme ;
    skos:definition "Thesaurus about character types"@en .

<http://postdata.linhd.uned.es/kos/foot-type> a owl:NamedIndividual,
        skos:ConceptScheme .

<http://postdata.linhd.uned.es/kos/footUnit-type> a owl:NamedIndividual,
        skos:ConceptScheme .

<http://postdata.linhd.uned.es/kos/metaplasm-type> a owl:NamedIndividual .

<http://postdata.linhd.uned.es/kos/metrical-category> a owl:NamedIndividual,
        skos:ConceptScheme .

<http://postdata.linhd.uned.es/kos/metrical-complexity> a owl:NamedIndividual,
        skos:ConceptScheme .

<http://postdata.linhd.uned.es/kos/metrical-context> a owl:NamedIndividual,
        skos:ConceptScheme .

<http://postdata.linhd.uned.es/kos/nucleus-type> a owl:NamedIndividual,
        skos:ConceptScheme .

<http://postdata.linhd.uned.es/kos/part-of-speech> a owl:NamedIndividual,
        skos:ConceptScheme .

<http://postdata.linhd.uned.es/kos/rhetorical-operation> a owl:NamedIndividual,
        skos:ConceptScheme .

<http://postdata.linhd.uned.es/kos/rhymeDisposition-type> a owl:NamedIndividual,
        skos:ConceptScheme .

<http://postdata.linhd.uned.es/kos/scheme-variety> a owl:NamedIndividual,
        skos:ConceptScheme .

<http://postdata.linhd.uned.es/kos/stanza-type> a owl:NamedIndividual,
        skos:ConceptScheme .

<http://postdata.linhd.uned.es/kos/stanzaEdition-type> a owl:NamedIndividual,
        skos:ConceptScheme .

<http://postdata.linhd.uned.es/kos/type-of-intertextuality> a owl:NamedIndividual,
        skos:ConceptScheme .

<http://postdata.linhd.uned.es/kos/versification-type> a owl:NamedIndividual,
        skos:ConceptScheme .

<http://postdata.linhd.uned.es/ontology/postdata-core#address> a owl:DatatypeProperty ;
    rdfs:label "address"@en ;
    rdfs:comment """Contains a postal address, for example of a publisher, an organisation, or an individual. There can only be one address per Organization.

Taking as example Cervantes' poem "Amadís de Gaula a Don Quijote de la Mancha", TEI-annotated in the ADSO corpus, the publisher would be "Natural Language Processing Group. Department of Software and Computing Systems. University of Alicante (Spain)", and its address would be "carretera San Vicente s/n 03690 San Vicente del Raspeig, Alicante (Spain)"."""@en ;
    rdfs:domain <http://postdata.linhd.uned.es/ontology/postdata-core#Organisation> ;
    rdfs:isDefinedBy "http://postdata.linhd.uned.es/ontology/postdata-core/" ;
    rdfs:range xsd:string .

<http://postdata.linhd.uned.es/ontology/postdata-core#audience> a owl:DatatypeProperty ;
    rdfs:label "audience"@en ;
    rdfs:comment """The meant readership, viewers or listeners of a cultural product (Redaction). There is at most one possible value for audience.

Taking as example the play "La segunda Celestina", "audience" would be the Spanish Queen and the people in the court attending the Queen's birthday celebrations."""@en ;
    rdfs:domain <http://postdata.linhd.uned.es/ontology/postdata-core#Redaction> ;
    rdfs:isDefinedBy "http://postdata.linhd.uned.es/ontology/postdata-core/" ;
    rdfs:range xsd:string .

<http://postdata.linhd.uned.es/ontology/postdata-core#authorEducationLevel> a owl:ObjectProperty ;
    rdfs:label "author Education Level"@en ;
    rdfs:comment "Level of education of the creator of a text/song. This property has as Domain PoeticWork and not Person since the education level of a person changes during time. That is, this is the education level of the author in the moment of writing the poem."@en ;
    rdfs:domain <http://postdata.linhd.uned.es/ontology/postdata-core#PoeticWork> ;
    rdfs:isDefinedBy "http://postdata.linhd.uned.es/ontology/postdata-core/" ;
    rdfs:range [ a owl:Restriction ;
            owl:hasValue <http://postdata.linhd.uned.es/kos/author-education-level> ;
            owl:onProperty skos:inScheme ],
        skos:Concept .

<http://postdata.linhd.uned.es/ontology/postdata-core#birthDate> a owl:ObjectProperty ;
    rdfs:label "birthDate"@en ;
    rdfs:comment "Date of birth"@en ;
    rdfs:domain <http://postdata.linhd.uned.es/ontology/postdata-core#Person> ;
    rdfs:isDefinedBy "http://postdata.linhd.uned.es/ontology/postdata-core/" ;
    rdfs:range <http://postdata.linhd.uned.es/ontology/postdata-dates#DateEntity> ;
    rdfs:subPropertyOf owl:topObjectProperty .

<http://postdata.linhd.uned.es/ontology/postdata-core#birthPlace> a owl:ObjectProperty ;
    rdfs:label "birth Place"@en ;
    rdfs:comment "This property points to the Place which is the provenance of the current instance of Person"@en ;
    rdfs:domain <http://postdata.linhd.uned.es/ontology/postdata-core#Person> ;
    rdfs:isDefinedBy "http://postdata.linhd.uned.es/ontology/postdata-core/" ;
    rdfs:range <http://postdata.linhd.uned.es/ontology/postdata-core#Place> ;
    rdfs:subPropertyOf <http://postdata.linhd.uned.es/ontology/postdata-core#isFrom> ;
    owl:inverseOf <http://postdata.linhd.uned.es/ontology/postdata-core#birthPlaceOf> .

<http://postdata.linhd.uned.es/ontology/postdata-core#birthPlaceOf> a owl:ObjectProperty ;
    rdfs:label "birth Place Of"@en ;
    rdfs:comment "This property points to a Person who was born in the Place"@en ;
    rdfs:domain <http://postdata.linhd.uned.es/ontology/postdata-core#Place> ;
    rdfs:isDefinedBy "http://postdata.linhd.uned.es/ontology/postdata-core/" ;
    rdfs:range <http://postdata.linhd.uned.es/ontology/postdata-core#Person> .

<http://postdata.linhd.uned.es/ontology/postdata-core#deathDate> a owl:ObjectProperty ;
    rdfs:label "deathDate"@en ;
    rdfs:comment "Date of death"@en ;
    rdfs:domain <http://postdata.linhd.uned.es/ontology/postdata-core#Person> ;
    rdfs:isDefinedBy "http://postdata.linhd.uned.es/ontology/postdata-core/" ;
    rdfs:range <http://postdata.linhd.uned.es/ontology/postdata-dates#DateEntity> ;
    rdfs:subPropertyOf owl:topObjectProperty .

<http://postdata.linhd.uned.es/ontology/postdata-core#deathPlaceOf> a owl:ObjectProperty ;
    rdfs:label "death Place Of"@en ;
    rdfs:comment "This property points to a Person who died in the current instance of Place"@en ;
    rdfs:domain <http://postdata.linhd.uned.es/ontology/postdata-core#Place> ;
    rdfs:isDefinedBy "http://postdata.linhd.uned.es/ontology/postdata-core/" ;
    rdfs:range <http://postdata.linhd.uned.es/ontology/postdata-core#Person> .

<http://postdata.linhd.uned.es/ontology/postdata-core#editedIn> a owl:ObjectProperty ;
    rdfs:label "edited In"@en ;
    rdfs:comment "This property points to the specific Location in a bibliographic item that contains an edition of the current instance of Redaction."@en ;
    rdfs:domain <http://postdata.linhd.uned.es/ontology/postdata-core#Redaction> ;
    rdfs:isDefinedBy "http://postdata.linhd.uned.es/ontology/postdata-core/" ;
    rdfs:range <http://postdata.linhd.uned.es/ontology/postdata-transmission#Location> .

<http://postdata.linhd.uned.es/ontology/postdata-core#eventNarration> a owl:DatatypeProperty ;
    rdfs:label "event Narration"@en ;
    rdfs:comment """Text that narrates an Event, that is, an excerpt of the Redaction. There is at most one possible description for this property.

Taking as Opus example the "Poema de Mio Cid", and as Event example the Cid's arrival to Burgos, we find an "eventNarration" in  lines 1-64, starting with "De los sos ojos tan fuertemientre llorando"."""@en ;
    rdfs:domain <http://postdata.linhd.uned.es/ontology/postdata-core#Event> ;
    rdfs:isDefinedBy "http://postdata.linhd.uned.es/ontology/postdata-core/" ;
    rdfs:range xsd:string .

<http://postdata.linhd.uned.es/ontology/postdata-core#explicit> a owl:DatatypeProperty ;
    rdfs:label "explicit"@en ;
    rdfs:comment """The closing words of the composition (usually, the last verse). There is only one explicit per Redaction.

Taking as example the poem "Canary" by Rita Dove, the last verse, "If you can't be free, be a mystery", would be the "explicit"."""@en ;
    rdfs:domain <http://postdata.linhd.uned.es/ontology/postdata-core#Redaction> ;
    rdfs:isDefinedBy "http://postdata.linhd.uned.es/ontology/postdata-core/" ;
    rdfs:range xsd:string .

<http://postdata.linhd.uned.es/ontology/postdata-core#floruit> a owl:ObjectProperty ;
    rdfs:label "floruit"@en ;
    rdfs:comment "The period of activity of a person, used when a range cannot be established (e.g. “3rd century”)"@en ;
    rdfs:domain <http://postdata.linhd.uned.es/ontology/postdata-core#Person> ;
    rdfs:isDefinedBy "http://postdata.linhd.uned.es/ontology/postdata-core/" ;
    rdfs:range <http://postdata.linhd.uned.es/ontology/postdata-dates#DateEntity> .

<http://postdata.linhd.uned.es/ontology/postdata-core#forename> a owl:DatatypeProperty ;
    rdfs:label "forename"@en ;
    rdfs:comment """It contains a forename, given or baptismal name.

Taking as example the poet "Antonio Machado", his "forename" would be "Antonio"."""@en ;
    rdfs:domain <http://postdata.linhd.uned.es/ontology/postdata-core#Person> ;
    rdfs:isDefinedBy "http://postdata.linhd.uned.es/ontology/postdata-core/" ;
    rdfs:range xsd:string .

<http://postdata.linhd.uned.es/ontology/postdata-core#gender> a owl:ObjectProperty ;
    rdfs:label "gender"@en ;
    rdfs:comment "The gender of a Person"@en ;
    rdfs:domain <http://postdata.linhd.uned.es/ontology/postdata-core#Person> ;
    rdfs:isDefinedBy "http://postdata.linhd.uned.es/ontology/postdata-core/" ;
    rdfs:range [ a owl:Restriction ;
            owl:hasValue <http://postdata.linhd.uned.es/kos/gender> ;
            owl:onProperty skos:inScheme ],
        skos:Concept .

<http://postdata.linhd.uned.es/ontology/postdata-core#hasCharacter> a owl:ObjectProperty ;
    rdfs:label "has Character"@en ;
    rdfs:comment "This property points to a character depicted in the text of a Redaction, if any. The character is an instance of Agent (Organisation or Person)."@en ;
    rdfs:domain <http://postdata.linhd.uned.es/ontology/postdata-core#Redaction> ;
    rdfs:isDefinedBy "http://postdata.linhd.uned.es/ontology/postdata-core/" ;
    rdfs:range <http://postdata.linhd.uned.es/ontology/postdata-core#Agent> .

<http://postdata.linhd.uned.es/ontology/postdata-core#hasDedication> a owl:ObjectProperty ;
    rdfs:label "has Dedication"@en ;
    rdfs:comment "This property points to the text (an instance of Redaction) which was dedicated to the current Person."@en ;
    rdfs:domain <http://postdata.linhd.uned.es/ontology/postdata-core#Person> ;
    rdfs:isDefinedBy "http://postdata.linhd.uned.es/ontology/postdata-core/" ;
    rdfs:range <http://postdata.linhd.uned.es/ontology/postdata-core#Redaction> .

<http://postdata.linhd.uned.es/ontology/postdata-core#hasFirstPart> a owl:ObjectProperty ;
    rdfs:label "has First Part"@en ;
    rdfs:comment "This property points to the first text unit  which form the current element under analysis"@en ;
    rdfs:domain <http://postdata.linhd.uned.es/ontology/postdata-core#OrderedTextUnitList> ;
    rdfs:isDefinedBy "http://postdata.linhd.uned.es/ontology/postdata-core/" ;
    rdfs:range <http://postdata.linhd.uned.es/ontology/postdata-core#TextUnit> ;
    rdfs:subPropertyOf <http://www.ontologydesignpatterns.org/cp/owl/partof.owl#hasPart> .

<http://postdata.linhd.uned.es/ontology/postdata-core#hasOrderedTextUnitList> a owl:ObjectProperty ;
    rdfs:label "has Ordered Text Unit List"@en ;
    rdfs:comment "List of text units that form the Redaction"@en ;
    rdfs:domain <http://postdata.linhd.uned.es/ontology/postdata-core#Redaction> ;
    rdfs:isDefinedBy "http://postdata.linhd.uned.es/ontology/postdata-core/" ;
    rdfs:range <http://postdata.linhd.uned.es/ontology/postdata-core#OrderedTextUnitList> .

<http://postdata.linhd.uned.es/ontology/postdata-core#hasSynthesis> a owl:ObjectProperty ;
    rdfs:comment "This property points to one of the texts (an instance of Redaction) which is an analytical version of the text at hand (the current Redaction)"@en,
        "has Synthesis"@en ;
    rdfs:domain <http://postdata.linhd.uned.es/ontology/postdata-core#Redaction> ;
    rdfs:isDefinedBy "http://postdata.linhd.uned.es/ontology/postdata-core/" ;
    rdfs:range <http://postdata.linhd.uned.es/ontology/postdata-core#Redaction> ;
    owl:inverseOf <http://postdata.linhd.uned.es/ontology/postdata-core#isSynthesisOf> .

<http://postdata.linhd.uned.es/ontology/postdata-core#incipit> a owl:DatatypeProperty ;
    rdfs:label "incipit"@en ;
    rdfs:comment """The first line of the work. There is one incipit for each Redaction.

Taking as example the "Soledades" by Góngora, the "incipit" is "Pasos de un peregrino son errante"."""@en ;
    rdfs:domain <http://postdata.linhd.uned.es/ontology/postdata-core#Redaction> ;
    rdfs:isDefinedBy "http://postdata.linhd.uned.es/ontology/postdata-core/" ;
    rdfs:range xsd:string .

<http://postdata.linhd.uned.es/ontology/postdata-core#isIndexedIn> a owl:ObjectProperty ;
    rdfs:label "is Indexed In"@en ;
    rdfs:comment "This property points to the specific location in the text of the bibliographic item (an instance of Location) in which the current text (Redaction) is indexed."@en ;
    rdfs:domain <http://postdata.linhd.uned.es/ontology/postdata-core#Redaction> ;
    rdfs:isDefinedBy "http://postdata.linhd.uned.es/ontology/postdata-core/" ;
    rdfs:range <http://postdata.linhd.uned.es/ontology/postdata-transmission#Location> .

<http://postdata.linhd.uned.es/ontology/postdata-core#isMemberOf> a owl:ObjectProperty ;
    rdfs:label "is Member Of"@en ;
    rdfs:comment "This property points to the instance of Organisation to which the Person at hand belongs"@en ;
    rdfs:domain <http://postdata.linhd.uned.es/ontology/postdata-core#Person> ;
    rdfs:isDefinedBy "http://postdata.linhd.uned.es/ontology/postdata-core/" ;
    rdfs:range <http://postdata.linhd.uned.es/ontology/postdata-core#Organisation> .

<http://postdata.linhd.uned.es/ontology/postdata-core#isProvenanceFor> a owl:ObjectProperty ;
    rdfs:label "is Provenance For"@en ;
    rdfs:comment "This property points to the Entity whose provenance corresponds to the current instance of Place"@en ;
    rdfs:domain <http://postdata.linhd.uned.es/ontology/postdata-core#Place> ;
    rdfs:isDefinedBy "http://postdata.linhd.uned.es/ontology/postdata-core/" ;
    rdfs:range [ a owl:Class ;
            owl:unionOf ( <http://postdata.linhd.uned.es/ontology/postdata-core#Ensemble> <http://postdata.linhd.uned.es/ontology/postdata-core#PoeticWork> ) ] .

<http://postdata.linhd.uned.es/ontology/postdata-core#literaryPeriod> a owl:ObjectProperty ;
    rdfs:label "literary Period"@en ;
    rdfs:comment """Label of a time frame for grouping certain works. Cf. "school".
The values of this property are defined in a controlled vocabulary about literary periods."""@en ;
    rdfs:domain <http://postdata.linhd.uned.es/ontology/postdata-core#Person> ;
    rdfs:isDefinedBy "http://postdata.linhd.uned.es/ontology/postdata-core/" ;
    rdfs:range [ a owl:Restriction ;
            owl:hasValue <http://postdata.linhd.uned.es/kos/literary-period> ;
            owl:onProperty skos:inScheme ],
        skos:Concept .

<http://postdata.linhd.uned.es/ontology/postdata-core#mentions> a owl:ObjectProperty ;
    rdfs:label "mentions"@en ;
    rdfs:comment "This property points to an instance of Event  or Person or Organisation or Place that is referred in a given Redaction"@en ;
    rdfs:domain <http://postdata.linhd.uned.es/ontology/postdata-core#Redaction> ;
    rdfs:isDefinedBy "http://postdata.linhd.uned.es/ontology/postdata-core/" ;
    rdfs:range [ a owl:Class ;
            owl:unionOf ( <http://postdata.linhd.uned.es/ontology/postdata-core#Place> <http://www.europeana.eu/schemas/edm/Event> <http://xmlns.com/foaf/0.1/Organization> <http://xmlns.com/foaf/0.1/Person> ) ] .

<http://postdata.linhd.uned.es/ontology/postdata-core#nameLink> a owl:DatatypeProperty ;
    rdfs:label "name Link"@en ;
    rdfs:comment """A connecting phrase or link used within a name but not regarded as part of it.

Taking as example the writer “Hildegard von Bingen”, her “nameLink” would be “von”."""@en ;
    rdfs:domain <http://postdata.linhd.uned.es/ontology/postdata-core#Person> ;
    rdfs:isDefinedBy "http://postdata.linhd.uned.es/ontology/postdata-core/" ;
    rdfs:range xsd:string ;
    rdfs:subPropertyOf owl:topDataProperty .

<http://postdata.linhd.uned.es/ontology/postdata-core#notes> a owl:DatatypeProperty ;
    rdfs:label "notes"@en ;
    rdfs:comment "Comment or explanations"@en ;
    rdfs:isDefinedBy "http://postdata.linhd.uned.es/ontology/postdata-core"@en ;
    rdfs:range xsd:string .

<http://postdata.linhd.uned.es/ontology/postdata-core#numberOfLines> a owl:DatatypeProperty ;
    rdfs:label "number of Lines"@en ;
    rdfs:comment "Number of total lines comprising the Ensemble"@en ;
    rdfs:domain <http://postdata.linhd.uned.es/ontology/postdata-core#Ensemble> ;
    rdfs:isDefinedBy "http://postdata.linhd.uned.es/ontology/postdata-core/" ;
    rdfs:range xsd:integer .

<http://postdata.linhd.uned.es/ontology/postdata-core#numberOfPlays> a owl:DatatypeProperty ;
    rdfs:label "number of Plays"@en ;
    rdfs:comment "Number of plays of an Ensemble"@en ;
    rdfs:domain <http://postdata.linhd.uned.es/ontology/postdata-core#Ensemble> ;
    rdfs:isDefinedBy "http://postdata.linhd.uned.es/ontology/postdata-core/" ;
    rdfs:range xsd:integer .

<http://postdata.linhd.uned.es/ontology/postdata-core#numberOfPoems> a owl:DatatypeProperty ;
    rdfs:label "number of poems"@en ;
    rdfs:comment "Number of poems of an Ensemble"@en ;
    rdfs:domain <http://postdata.linhd.uned.es/ontology/postdata-core#Ensemble> ;
    rdfs:isDefinedBy "http://postdata.linhd.uned.es/ontology/postdata-core/" ;
    rdfs:range xsd:integer .

<http://postdata.linhd.uned.es/ontology/postdata-core#numberOfWitnessesUsed> a owl:DatatypeProperty ;
    rdfs:label "number of Witnesses Used"@en ;
    rdfs:comment "Number of Primary Sources used in the elaboration of an edition (Redaction)"@en ;
    rdfs:domain <http://postdata.linhd.uned.es/ontology/postdata-core#Redaction> ;
    rdfs:isDefinedBy "http://postdata.linhd.uned.es/ontology/postdata-core/" ;
    rdfs:range xsd:integer .

<http://postdata.linhd.uned.es/ontology/postdata-core#originalLanguage> a owl:DatatypeProperty ;
    rdfs:label "original Language"@en ;
    rdfs:comment "The language from which the Redaction is a translation"@en ;
    rdfs:domain <http://postdata.linhd.uned.es/ontology/postdata-core#Redaction> ;
    rdfs:isDefinedBy "http://postdata.linhd.uned.es/ontology/postdata-core/" ;
    rdfs:range [ a rdfs:Datatype ;
            owl:unionOf ( xsd:language xsd:string ) ] .

<http://postdata.linhd.uned.es/ontology/postdata-core#paraphrasis> a owl:DatatypeProperty ;
    rdfs:label "paraphrasis"@en ;
    rdfs:comment "The recasting of the contents in words different from that originally used, whether in the same language or in a translation. A Redaction may have zero or one paraphrasis associated."@en ;
    rdfs:domain <http://postdata.linhd.uned.es/ontology/postdata-core#Redaction> ;
    rdfs:isDefinedBy "http://postdata.linhd.uned.es/ontology/postdata-core/" ;
    rdfs:range xsd:string .

<http://postdata.linhd.uned.es/ontology/postdata-core#penName> a owl:DatatypeProperty ;
    rdfs:label "pen Name"@en ;
    rdfs:comment "A fictitious name, especially a pen name. A variant name"@en ;
    rdfs:domain <http://postdata.linhd.uned.es/ontology/postdata-core#CreatorRole> ;
    rdfs:isDefinedBy "http://postdata.linhd.uned.es/ontology/postdata-core/" ;
    rdfs:range xsd:string .

<http://postdata.linhd.uned.es/ontology/postdata-core#poeticType> a owl:ObjectProperty ;
    rdfs:label "poetic Type"@en ;
    rdfs:comment "Major literary genre of a Poetic Work, that is, drama or poetry. The values of this property are defined in a controlled vocabulary about poetic types"@en ;
    rdfs:domain <http://postdata.linhd.uned.es/ontology/postdata-core#PoeticWork> ;
    rdfs:isDefinedBy "http://postdata.linhd.uned.es/ontology/postdata-core/" ;
    rdfs:range [ a owl:Restriction ;
            owl:hasValue <http://postdata.linhd.uned.es/kos/poetic-type> ;
            owl:onProperty skos:inScheme ],
        skos:Concept .

<http://postdata.linhd.uned.es/ontology/postdata-core#religiousAffiliation> a owl:ObjectProperty ;
    rdfs:label "religious Affiliation"@en ;
    rdfs:comment "Association of a person with a religion, denomination or sub–denominational religious group. The values of this property are defined in a controlled vocabulary about religious affiliation"@en ;
    rdfs:domain <http://postdata.linhd.uned.es/ontology/postdata-core#Person> ;
    rdfs:isDefinedBy "http://postdata.linhd.uned.es/ontology/postdata-core/" ;
    rdfs:range [ a owl:Restriction ;
            owl:hasValue <http://postdata.linhd.uned.es/kos/religious-affiliation> ;
            owl:onProperty skos:inScheme ],
        skos:Concept .

<http://postdata.linhd.uned.es/ontology/postdata-core#retrievesText> a owl:ObjectProperty ;
    rdfs:label "retrieves Text"@en ;
    rdfs:comment "This property points to the specific location in a bibliographic item (an instance of Location) which contains the edition used as the base of text at hand"@en ;
    rdfs:domain <http://postdata.linhd.uned.es/ontology/postdata-core#Redaction> ;
    rdfs:isDefinedBy "http://postdata.linhd.uned.es/ontology/postdata-core/" ;
    rdfs:range <http://postdata.linhd.uned.es/ontology/postdata-transmission#Location> .

<http://postdata.linhd.uned.es/ontology/postdata-core#roleFunction> a owl:ObjectProperty ;
    rdfs:label "role Function"@en ;
    rdfs:comment "Specific function performed by some agent on a work (e.g. sponsor, actor, collector, singer, arranger, transcriptor). This is connected to the Role class."@en ;
    rdfs:domain <http://postdata.linhd.uned.es/ontology/postdata-core#Role> ;
    rdfs:isDefinedBy "http://postdata.linhd.uned.es/ontology/postdata-core/" ;
    rdfs:range [ a owl:Restriction ;
            owl:hasValue <http://postdata.linhd.uned.es/kos/role-function> ;
            owl:onProperty skos:inScheme ],
        skos:Concept .

<http://postdata.linhd.uned.es/ontology/postdata-core#school> a owl:ObjectProperty ;
    rdfs:label "school"@en ;
    rdfs:comment "Literary movement/school of a Person"@en ;
    rdfs:domain <http://postdata.linhd.uned.es/ontology/postdata-core#Person> ;
    rdfs:isDefinedBy "http://postdata.linhd.uned.es/ontology/postdata-core/" ;
    rdfs:range [ a owl:Restriction ;
            owl:hasValue <http://postdata.linhd.uned.es/kos/school> ;
            owl:onProperty skos:inScheme ],
        skos:Concept .

<http://postdata.linhd.uned.es/ontology/postdata-core#socialStatus> a owl:ObjectProperty ;
    rdfs:label "social Status"@en ;
    rdfs:comment "The social status of the Person, that is the position or rank of a Person within the society. The values are specified in a controlled vocabulary"@en ;
    rdfs:domain <http://postdata.linhd.uned.es/ontology/postdata-core#Person> ;
    rdfs:isDefinedBy "http://postdata.linhd.uned.es/ontology/postdata-core/" ;
    rdfs:range [ a owl:Restriction ;
            owl:hasValue <http://postdata.linhd.uned.es/kos/social-status> ;
            owl:onProperty skos:inScheme ],
        skos:Concept .

<http://postdata.linhd.uned.es/ontology/postdata-core#sourceNote> a owl:DatatypeProperty ;
    rdfs:label "source Note"@en ;
    rdfs:comment "Note about the source used to give a particular piece of information"@en ;
    rdfs:domain <http://postdata.linhd.uned.es/ontology/postdata-core#Person> ;
    rdfs:isDefinedBy "http://postdata.linhd.uned.es/ontology/postdata-core/" ;
    rdfs:range xsd:string ;
    rdfs:subPropertyOf <http://purl.org/net/nknouf/ns/bibtex#hasNote> .

<http://postdata.linhd.uned.es/ontology/postdata-core#surname> a owl:DatatypeProperty ;
    rdfs:label "surname"@en ;
    rdfs:comment "Contains a family (inherited) name, as opposed to a given, baptismal, or nick name"@en ;
    rdfs:domain <http://postdata.linhd.uned.es/ontology/postdata-core#Person> ;
    rdfs:isDefinedBy "http://postdata.linhd.uned.es/ontology/postdata-core/" ;
    rdfs:range xsd:string .

<http://postdata.linhd.uned.es/ontology/postdata-core#text> a owl:DatatypeProperty ;
    rdfs:label "text"@en ;
    rdfs:comment "Reference to textual contents . The contents of this property do not allow finer analysis by stanza or line. It can be a text of a diplomatic edition, semidiplomatic edition or of a critical edition (among others) or even a translation. The property typeOfRedaction defines the type of Edition or if it is a translation. There is only one possible text for each Redaction."@en ;
    rdfs:domain <http://postdata.linhd.uned.es/ontology/postdata-core#Redaction> ;
    rdfs:isDefinedBy "http://postdata.linhd.uned.es/ontology/postdata-core/" ;
    rdfs:range xsd:string .

<http://postdata.linhd.uned.es/ontology/postdata-core#typeOfDesignation> a owl:ObjectProperty ;
    rdfs:label "type Of Designation"@en ;
    rdfs:comment "Type of designation/name. E.g. pseudonym, heteronym, allonym, orthonym variant"@en ;
    rdfs:domain <http://postdata.linhd.uned.es/ontology/postdata-core#CreatorRole> ;
    rdfs:isDefinedBy "http://postdata.linhd.uned.es/ontology/postdata-core/" ;
    rdfs:range [ a owl:Restriction ;
            owl:hasValue <http://postdata.linhd.uned.es/kos/designation-type> ;
            owl:onProperty skos:inScheme ],
        skos:Concept .

<http://postdata.linhd.uned.es/ontology/postdata-core#typeOfTextualElement> a owl:ObjectProperty ;
    rdfs:label "type Of Textual Element"@en ;
    rdfs:comment "The type of textual element (e.g. part of a greater ensemble; part of a composed collection of poems; prologue of a work; epilogue of a work; a chapter of a work...)"@en ;
    rdfs:domain <http://postdata.linhd.uned.es/ontology/postdata-core#Redaction> ;
    rdfs:isDefinedBy "http://postdata.linhd.uned.es/ontology/postdata-core/" ;
    rdfs:range [ a owl:Restriction ;
            owl:hasValue <http://postdata.linhd.uned.es/kos/textual-element-type> ;
            owl:onProperty skos:inScheme ],
        skos:Concept .

<http://postdata.linhd.uned.es/ontology/postdata-core#unusedWitnesses> a owl:DatatypeProperty ;
    rdfs:label "unused Witnesses"@en ;
    rdfs:comment "Primary sources of the text excluded during the elaboration of a Redaction (usually, dependent witnesses)"@en ;
    rdfs:domain <http://postdata.linhd.uned.es/ontology/postdata-core#Redaction> ;
    rdfs:isDefinedBy "http://postdata.linhd.uned.es/ontology/postdata-core/" ;
    rdfs:range xsd:string .

<http://postdata.linhd.uned.es/ontology/postdata-core#workNumber> a owl:DatatypeProperty ;
    rdfs:label "work Number"@en ;
    rdfs:comment "Number that identifies the Redaction inside a collection. There can only be one value associated for each Redaction."@en ;
    rdfs:domain <http://postdata.linhd.uned.es/ontology/postdata-core#Redaction> ;
    rdfs:isDefinedBy "http://postdata.linhd.uned.es/ontology/postdata-core/" ;
    rdfs:range xsd:string .

<http://postdata.linhd.uned.es/ontology/postdata-literaryAnalysisElements#Scheme> a owl:Class ;
    rdfs:label "Scheme"@en ;
    rdfs:comment "Change in the usual order of words"@en ;
    rdfs:isDefinedBy "http://postdata.linhd.uned.es/ontology/postdata-literaryAnalysisElements/"@en ;
    rdfs:subClassOf [ a owl:Restriction ;
            owl:onDataRange xsd:string ;
            owl:onProperty <http://postdata.linhd.uned.es/ontology/postdata-literaryAnalysisElements#content> ;
            owl:qualifiedCardinality "1"^^xsd:nonNegativeInteger ],
        <http://postdata.linhd.uned.es/ontology/postdata-literaryAnalysisElements#FigureOfSpeech> .

<http://postdata.linhd.uned.es/ontology/postdata-literaryAnalysisElements#Trope> a owl:Class ;
    rdfs:label "Trope"@en ;
    rdfs:comment "The use of a word or  a phrase with a meaning that is not the usual one"@en ;
    rdfs:isDefinedBy "http://postdata.linhd.uned.es/ontology/postdata-literaryAnalysisElements/"@en ;
    rdfs:subClassOf [ a owl:Restriction ;
            owl:onDataRange xsd:string ;
            owl:onProperty <http://postdata.linhd.uned.es/ontology/postdata-literaryAnalysisElements#content> ;
            owl:qualifiedCardinality "1"^^xsd:nonNegativeInteger ],
        <http://postdata.linhd.uned.es/ontology/postdata-literaryAnalysisElements#FigureOfSpeech> .

<http://postdata.linhd.uned.es/ontology/postdata-literaryAnalysisElements#figureMeaning> a owl:DatatypeProperty ;
    rdfs:label "figureMeaning"@en ;
    dc:creator "mluisadiez" ;
    dc:date "2018-06-16T18:39:21+00:00"^^xsd:dateTime ;
    rdfs:comment "Meaning of the figure"@en ;
    rdfs:domain <http://postdata.linhd.uned.es/ontology/postdata-literaryAnalysisElements#FigureOfSpeech> ;
    rdfs:isDefinedBy "http://postdata.linhd.uned.es/ontology/postdata-literaryAnalysisElements/"@en ;
    rdfs:range xsd:string ;
    rdfs:subPropertyOf owl:topDataProperty .

<http://postdata.linhd.uned.es/ontology/postdata-literaryAnalysisElements#figureReferent> a owl:DatatypeProperty ;
    rdfs:label "figureReferent"@en ;
    dc:creator "mluisadiez" ;
    dc:date "2018-06-16T18:39:21+00:00"^^xsd:dateTime ;
    rdfs:comment "Unspoken name which is equivalent to the figure"@en ;
    rdfs:domain <http://postdata.linhd.uned.es/ontology/postdata-literaryAnalysisElements#FigureOfSpeech> ;
    rdfs:isDefinedBy "http://postdata.linhd.uned.es/ontology/postdata-literaryAnalysisElements/"@en ;
    rdfs:range xsd:string ;
    rdfs:subPropertyOf owl:topDataProperty .

<http://postdata.linhd.uned.es/ontology/postdata-literaryAnalysisElements#isContainedIn> a owl:ObjectProperty ;
    rdfs:label "isContainedIn"@en ;
    rdfs:comment "This property points to the Redaction (version of the Opus) in which the Acrostic is present"@en ;
    rdfs:domain <http://postdata.linhd.uned.es/ontology/postdata-literaryAnalysisElements#Acrostic> ;
    rdfs:isDefinedBy "http://postdata.linhd.uned.es/ontology/postdata-literaryAnalysisElements/"@en ;
    rdfs:range <http://postdata.linhd.uned.es/ontology/postdata-core#Redaction> .

<http://postdata.linhd.uned.es/ontology/postdata-literaryAnalysisElements#isDerivedFrom> a owl:ObjectProperty ;
    rdfs:label "isDerivedFrom"@en ;
    rdfs:comment "This property points to the text under analysis (Redaction) which has been a source for the current cultural product"@en ;
    rdfs:domain <http://postdata.linhd.uned.es/ontology/postdata-literaryAnalysisElements#Intertextuality> ;
    rdfs:isDefinedBy "http://postdata.linhd.uned.es/ontology/postdata-literaryAnalysisElements/"@en ;
    rdfs:range <http://postdata.linhd.uned.es/ontology/postdata-core#Redaction> .

<http://postdata.linhd.uned.es/ontology/postdata-literaryAnalysisElements#isRelatedContemporaneouslyWith> a owl:ObjectProperty ;
    rdfs:label "isRelatedContemporaneouslyWith"@en ;
    rdfs:comment "This property points to a cultural product (Intertextuality) which is contemporary to the work under analysis and some kind of intertextual relationship is detected"@en ;
    rdfs:domain <http://postdata.linhd.uned.es/ontology/postdata-core#Redaction> ;
    rdfs:isDefinedBy "http://postdata.linhd.uned.es/ontology/postdata-literaryAnalysisElements/"@en ;
    rdfs:range <http://postdata.linhd.uned.es/ontology/postdata-literaryAnalysisElements#Intertextuality> .

<http://postdata.linhd.uned.es/ontology/postdata-literaryAnalysisElements#isRelatedWith> a owl:ObjectProperty ;
    rdfs:label "isRelatedWith"@en ;
    rdfs:comment "This property points to a cultural product (Intertextuality) which has a generic intertextual relationship with the work under analysis"@en ;
    rdfs:domain <http://postdata.linhd.uned.es/ontology/postdata-literaryAnalysisElements#Intertextuality> ;
    rdfs:isDefinedBy "http://postdata.linhd.uned.es/ontology/postdata-literaryAnalysisElements/"@en ;
    rdfs:range <http://postdata.linhd.uned.es/ontology/postdata-core#Redaction> .

<http://postdata.linhd.uned.es/ontology/postdata-literaryAnalysisElements#isSmallerUnitOf> a owl:ObjectProperty ;
    rdfs:label "isSmallerUnit"@en ;
    rdfs:comment "The current instance of Figure of Speech is a smaller unit of another instance of Figure Of Speech"@en ;
    rdfs:domain <http://postdata.linhd.uned.es/ontology/postdata-literaryAnalysisElements#FigureOfSpeech> ;
    rdfs:isDefinedBy "http://postdata.linhd.uned.es/ontology/postdata-literaryAnalysisElements/"@en ;
    rdfs:range <http://postdata.linhd.uned.es/ontology/postdata-literaryAnalysisElements#FigureOfSpeech> .

<http://postdata.linhd.uned.es/ontology/postdata-literaryAnalysisElements#reference> a owl:DatatypeProperty ;
    rdfs:label "reference"@en ;
    rdfs:comment "A non-structured mention of the textual source with which there is intertextual relationships"@en ;
    rdfs:domain <http://postdata.linhd.uned.es/ontology/postdata-literaryAnalysisElements#Intertextuality> ;
    rdfs:isDefinedBy "http://postdata.linhd.uned.es/ontology/postdata-literaryAnalysisElements/"@en ;
    rdfs:range xsd:string ;
    owl:equivalentProperty terms:bibliographicCitation .

<http://postdata.linhd.uned.es/ontology/postdata-literaryAnalysisElements#referenceLocation> a owl:DatatypeProperty ;
    rdfs:label "referenceLocation"@en ;
    rdfs:comment "The location of the relevant piece of information in that particular textual source with which there is intertextual relationships"@en ;
    rdfs:domain <http://postdata.linhd.uned.es/ontology/postdata-literaryAnalysisElements#Intertextuality> ;
    rdfs:isDefinedBy "http://postdata.linhd.uned.es/ontology/postdata-literaryAnalysisElements/"@en ;
    rdfs:range xsd:string .

<http://postdata.linhd.uned.es/ontology/postdata-literaryAnalysisElements#refersTo> a owl:ObjectProperty ;
    rdfs:label "refersTo"@en ;
    rdfs:comment "This property points to a Person or Place that is referred in the Acrostic"@en ;
    rdfs:domain <http://postdata.linhd.uned.es/ontology/postdata-literaryAnalysisElements#Acrostic> ;
    rdfs:isDefinedBy "http://postdata.linhd.uned.es/ontology/postdata-literaryAnalysisElements/"@en .

<http://postdata.linhd.uned.es/ontology/postdata-literaryAnalysisElements#usesAsSource> a owl:ObjectProperty ;
    rdfs:label "usesAsSource"@en ;
    rdfs:comment "This property points to a cultural product (Intertextuality) which was a source for the work under analysis"@en ;
    rdfs:domain <http://postdata.linhd.uned.es/ontology/postdata-core#Redaction> ;
    rdfs:isDefinedBy "http://postdata.linhd.uned.es/ontology/postdata-literaryAnalysisElements/"@en ;
    rdfs:range <http://postdata.linhd.uned.es/ontology/postdata-literaryAnalysisElements#Intertextuality> .

<http://postdata.linhd.uned.es/ontology/postdata-prosodicElements#MetricalSyllable> a owl:Class ;
    rdfs:label "MetricalSyllable"@en ;
    rdfs:comment "Metric syllable built by applying metaplasms to syllables."@en ;
    rdfs:isDefinedBy "http://postdata.linhd.uned.es/ontology/postdata-prosodicElements"@en .

<http://postdata.linhd.uned.es/ontology/postdata-prosodicElements#accentedVowels> a owl:DatatypeProperty ;
    rdfs:label "accentedVowels"@en ;
    dc:creator "mluisadiez" ;
    rdfs:comment "Stressed vowels in the order in which they occur in the text"@en ;
    rdfs:domain <http://postdata.linhd.uned.es/ontology/postdata-prosodicElements#LinePattern> ;
    rdfs:isDefinedBy "http://postdata.linhd.uned.es/ontology/postdata-prosodicElements"@en ;
    rdfs:range xsd:string ;
    rdfs:subPropertyOf owl:topDataProperty .

<http://postdata.linhd.uned.es/ontology/postdata-prosodicElements#accentedVowelsPattern> a owl:DatatypeProperty ;
    rdfs:label "accentedVowelsPattern"@en ;
    dc:creator "mluisadiez" ;
    rdfs:comment "Stressed vowels in a line, in alphabetical order to show sound repetitions"@en ;
    rdfs:domain [ a owl:Restriction ;
            owl:maxQualifiedCardinality "1"^^xsd:nonNegativeInteger ;
            owl:onDataRange xsd:string ;
            owl:onProperty <http://postdata.linhd.uned.es/ontology/postdata-prosodicElements#accentedVowelsPattern> ],
        <http://postdata.linhd.uned.es/ontology/postdata-prosodicElements#LinePattern> ;
    rdfs:isDefinedBy "http://postdata.linhd.uned.es/ontology/postdata-prosodicElements"@en ;
    rdfs:range xsd:string ;
    rdfs:subPropertyOf owl:topDataProperty .

<http://postdata.linhd.uned.es/ontology/postdata-prosodicElements#clausula> a owl:ObjectProperty ;
    rdfs:label "clausula"@en ;
    rdfs:comment "The categorisation of the item according to the rhythmic ending of a line  determined by the number of unstressed syllables following the last stressed one. This property is both valid for accentual and syllabic versification, so possible values include: masculine (zero syllables), femenine (one), dactylic, proparoxitone, etc."@en ;
    rdfs:domain <http://postdata.linhd.uned.es/ontology/postdata-prosodicElements#Foot> ;
    rdfs:isDefinedBy "http://postdata.linhd.uned.es/ontology/postdata-prosodicElements#clausula"@en ;
    rdfs:range [ a owl:Restriction ;
            owl:hasValue <http://postdata.linhd.uned.es/kos/clausula> ;
            owl:onProperty skos:inScheme ],
        skos:Concept .

<http://postdata.linhd.uned.es/ontology/postdata-prosodicElements#clausulaSchemeType> a owl:ObjectProperty ;
    rdfs:label "clausulaSchemeType"@en ;
    rdfs:comment "Categorisation of the stanza according to the distribution of clausulae/gender of rhymes (eg. “classic”, “heterogonique”, etc.)"@en ;
    rdfs:domain <http://postdata.linhd.uned.es/ontology/postdata-prosodicElements#StanzaPattern> ;
    rdfs:isDefinedBy "http://postdata.linhd.uned.es/ontology/postdata-prosodicElements"@en ;
    rdfs:range [ a owl:Restriction ;
            owl:hasValue <http://postdata.linhd.uned.es/kos/clausulaScheme-type> ;
            owl:onProperty skos:inScheme ],
        skos:Concept .

<http://postdata.linhd.uned.es/ontology/postdata-prosodicElements#initialPhonemesPatternByManner> a owl:DatatypeProperty ;
    rdfs:label "initialPhonemesPatternByManner"@en ;
    rdfs:comment "Initial phonemes of each word in a line represented by manner, in alphabetical order to show sound repetitions"@en ;
    rdfs:domain [ a owl:Restriction ;
            owl:maxQualifiedCardinality "1"^^xsd:nonNegativeInteger ;
            owl:onDataRange xsd:string ;
            owl:onProperty <http://postdata.linhd.uned.es/ontology/postdata-prosodicElements#initialPhonemesPatternByManner> ],
        <http://postdata.linhd.uned.es/ontology/postdata-prosodicElements#LinePattern> ;
    rdfs:isDefinedBy "http://postdata.linhd.uned.es/ontology/postdata-prosodicElements"@en ;
    rdfs:range xsd:string .

<http://postdata.linhd.uned.es/ontology/postdata-prosodicElements#isEmployedIn> a owl:ObjectProperty ;
    rdfs:label "isEmployedIn"@en ;
    rdfs:comment "This property points to the instance of MetricalEncoding that employs the item at hand"@en ;
    rdfs:domain <http://postdata.linhd.uned.es/ontology/postdata-prosodicElements#Symbol> ;
    rdfs:isDefinedBy "http://postdata.linhd.uned.es/ontology/postdata-prosodicElements"@en ;
    rdfs:range <http://postdata.linhd.uned.es/ontology/postdata-prosodicElements#MetricalEncoding> .

<http://postdata.linhd.uned.es/ontology/postdata-prosodicElements#isFirstFoot> a owl:ObjectProperty ;
    rdfs:label "isFirstFoot"@en ;
    rdfs:comment "This property points to the LinePattern whose feet description begins with the current item under analysis"@en ;
    rdfs:domain <http://postdata.linhd.uned.es/ontology/postdata-prosodicElements#Foot> ;
    rdfs:isDefinedBy "http://postdata.linhd.uned.es/ontology/postdata-prosodicElements"@en ;
    rdfs:range <http://postdata.linhd.uned.es/ontology/postdata-prosodicElements#LinePattern> .

<http://postdata.linhd.uned.es/ontology/postdata-prosodicElements#isFirstUnit> a owl:ObjectProperty ;
    rdfs:comment "This property points to the Foot that contains the item at hand as its first element"@en,
        "isFirstUnit"@en ;
    rdfs:domain <http://postdata.linhd.uned.es/ontology/postdata-prosodicElements#FootDivision> ;
    rdfs:isDefinedBy "http://postdata.linhd.uned.es/ontology/postdata-prosodicElements"@en ;
    rdfs:range <http://postdata.linhd.uned.es/ontology/postdata-prosodicElements#Foot> .

<http://postdata.linhd.uned.es/ontology/postdata-prosodicElements#isRhymeWord> a owl:ObjectProperty ;
    rdfs:label "isRhymeWord"@en ;
    rdfs:comment "This property points to the instance of Rhyme that contains the item at hand as its rhyme word"@en ;
    rdfs:domain <http://postdata.linhd.uned.es/ontology/postdata-structuralElements#Word> ;
    rdfs:isDefinedBy "http://postdata.linhd.uned.es/ontology/postdata-prosodicElements"@en ;
    rdfs:range <http://postdata.linhd.uned.es/ontology/postdata-prosodicElements#Rhyme> .

<http://postdata.linhd.uned.es/ontology/postdata-prosodicElements#matches> a owl:ObjectProperty ;
    rdfs:label "matches"@en ;
    dc:creator "mluisadiez" ;
    dc:date "2018-06-16T20:30:43+00:00"^^xsd:dateTime ;
    rdfs:comment "This property points to the instance of RhymeMatch that contains the echo of the current rhyme word under analysis"@en ;
    rdfs:domain <http://postdata.linhd.uned.es/ontology/postdata-prosodicElements#Rhyme> ;
    rdfs:isDefinedBy "http://postdata.linhd.uned.es/ontology/postdata-prosodicElements"@en ;
    rdfs:range <http://postdata.linhd.uned.es/ontology/postdata-prosodicElements#RhymeMatch> ;
    rdfs:subPropertyOf owl:topObjectProperty .

<http://postdata.linhd.uned.es/ontology/postdata-prosodicElements#presents> a owl:ObjectProperty ;
    rdfs:label "presents"@en ;
    dc:creator "mluisadiez" ;
    dc:date "2018-06-16T20:30:43+00:00"^^xsd:dateTime ;
    rdfs:comment "This property points to an instance of Rhyme that is contained in the current item under analysis"@en ;
    rdfs:isDefinedBy "http://postdata.linhd.uned.es/ontology/postdata-prosodicElements"@en ;
    rdfs:range <http://postdata.linhd.uned.es/ontology/postdata-prosodicElements#Rhyme> ;
    rdfs:subPropertyOf owl:topObjectProperty .

<http://postdata.linhd.uned.es/ontology/postdata-prosodicElements#previousFoot> a owl:ObjectProperty ;
    rdfs:label "previousFoot"@en ;
    rdfs:comment "This property points to the previous instance of Foot"@en ;
    rdfs:domain <http://postdata.linhd.uned.es/ontology/postdata-prosodicElements#Foot> ;
    rdfs:isDefinedBy "http://postdata.linhd.uned.es/ontology/postdata-prosodicElements"@en ;
    rdfs:range <http://postdata.linhd.uned.es/ontology/postdata-prosodicElements#Foot> .

<http://postdata.linhd.uned.es/ontology/postdata-prosodicElements#previousUnit> a owl:ObjectProperty ;
    rdfs:label "previousUnit"@en ;
    rdfs:comment "This property points to the previous unit that forms the foot (an instance of FootDivision)"@en ;
    rdfs:domain <http://postdata.linhd.uned.es/ontology/postdata-prosodicElements#FootDivision> ;
    rdfs:isDefinedBy "http://postdata.linhd.uned.es/ontology/postdata-prosodicElements"@en ;
    rdfs:range <http://postdata.linhd.uned.es/ontology/postdata-prosodicElements#FootDivision> .

<http://postdata.linhd.uned.es/ontology/postdata-prosodicElements#uses> a owl:ObjectProperty ;
    rdfs:label "uses"@en ;
    dc:creator "mluisadiez" ;
    dc:date "2018-06-16T20:30:43+00:00"^^xsd:dateTime ;
    rdfs:comment "This property points to the instance of MetricalEncoding in which the conventions implemented in the item at hand are explained" ;
    rdfs:domain <http://postdata.linhd.uned.es/ontology/postdata-prosodicElements#Pattern> ;
    rdfs:isDefinedBy "http://postdata.linhd.uned.es/ontology/postdata-prosodicElements"@en ;
    rdfs:range <http://postdata.linhd.uned.es/ontology/postdata-prosodicElements#MetricalEncoding> ;
    rdfs:subPropertyOf owl:topObjectProperty .

<http://postdata.linhd.uned.es/ontology/postdata-structuralElements#> a owl:Ontology ;
    dc:contributors """Alvaro Pérez (LINHD_POSTDATA-UNED)
https://www.linkedin.com/in/álvaro-pérez-pozo-ab241154/"""@en,
        """Bruno Sartini (Bolonia University)
https://orcid.org/0000-0002-9152-4402"""@en,
        """Javier de la Rosa (LINHD_POSTDATA-UNED)
https://www.linkedin.com/in/versae/"""@en,
        """Oscar Corcho (Universidad Politécnica de Madrid)
http://orcid.org/0000-0002-9260-0753"""@en ;
    dc:creator """Helena Bermúdez Sabel 
https://orcid.org/0000-0001-7782-206X"""@en,
        """Mª Luisa Díez Platas 
https://orcid.org/0000-0002-9416-3147"""@en ;
    dc:date "2019-07-12"@en ;
    dc:description "This ontology module contains classes and properties that provide information about the structure of a redaction. It models the structural elements from lexical level like lexical units, for example, word, to more complexity level as line or stanza."@en ;
    dc:title "postdata-structural ontology"@en ;
    terms:publisher "POSTDATA Project",
        """POSTDATA Project

“This project has received funding from the European Research Council (ERC) under the European Union’s Horizon 2020 research and innovation programme (grant agreement Nº [679528])”
Principal Investigator. Elena González Blanco -- https://orcid.org/0000-0002-0448-1812
Technical Director. Salvador Ros Muñoz -- https://orcid.org/0000-0001-6330-4958"""@en ;
    vann:preferredNamespacePrefix "pdstruct" ;
    owl:imports <http://postdata.linhd.uned.es/ontology/postdata-core>,
        <http://purl.org/ontology/olo/core#> ;
    owl:versionInfo "V1.0" ;
    ns1:license "https://creativecommons.org/licenses/by/4.0/"@en .

<http://postdata.linhd.uned.es/ontology/postdata-structuralElements#altStanzaNumber> a owl:DatatypeProperty ;
    rdfs:label "altStanzaNumber"@en ;
    dc:creator "mluisadiez" ;
    rdfs:comment "Position of the stanza inside the composition when a different ordering is possible"@en ;
    rdfs:domain <http://postdata.linhd.uned.es/ontology/postdata-structuralElements#Stanza> ;
    rdfs:isDefinedBy "http://postdata.linhd.uned.es/ontology/postdata-structuralElements"@en ;
    rdfs:range xsd:positiveInteger ;
    rdfs:subPropertyOf <http://purl.org/ontology/olo/core#index> .

<http://postdata.linhd.uned.es/ontology/postdata-structuralElements#hasLastLine> a owl:ObjectProperty ;
    rdfs:label "hasLastLine"@en ;
    rdfs:comment "This property points to the last line (an instance of Line) which form the current element under analysis"@en ;
    rdfs:domain [ a owl:Class ;
            owl:unionOf ( <http://postdata.linhd.uned.es/ontology/postdata-core#Redaction> <http://postdata.linhd.uned.es/ontology/postdata-structuralElements#OrderedLineList> <http://postdata.linhd.uned.es/ontology/postdata-structuralElements#Stanza> ) ] ;
    rdfs:range <http://postdata.linhd.uned.es/ontology/postdata-structuralElements#Line> ;
    rdfs:subPropertyOf owl:topObjectProperty ;
    owl:inverseOf <http://postdata.linhd.uned.es/ontology/postdata-structuralElements#isLastLine> .

<http://postdata.linhd.uned.es/ontology/postdata-structuralElements#hasLine> a owl:ObjectProperty ;
    rdfs:label "hasLine"@en ;
    rdfs:comment "Line of a Stanza considered as list"@en ;
    rdfs:domain <http://postdata.linhd.uned.es/ontology/postdata-structuralElements#Stanza> ;
    rdfs:isDefinedBy "http://postdata.linhd.uned.es/ontology/postdata-structuralElements"@en ;
    rdfs:range <http://postdata.linhd.uned.es/ontology/postdata-structuralElements#Line> ;
    rdfs:subPropertyOf <http://purl.org/ontology/olo/core#slot> .

<http://postdata.linhd.uned.es/ontology/postdata-structuralElements#hasSyllable> a owl:ObjectProperty ;
    rdfs:label "Syllable of a Word considered as list"@en,
        "hasSyllable"@en ;
    rdfs:domain <http://postdata.linhd.uned.es/ontology/postdata-structuralElements#Word> ;
    rdfs:isDefinedBy "http://postdata.linhd.uned.es/ontology/postdata-structuralElements"@en ;
    rdfs:range <http://postdata.linhd.uned.es/ontology/postdata-structuralElements#Syllable> ;
    rdfs:subPropertyOf <http://purl.org/ontology/olo/core#slot> .

<http://postdata.linhd.uned.es/ontology/postdata-structuralElements#hasToken> a owl:ObjectProperty ;
    rdfs:label "hasToken"@en ;
    rdfs:comment "Token of a Line considered as list"@en ;
    rdfs:domain <http://postdata.linhd.uned.es/ontology/postdata-structuralElements#Line> ;
    rdfs:isDefinedBy "http://postdata.linhd.uned.es/ontology/postdata-structuralElements"@en ;
    rdfs:range <http://postdata.linhd.uned.es/ontology/postdata-structuralElements#Token> ;
    rdfs:subPropertyOf <http://purl.org/ontology/olo/core#slot> .

<http://postdata.linhd.uned.es/ontology/postdata-structuralElements#isFirstLine> a owl:ObjectProperty ;
    rdfs:label "isFirstLine"@en ;
    rdfs:comment "This property points to the group of lines (an instance of Stanza or an instance of OrderedLineList) of which the current item under analysis is its first line"@en ;
    rdfs:domain <http://postdata.linhd.uned.es/ontology/postdata-structuralElements#Line> ;
    rdfs:isDefinedBy "http://postdata.linhd.uned.es/ontology/postdata-structuralElements"@en ;
    rdfs:range <http://postdata.linhd.uned.es/ontology/postdata-structuralElements#Stanza> .

<http://postdata.linhd.uned.es/ontology/postdata-structuralElements#isFirstStanza> a owl:ObjectProperty ;
    rdfs:label "isFirstStanza"@en ;
    rdfs:comment "This property points to the text (an instance of OrderedStanzaList) of which the current item under analysis is its first line grouping"@en ;
    rdfs:domain <http://postdata.linhd.uned.es/ontology/postdata-structuralElements#Stanza> ;
    rdfs:isDefinedBy "http://postdata.linhd.uned.es/ontology/postdata-structuralElements"@en ;
    rdfs:range <http://postdata.linhd.uned.es/ontology/postdata-core#Redaction> .

<http://postdata.linhd.uned.es/ontology/postdata-structuralElements#isFirstSyllable> a owl:ObjectProperty ;
    rdfs:label "isFirstSyllable"@en ;
    rdfs:comment "This property points to an instance of Word of which the current item under analysis is its first Syllable"@en ;
    rdfs:domain <http://postdata.linhd.uned.es/ontology/postdata-structuralElements#Syllable> ;
    rdfs:isDefinedBy "http://postdata.linhd.uned.es/ontology/postdata-structuralElements"@en ;
    rdfs:range <http://postdata.linhd.uned.es/ontology/postdata-structuralElements#Word> .

<http://postdata.linhd.uned.es/ontology/postdata-structuralElements#isFirstToken> a owl:ObjectProperty ;
    rdfs:label "isFirstToken"@en ;
    rdfs:comment "This property points to an instance of Line of which the current item under analysis is its first Token" ;
    rdfs:domain <http://postdata.linhd.uned.es/ontology/postdata-structuralElements#Token> ;
    rdfs:isDefinedBy "http://postdata.linhd.uned.es/ontology/postdata-structuralElements"@en ;
    rdfs:range <http://postdata.linhd.uned.es/ontology/postdata-structuralElements#Line> .

<http://postdata.linhd.uned.es/ontology/postdata-structuralElements#isInflectedForm> a owl:ObjectProperty ;
    rdfs:label "inflectedForm"@en ;
    dc:creator "mluisadiez" ;
    rdfs:comment "This property points to its lemma (an instance of Word)"@en ;
    rdfs:domain <http://postdata.linhd.uned.es/ontology/postdata-structuralElements#Word> ;
    rdfs:range <http://postdata.linhd.uned.es/ontology/postdata-structuralElements#Word> ;
    rdfs:subPropertyOf owl:topObjectProperty ;
    owl:inverseOf <http://postdata.linhd.uned.es/ontology/postdata-structuralElements#isLemma> .

<http://postdata.linhd.uned.es/ontology/postdata-structuralElements#isLastLine> a owl:ObjectProperty ;
    rdfs:label "isLastLine"@en ;
    rdfs:comment "This property points to Stanza or OrderedLineList of which the current item under analysis is its last Line"@en ;
    rdfs:domain <http://postdata.linhd.uned.es/ontology/postdata-structuralElements#Line> ;
    rdfs:isDefinedBy "http://postdata.linhd.uned.es/ontology/postdata-structuralElements"@en ;
    rdfs:range [ a owl:Class ;
            owl:unionOf ( <http://postdata.linhd.uned.es/ontology/postdata-core#Redaction> <http://postdata.linhd.uned.es/ontology/postdata-structuralElements#OrderedLineList> <http://postdata.linhd.uned.es/ontology/postdata-structuralElements#Stanza> ) ] ;
    rdfs:subPropertyOf owl:topObjectProperty .

<http://postdata.linhd.uned.es/ontology/postdata-structuralElements#isLastStanza> a owl:ObjectProperty ;
    rdfs:label "isLastStanza"@en ;
    rdfs:comment "This property points to OrderedStanzaList of which the current item under analysis is its last Stanza"@en ;
    rdfs:domain <http://postdata.linhd.uned.es/ontology/postdata-structuralElements#Stanza> ;
    rdfs:isDefinedBy "http://postdata.linhd.uned.es/ontology/postdata-structuralElements"@en ;
    rdfs:range [ a owl:Class ;
            owl:unionOf ( <http://postdata.linhd.uned.es/ontology/postdata-core#Redaction> <http://postdata.linhd.uned.es/ontology/postdata-structuralElements#OrderedStanzaList> ) ] ;
    rdfs:subPropertyOf owl:topObjectProperty .

<http://postdata.linhd.uned.es/ontology/postdata-structuralElements#isLastSyllable> a owl:ObjectProperty ;
    rdfs:label "isLastSyllable"@en ;
    rdfs:comment "This property points to Word of which the current item under analysis is its last Syllable"@en ;
    rdfs:domain <http://postdata.linhd.uned.es/ontology/postdata-structuralElements#Syllable> ;
    rdfs:isDefinedBy "http://postdata.linhd.uned.es/ontology/postdata-structuralElements"@en ;
    rdfs:range <http://postdata.linhd.uned.es/ontology/postdata-structuralElements#Word> ;
    rdfs:subPropertyOf owl:topObjectProperty .

<http://postdata.linhd.uned.es/ontology/postdata-structuralElements#isLastToken> a owl:ObjectProperty ;
    rdfs:label "isLastToken"@en ;
    rdfs:comment "This property points to Line of which the current item under analysis is its last Token"@en ;
    rdfs:domain <http://postdata.linhd.uned.es/ontology/postdata-structuralElements#Token> ;
    rdfs:isDefinedBy "http://postdata.linhd.uned.es/ontology/postdata-structuralElements"@en ;
    rdfs:range <http://postdata.linhd.uned.es/ontology/postdata-structuralElements#Line> ;
    rdfs:subPropertyOf owl:topObjectProperty .

<http://postdata.linhd.uned.es/ontology/postdata-structuralElements#isLemma> a owl:ObjectProperty ;
    rdfs:label "isLemma"@en ;
    rdfs:comment "This property points to one of the inflected forms (an instance of Word) of the current headword (the Word at hand)"@en ;
    rdfs:domain <http://postdata.linhd.uned.es/ontology/postdata-structuralElements#Word> ;
    rdfs:isDefinedBy "http://postdata.linhd.uned.es/ontology/postdata-structuralElements"@en ;
    rdfs:range <http://postdata.linhd.uned.es/ontology/postdata-structuralElements#Word> .

<http://postdata.linhd.uned.es/ontology/postdata-structuralElements#isLineListOfRedaction> a owl:ObjectProperty ;
    rdfs:label "isLineListOfRedaction"@en ;
    rdfs:comment "This property refers to the Redaction that OrderedLineList belongs to"@en ;
    rdfs:domain <http://postdata.linhd.uned.es/ontology/postdata-structuralElements#OrderedLineList> ;
    rdfs:isDefinedBy "http://postdata.linhd.uned.es/ontology/postdata-structuralElements/"@en ;
    rdfs:range <http://postdata.linhd.uned.es/ontology/postdata-core#Redaction> .

<http://postdata.linhd.uned.es/ontology/postdata-structuralElements#isStanzaListOfRedaction> a owl:ObjectProperty ;
    rdfs:label "isStanzaListOfRedaction"@en ;
    rdfs:comment "This property refers to the Redaction that OrderedStanzaList belongs to"@en ;
    rdfs:domain <http://postdata.linhd.uned.es/ontology/postdata-structuralElements#OrderedStanzaList> ;
    rdfs:isDefinedBy "http://postdata.linhd.uned.es/ontology/postdata-structuralElements/"@en ;
    rdfs:range <http://postdata.linhd.uned.es/ontology/postdata-core#Redaction> .

<http://postdata.linhd.uned.es/ontology/postdata-structuralElements#lemma> a owl:DatatypeProperty ;
    rdfs:label "lemma"@en ;
    dc:creator "mluisadiez" ;
    rdfs:comment "Citation form, the particular form that is chosen by convention to represent the lexeme"@en ;
    rdfs:domain <http://postdata.linhd.uned.es/ontology/postdata-structuralElements#Word> ;
    rdfs:isDefinedBy "http://postdata.linhd.uned.es/ontology/postdata-structuralElements"@en ;
    rdfs:range xsd:string ;
    rdfs:subPropertyOf owl:topDataProperty .

<http://postdata.linhd.uned.es/ontology/postdata-structuralElements#morphologicalAnnotation> a owl:DatatypeProperty ;
    rdfs:label "morphologicalAnnotation"@en ;
    dc:creator "mluisadiez" ;
    rdfs:comment "Any type of morphological analysis (from POS to morpheme composition)"@en ;
    rdfs:domain <http://postdata.linhd.uned.es/ontology/postdata-structuralElements#Word> ;
    rdfs:isDefinedBy "http://postdata.linhd.uned.es/ontology/postdata-structuralElements"@en ;
    rdfs:range xsd:string ;
    rdfs:subPropertyOf owl:topDataProperty .

<http://postdata.linhd.uned.es/ontology/postdata-structuralElements#paraphrasis> a owl:DatatypeProperty ;
    rdfs:label "paraphrasis"@en ;
    dc:creator "mluisadiez" ;
    rdfs:comment "The recasting of the contents in words different from that originally used, whether in the same language or in a translation"@en ;
    rdfs:domain <http://postdata.linhd.uned.es/ontology/postdata-structuralElements#Stanza> ;
    rdfs:isDefinedBy "http://postdata.linhd.uned.es/ontology/postdata-structuralElements"@en ;
    rdfs:range xsd:string ;
    rdfs:subPropertyOf owl:topDataProperty .

<http://postdata.linhd.uned.es/ontology/postdata-structuralElements#phoneticTranscription> a owl:DatatypeProperty ;
    rdfs:label "phoneticTranscription"@en ;
    dc:creator "mluisadiez" ;
    rdfs:comment "Phonetic transcription"@en ;
    rdfs:domain <http://postdata.linhd.uned.es/ontology/postdata-structuralElements#Word> ;
    rdfs:isDefinedBy "http://postdata.linhd.uned.es/ontology/postdata-structuralElements"@en ;
    rdfs:range xsd:string ;
    rdfs:subPropertyOf owl:topDataProperty .

<http://postdata.linhd.uned.es/ontology/postdata-structuralElements#previousLine> a owl:ObjectProperty ;
    rdfs:label "previousLine"@en ;
    rdfs:comment "This property points to the previous item of a list that contains an instance of Line"@en ;
    rdfs:domain <http://postdata.linhd.uned.es/ontology/postdata-structuralElements#Line> ;
    rdfs:isDefinedBy "http://postdata.linhd.uned.es/ontology/postdata-structuralElements"@en ;
    rdfs:range <http://postdata.linhd.uned.es/ontology/postdata-structuralElements#Line> ;
    rdfs:subPropertyOf <http://purl.org/ontology/olo/core#previous> .

<http://postdata.linhd.uned.es/ontology/postdata-structuralElements#previousStanza> a owl:ObjectProperty ;
    rdfs:label "previousStanza"@en ;
    rdfs:comment "This property points to previous Stanza of the Stanza under analysis, in a OrderedLineList or in a Stanza"@en ;
    rdfs:domain <http://postdata.linhd.uned.es/ontology/postdata-structuralElements#Stanza> ;
    rdfs:isDefinedBy "http://postdata.linhd.uned.es/ontology/postdata-structuralElements"@en ;
    rdfs:range <http://postdata.linhd.uned.es/ontology/postdata-structuralElements#Stanza> ;
    rdfs:subPropertyOf <http://purl.org/ontology/olo/core#previous> .

<http://postdata.linhd.uned.es/ontology/postdata-structuralElements#previousSyllable> a owl:ObjectProperty ;
    rdfs:label "previousSyllable"@en ;
    rdfs:comment "This property points to previous Syllable of the Syllable under analysis, in a Word"@en ;
    rdfs:domain <http://postdata.linhd.uned.es/ontology/postdata-structuralElements#Syllable> ;
    rdfs:isDefinedBy "http://postdata.linhd.uned.es/ontology/postdata-structuralElements"@en ;
    rdfs:range <http://postdata.linhd.uned.es/ontology/postdata-structuralElements#Syllable> ;
    rdfs:subPropertyOf <http://purl.org/ontology/olo/core#previous> .

<http://postdata.linhd.uned.es/ontology/postdata-structuralElements#previousToken> a owl:ObjectProperty ;
    rdfs:label "previousToken"@en ;
    rdfs:comment "This property points to previous Token of the Token under analysis, in a Line" ;
    rdfs:domain <http://postdata.linhd.uned.es/ontology/postdata-structuralElements#Token> ;
    rdfs:isDefinedBy "http://postdata.linhd.uned.es/ontology/postdata-structuralElements"@en ;
    rdfs:range <http://postdata.linhd.uned.es/ontology/postdata-structuralElements#Token> ;
    rdfs:subPropertyOf <http://purl.org/ontology/olo/core#previous> .

dc:title a owl:AnnotationProperty,
        owl:DatatypeProperty .

terms:bibliographicCitation a owl:DatatypeProperty .

<http://purl.org/linguistics/gold/Foot> a owl:Class .

<http://purl.org/spar/fabio/hasSubtitle> a owl:DatatypeProperty ;
    rdfs:label "has subtitle"@en ;
    rdfs:comment "A secondary title that follows the main title of a work."@en .

<http://purl.org/vocab/bio/0.1/biography> a owl:DatatypeProperty ;
    rdfs:label "Biography"@en ;
    rdfs:comment "An extended description or account of someone's life."@en ;
    rdfs:isDefinedBy "http://purl.org/vocab/bio/0.1/" .

<http://schema.org/endDate> a owl:DatatypeProperty ;
    rdfs:label "endDate"@en ;
    rdfs:comment "The end date and time of the item (in <a href=\"http://en.wikipedia.org/wiki/ISO_8601\">ISO 8601 date format</a>)."@en ;
    rdfs:isDefinedBy "https://schema.org/endDate" .

<http://schema.org/startDate> a owl:DatatypeProperty ;
    rdfs:label "startDate"@en .

<http://www.europeana.eu/schemas/edm/Agent> a owl:Class ;
    rdfs:label "Agent"@en ;
    skos:definition """This class comprises people, either individually or in groups, who have the
potential to perform intentional actions for which they can be held responsible.""" ;
    skos:example "Leonardo da Vinci, the British Museum, W3C" .

<http://www.europeana.eu/schemas/edm/Place> a owl:Class ;
    rdfs:label "Place"@en ;
    skos:definition "An \"extent in space, in particular on the surface of the earth, in the pure sense of physics: independent from temporal phenomena and matter\" (CIDOC CRM)"@en .

<http://www.europeana.eu/schemas/edm/ProvidedCHO> a owl:Class ;
    rdfs:label "Provided CHO"@en ;
    skos:definition "This class comprises the Cultural Heritage objects that Europeana collects descriptions about."@en ;
    skos:note "This class has been mostly motivated by the need to assign a type to the “central node” in the EDM pattern, during the ingestion process, related to the XML expression of EDM at that stage. It was especially intended to fit the cases where edm:PhysicalThing  cannot be used as the type of the resource standing for the real-world object (independently of any specific data contributor perspective)."@en .

<http://www.europeana.eu/schemas/edm/TimeSpan> a owl:Class .

<http://www.ontologydesignpatterns.org/cp/owl/agentrole.owl#Agent> a owl:Class .

<http://xmlns.com/foaf/0.1/name> a owl:DatatypeProperty ;
    rdfs:label "name"@en ;
    rdfs:comment "A name for some thing."@en ;
    rdfs:isDefinedBy "http://xmlns.com/foaf/0.1" ;
    ns1:term_status "testing"@en .

<http://iflastandards.info/ns/fr/frbr/frbroo/F2_Expression> a owl:Class .

<http://postdata.linhd.uned.es/kos/author-education-level> a owl:NamedIndividual,
        skos:ConceptScheme ;
    skos:definition "Thesaurus about author education level"@en .

<http://postdata.linhd.uned.es/kos/clausula> a owl:NamedIndividual,
        skos:ConceptScheme .

<http://postdata.linhd.uned.es/kos/clausulaScheme-type> a owl:NamedIndividual,
        skos:ConceptScheme .

<http://postdata.linhd.uned.es/kos/designation-type> a owl:NamedIndividual,
        skos:ConceptScheme ;
    skos:definition "Thesaurus about type of name"@en .

<http://postdata.linhd.uned.es/kos/gender> a owl:NamedIndividual,
        skos:ConceptScheme ;
    skos:definition "Thesaurus about genders"@en .

<http://postdata.linhd.uned.es/kos/literary-period> a owl:NamedIndividual,
        skos:ConceptScheme ;
    skos:definition "Thesaurus about labels of a time frame for grouping certain works"@en .

<http://postdata.linhd.uned.es/kos/poetic-type> a owl:NamedIndividual,
        skos:ConceptScheme ;
    skos:definition "Thesaurus about major literary genre of the compositions"@en .

<http://postdata.linhd.uned.es/kos/religious-affiliation> a owl:NamedIndividual,
        skos:ConceptScheme ;
    skos:definition "Thesaurus about religious affiliations"@en .

<http://postdata.linhd.uned.es/kos/role-function> a owl:NamedIndividual,
        skos:ConceptScheme ;
    skos:definition "Thesaurus about specific function performed by some agent on a work"@en .

<http://postdata.linhd.uned.es/kos/school> a owl:NamedIndividual,
        skos:ConceptScheme ;
    skos:definition "Thesaurus about literary movements or schools of an author"@en .

<http://postdata.linhd.uned.es/kos/social-status> a owl:NamedIndividual,
        skos:ConceptScheme ;
    skos:definition "Thesaurus about the socialstatus of a person"@en .

<http://postdata.linhd.uned.es/kos/textual-element-type> a owl:NamedIndividual,
        skos:ConceptScheme ;
    skos:definition "Thesaurus about type of textual element"@en .

<http://postdata.linhd.uned.es/ontology/postdata-core#birthPlaceCertainty> a owl:ObjectProperty ;
    rdfs:label "birth Place Certainty"@en ;
    rdfs:comment "Certainty of the date of birth of a Person"@en ;
    rdfs:domain <http://postdata.linhd.uned.es/ontology/postdata-core#Person> ;
    rdfs:isDefinedBy "http://postdata.linhd.uned.es/ontology/postdata-core/" ;
    rdfs:subPropertyOf <http://postdata.linhd.uned.es/ontology/postdata-core#certainty> .

<http://postdata.linhd.uned.es/ontology/postdata-core#genre> a owl:ObjectProperty ;
    rdfs:label "genre"@en ;
    rdfs:comment "Type of art, literature or music characterized by a specific form, content and style"@en ;
    rdfs:domain [ a owl:Class ;
            owl:unionOf ( <http://postdata.linhd.uned.es/ontology/postdata-core#PoeticWork> <http://postdata.linhd.uned.es/ontology/postdata-core#Redaction> ) ] ;
    rdfs:isDefinedBy "http://postdata.linhd.uned.es/ontology/postdata-core/" ;
    rdfs:range [ a owl:Restriction ;
            owl:hasValue <http://postdata.linhd.uned.es/kos/genre> ;
            owl:onProperty skos:inScheme ],
        skos:Concept .

<http://postdata.linhd.uned.es/ontology/postdata-core#hasEditor> a owl:ObjectProperty ;
    rdfs:label "has Editor"@en ;
    rdfs:comment "This property points to the Person who has edited the current instance of Redaction"@en ;
    rdfs:domain <http://postdata.linhd.uned.es/ontology/postdata-core#Redaction> ;
    rdfs:isDefinedBy "http://postdata.linhd.uned.es/ontology/postdata-core/" ;
    rdfs:range <http://postdata.linhd.uned.es/ontology/postdata-core#Person> .

<http://postdata.linhd.uned.es/ontology/postdata-core#hasProvenance> a owl:ObjectProperty ;
    rdfs:label "has Provenance"@en ;
    rdfs:comment "This property points to the Place which is the provenance of the current instance of Ensemble or Poetic Work"@en ;
    rdfs:domain [ a owl:Class ;
            owl:unionOf ( <http://postdata.linhd.uned.es/ontology/postdata-core#Ensemble> <http://postdata.linhd.uned.es/ontology/postdata-core#PoeticWork> ) ] ;
    rdfs:isDefinedBy "http://postdata.linhd.uned.es/ontology/postdata-core/" ;
    rdfs:range <http://postdata.linhd.uned.es/ontology/postdata-core#Place> ;
    owl:inverseOf <http://postdata.linhd.uned.es/ontology/postdata-core#isProvenanceFor> .

<http://postdata.linhd.uned.es/ontology/postdata-core#hasTranslation> a owl:ObjectProperty ;
    rdfs:label "has Translation"@en ;
    rdfs:comment "This property points to another work (an instance of Redaction) which is a translation of this one"@en,
        "This property points to the specific location in a bibliographic item (an instance of Location) which contains a translation of the text at hand"@en ;
    rdfs:domain <http://postdata.linhd.uned.es/ontology/postdata-core#Redaction> ;
    rdfs:isDefinedBy "http://postdata.linhd.uned.es/ontology/postdata-core/" ;
    rdfs:range <http://postdata.linhd.uned.es/ontology/postdata-core#Redaction>,
        <http://postdata.linhd.uned.es/ontology/postdata-transmission#Location> ;
    owl:inverseOf <http://postdata.linhd.uned.es/ontology/postdata-core#isTranslationOf> .

<http://postdata.linhd.uned.es/ontology/postdata-core#isInvolvedIn> a owl:ObjectProperty ;
    rdfs:label "is Involved In"@en ;
    rdfs:comment "This property points to the Event in which the current instance of Organisation, Person or Place is referenced"@en ;
    rdfs:domain [ a owl:Class ;
            owl:unionOf ( <http://postdata.linhd.uned.es/ontology/postdata-core#Agent> <http://postdata.linhd.uned.es/ontology/postdata-core#Place> ) ] ;
    rdfs:isDefinedBy "http://postdata.linhd.uned.es/ontology/postdata-core/" ;
    rdfs:range <http://postdata.linhd.uned.es/ontology/postdata-core#Event> .

<http://postdata.linhd.uned.es/ontology/postdata-core#isSynthesisOf> a owl:ObjectProperty ;
    rdfs:label "is Synthesis Of"@en ;
    rdfs:comment "This property points to another text (an instance of Redaction) of which this version (Redaction) is a synthesis"@en ;
    rdfs:domain <http://postdata.linhd.uned.es/ontology/postdata-core#Redaction> ;
    rdfs:isDefinedBy "http://postdata.linhd.uned.es/ontology/postdata-core/" ;
    rdfs:range <http://postdata.linhd.uned.es/ontology/postdata-core#Redaction> .

<http://postdata.linhd.uned.es/ontology/postdata-core#narrativeLocation> a owl:DatatypeProperty ;
    rdfs:label "narrative Location"@en ;
    rdfs:comment """Location of the narrative. There is at most one possible location for a Redaction or Poetic Work.

Taking as example the poem “Cantar de Mio Cid”, the “narrativeLocation” would be “Spain”."""@en ;
    rdfs:domain [ a owl:Class ;
            owl:unionOf ( <http://postdata.linhd.uned.es/ontology/postdata-core#PoeticWork> <http://postdata.linhd.uned.es/ontology/postdata-core#Redaction> ) ] ;
    rdfs:isDefinedBy "http://postdata.linhd.uned.es/ontology/postdata-core/" ;
    rdfs:range xsd:string .

<http://postdata.linhd.uned.es/ontology/postdata-core#originalName> a owl:DatatypeProperty ;
    rdfs:label "original Name"@en ;
    rdfs:comment "Name of the place as it appears in the source text"@en ;
    rdfs:domain [ a owl:Class ;
            owl:unionOf ( <http://postdata.linhd.uned.es/ontology/postdata-core#Place> <http://xmlns.com/foaf/0.1/Person> ) ] ;
    rdfs:isDefinedBy "http://postdata.linhd.uned.es/ontology/postdata-core/" ;
    rdfs:range xsd:string ;
    rdfs:subPropertyOf owl:topDataProperty .

<http://postdata.linhd.uned.es/ontology/postdata-core#originalTitle> a owl:DatatypeProperty ;
    rdfs:label "original Title"@en ;
    rdfs:comment "The identifying name of a Redaction or Poetic Work as it appears in its primary source. There is at most one possible original title."@en ;
    rdfs:domain [ a owl:Class ;
            owl:unionOf ( <http://postdata.linhd.uned.es/ontology/postdata-core#PoeticWork> <http://postdata.linhd.uned.es/ontology/postdata-core#Redaction> ) ] ;
    rdfs:isDefinedBy "http://postdata.linhd.uned.es/ontology/postdata-core/" ;
    rdfs:range xsd:string .

<http://postdata.linhd.uned.es/ontology/postdata-core#realises> a owl:ObjectProperty ;
    rdfs:label "realises"@en ;
    rdfs:comment "This property points to the work (an instance of Poetic Work) of which the text at hand (the current Redaction) is a materialisation"@en ;
    rdfs:domain <http://postdata.linhd.uned.es/ontology/postdata-core#Redaction> ;
    rdfs:isDefinedBy "http://postdata.linhd.uned.es/ontology/postdata-core/" ;
    rdfs:range <http://postdata.linhd.uned.es/ontology/postdata-core#PoeticWork> .

<http://postdata.linhd.uned.es/ontology/postdata-dates#OpenedIntervalExpression> a owl:Class ;
    rdfs:label "OpenInterval"@en ;
    rdfs:comment "The date range without precise specification"@en ;
    rdfs:isDefinedBy "http://postdata.linhd.uned.es/ontology/postdata-dates" ;
    rdfs:subClassOf <http://postdata.linhd.uned.es/ontology/postdata-dates#IntervalExpression> .

<http://postdata.linhd.uned.es/ontology/postdata-dates#stringContent> a owl:DatatypeProperty ;
    rdfs:label "stringContent"@en ;
    rdfs:comment "Value of the date as string ."@en ;
    rdfs:domain <http://postdata.linhd.uned.es/ontology/postdata-dates#ApproximateDateExpression> ;
    rdfs:isDefinedBy "http://postdata.linhd.uned.es/ontology/postdata-dates" ;
    rdfs:range xsd:string ;
    rdfs:subPropertyOf owl:topDataProperty .

<http://postdata.linhd.uned.es/ontology/postdata-prosodicElements#altRhymeScheme> a owl:DatatypeProperty ;
    rdfs:label "altRhymeScheme"@en ;
    dc:creator "mluisadiez" ;
    rdfs:comment "An alternative rhyme scheme (usually in relation with an alternative metrical scheme)" ;
    rdfs:isDefinedBy "http://postdata.linhd.uned.es/ontology/postdata-prosodicElements"@en ;
    rdfs:range xsd:string ;
    rdfs:subPropertyOf owl:topDataProperty .

<http://postdata.linhd.uned.es/ontology/postdata-prosodicElements#feetType> a owl:ObjectProperty ;
    rdfs:label "feetType"@en ;
    rdfs:comment "Categorisation of the stanza or line according to the type of feet"@en ;
    rdfs:isDefinedBy "http://postdata.linhd.uned.es/ontology/postdata-prosodicElements"@en ;
    rdfs:range [ a owl:Restriction ;
            owl:hasValue <http://postdata.linhd.uned.es/kos/feet-type> ;
            owl:onProperty skos:inScheme ],
        skos:Concept .

<http://postdata.linhd.uned.es/ontology/postdata-prosodicElements#grammaticalStressPattern> a owl:DatatypeProperty ;
    rdfs:label "grammaticalStressPattern"@en ;
    dc:creator "mluisadiez" ;
    rdfs:comment "Pattern based on disposition of the expected stresses according to grammar rules. This includes the distribution of weak and strong positions" ;
    rdfs:isDefinedBy "http://postdata.linhd.uned.es/ontology/postdata-prosodicElements"@en ;
    rdfs:range xsd:string ;
    rdfs:subPropertyOf owl:topDataProperty .

<http://postdata.linhd.uned.es/ontology/postdata-prosodicElements#hasAnacrusis> a owl:DatatypeProperty ;
    rdfs:label "hasAnacrusis"@en ;
    dc:creator "mluisadiez" ;
    dc:date "2018-06-16T18:39:21+00:00"^^xsd:dateTime ;
    rdfs:comment "If the line has one or more unstressed syllables at the beginning of a line of verse, before the reckoning of the normal meter begins" ;
    rdfs:isDefinedBy "http://postdata.linhd.uned.es/ontology/postdata-prosodicElements"@en ;
    rdfs:range xsd:boolean ;
    rdfs:subPropertyOf owl:topDataProperty .

<http://postdata.linhd.uned.es/ontology/postdata-prosodicElements#metricalType> a owl:ObjectProperty ;
    rdfs:label "metricalType"@en ;
    rdfs:comment "Categorisation of the stanza/line  grouping or work according to metrics. E.g. “sapphic stanza”"@en ;
    rdfs:isDefinedBy "http://postdata.linhd.uned.es/ontology/postdata-prosodicElements"@en ;
    rdfs:range [ a owl:Restriction ;
            owl:hasValue <http://postdata.linhd.uned.es/kos/metrical-type> ;
            owl:onProperty skos:inScheme ],
        skos:Concept .

<http://postdata.linhd.uned.es/ontology/postdata-prosodicElements#previousFootBeforeCaesura> a owl:ObjectProperty ;
    rdfs:label "previousFootBeforeCaesura"@en ;
    rdfs:comment "This property points to the previous instance of Foot when this is positioned before a caesura"@en ;
    rdfs:domain [ a owl:Restriction ;
            owl:maxQualifiedCardinality "1"^^xsd:nonNegativeInteger ;
            owl:onClass <http://postdata.linhd.uned.es/ontology/postdata-prosodicElements#Foot> ;
            owl:onProperty <http://postdata.linhd.uned.es/ontology/postdata-prosodicElements#previousFootBeforeCaesura> ],
        <http://postdata.linhd.uned.es/ontology/postdata-prosodicElements#Foot> ;
    rdfs:isDefinedBy "http://postdata.linhd.uned.es/ontology/postdata-prosodicElements"@en ;
    rdfs:range <http://postdata.linhd.uned.es/ontology/postdata-prosodicElements#Foot> .

<http://postdata.linhd.uned.es/ontology/postdata-prosodicElements#rhymeScheme> a owl:DatatypeProperty ;
    rdfs:label "rhymeScheme"@en ;
    dc:creator "mluisadiez" ;
    dc:date "2018-06-16T18:39:21+00:00"^^xsd:dateTime ;
    rdfs:comment "A rhyme scheme is the pattern of rhymes at the end of each line of a poem or song. It is usually referred to by using letters to indicate which lines rhyme; lines designated with the same letter all rhyme with each other" ;
    rdfs:domain <http://postdata.linhd.uned.es/ontology/postdata-prosodicElements#Rhyme> ;
    rdfs:isDefinedBy "http://postdata.linhd.uned.es/ontology/postdata-prosodicElements"@en ;
    rdfs:range xsd:string ;
    rdfs:subPropertyOf owl:topDataProperty .

<http://postdata.linhd.uned.es/ontology/postdata-structuralElements#containsMentionTo> a owl:ObjectProperty ;
    rdfs:label "containsMentionTo"@en ;
    rdfs:comment "Agent or Place that is mentioned on the line"@en ;
    rdfs:domain <http://postdata.linhd.uned.es/ontology/postdata-structuralElements#Line> ;
    rdfs:isDefinedBy "http://postdata.linhd.uned.es/ontology/postdata-structuralElements"@en .

<http://postdata.linhd.uned.es/ontology/postdata-structuralElements#hasFirstLine> a owl:ObjectProperty ;
    rdfs:label "hasFirstLine"@en ;
    dc:creator "mluisadiez" ;
    rdfs:comment "This property points to the first line (an instance of Line) which form the current element under analysis" ;
    rdfs:domain <http://postdata.linhd.uned.es/ontology/postdata-structuralElements#Stanza> ;
    rdfs:isDefinedBy "http://postdata.linhd.uned.es/ontology/postdata-structuralElements"@en ;
    rdfs:range <http://postdata.linhd.uned.es/ontology/postdata-structuralElements#Line> ;
    rdfs:subPropertyOf owl:topObjectProperty ;
    owl:inverseOf <http://postdata.linhd.uned.es/ontology/postdata-structuralElements#isFirstLine> .

<http://postdata.linhd.uned.es/ontology/postdata-structuralElements#hasLineItem> a owl:ObjectProperty ;
    rdfs:label "hasLineItem"@en ;
    rdfs:comment "Line of a OrderedLineList associated with a Redaction"@en ;
    rdfs:domain <http://postdata.linhd.uned.es/ontology/postdata-structuralElements#OrderedLineList> ;
    rdfs:isDefinedBy "http://postdata.linhd.uned.es/ontology/postdata-structuralElements"@en ;
    rdfs:range <http://postdata.linhd.uned.es/ontology/postdata-structuralElements#Line> ;
    rdfs:subPropertyOf <http://purl.org/ontology/olo/core#slot> .

<http://postdata.linhd.uned.es/ontology/postdata-structuralElements#hasStanzaItem> a owl:ObjectProperty ;
    rdfs:label "hasStanzaItem"@en ;
    rdfs:comment "Stanza of an OrderedStanzaList associated with a Redaction"@en ;
    rdfs:domain <http://postdata.linhd.uned.es/ontology/postdata-structuralElements#OrderedStanzaList> ;
    rdfs:isDefinedBy "http://postdata.linhd.uned.es/ontology/postdata-structuralElements"@en ;
    rdfs:range <http://postdata.linhd.uned.es/ontology/postdata-structuralElements#Stanza> ;
    rdfs:subPropertyOf <http://purl.org/ontology/olo/core#slot> .

<http://postdata.linhd.uned.es/ontology/postdata-structuralElements#isRefrain> a owl:DatatypeProperty ;
    rdfs:label "isRefrain"@en ;
    rdfs:comment "Whether the line or group of lines is part of a refrain"@en ;
    rdfs:domain <http://postdata.linhd.uned.es/ontology/postdata-structuralElements#Line> ;
    rdfs:isDefinedBy "http://postdata.linhd.uned.es/ontology/postdata-structuralElements"@en ;
    rdfs:range xsd:boolean .

<http://postdata.linhd.uned.es/ontology/postdata-structuralElements#lineNumber> a owl:DatatypeProperty ;
    rdfs:label "lineNumber"@en ;
    dc:creator "mluisadiez" ;
    rdfs:comment "Number of the verse" ;
    rdfs:domain <http://postdata.linhd.uned.es/ontology/postdata-structuralElements#Line> ;
    rdfs:isDefinedBy "http://postdata.linhd.uned.es/ontology/postdata-structuralElements"@en ;
    rdfs:range xsd:positiveInteger ;
    rdfs:subPropertyOf <http://purl.org/ontology/olo/core#index> .

<http://purl.org/net/nknouf/ns/bibtex#hasNote> a owl:DatatypeProperty ;
    rdfs:label "has note"@en ;
    rdfs:comment "Any additional information that can help the reader. The first word should be capitalized."@en .

<http://postdata.linhd.uned.es/kos/feet-type> a owl:NamedIndividual,
        skos:ConceptScheme .

<http://postdata.linhd.uned.es/kos/genre> a owl:NamedIndividual,
        skos:ConceptScheme ;
    skos:definition "Thesaurus about literary genres"@en .

<http://postdata.linhd.uned.es/kos/metrical-type> a owl:NamedIndividual,
        skos:ConceptScheme .

<http://postdata.linhd.uned.es/ontology/postdata-core> a owl:Ontology ;
    ns11:license <https://creativecommons.org/licenses/by/4.0/> ;
    dc:contributor """Aitor Díaz Medina (LINHD_POSTDATA-UNED) 
https://www.linkedin.com/in/aitordiazmedina/""",
        """Alvaro Pérez (LINHD_POSTDATA-UNED) 
https://www.linkedin.com/in/álvaro-pérez-pozo-ab241154/""",
        """Bruno Sartini (Bolonia University)
https://orcid.org/0000-0002-9152-4402""",
        """Helena Bermúdez Sabel
https://orcid.org/0000-0001-7782-206X""",
        """Javier de la Rosa (LINHD_POSTDATA-UNED)
https://www.linkedin.com/in/versae/""",
        """Laura Hernández Lorenzo (LINHD_POSTDATA-UNED) 
https://orcid.org/0000-0003-3489-2193""",
        """Mirella De Sisto (LINHD_POSTDATA-UNED) 
mdesisto@scc.uned.es""",
        """Mª Luisa Díez Platas
https://orcid.org/0000-0002-9416-3147""",
        """Omar Khalil Gómez (LINHD_POSTDATA-UNED) 
http://www.linkedin.com/in/omar-k-0959a8129""",
        """Oscar Corcho (Universidad Politécnica de Madrid)
http://orcid.org/0000-0002-9260-0753""",
        """Salvador Ros Muñoz (UNED)
srosmu@gmail.com""" ;
    dc:creator "POSTDATA Project “This project has received funding from the European Research Council (ERC) under the European Union’s Horizon 2020 research and innovation programme (grant agreement Nº [679528])”"@en ;
    dc:date "2020-02-22" ;
    dc:description "This ontology is the core of the POSTDATA network of ontologies. As such, it contains the most relevant classes and properties that allow representing poetic works and their characteristics. Besides, it contains common classes and properties that are used in many other ontologies in the network, such as those related to the representation of persons, organisations, events, places and roles that persons and organisations play in poetic works."@en ;
    dc:title "POSTDATA core ontology"@en ;
    terms:publisher """POSTDATA Project “This project has received funding from the European Research Council (ERC) under the European Union’s Horizon 2020 research and innovation programme (grant agreement Nº [679528])”
        Principal Investigator. Elena González Blanco -- <https://orcid.org/0000-0002-0448-1812>
        Technical Director. Salvador Ros Muñoz -- <https://orcid.org/0000-0001-6330-4958>"""@en ;
    vann:preferredNamespacePrefix "pdcore" ;
    owl:imports <http://postdata.linhd.uned.es/ontology/postdata-dates#>,
        <http://purl.org/ontology/olo/core#>,
        <http://www.ontologydesignpatterns.org/cp/owl/agentrole.owl>,
        <http://www.ontologydesignpatterns.org/cp/owl/partof.owl> ;
    owl:versionInfo "V1.2" .

<http://postdata.linhd.uned.es/ontology/postdata-core#Organisation> a owl:Class ;
    rdfs:label "Organisation"@en ;
    rdfs:comment """Named collection of people regarded as a single unit. Typical examples include institutions such as ‘UNED’ or ‘the BBC’ and businesses such as ‘Google’ but also racial or ethnic groupings or political factions where these are regarded as forming a single agency such as ‘the Carthaginians’ or ‘the Communists’.
This class is defined as a subclass of pdcore:Agent (which is a subclass of edm:Agent) and foaf:Organization, following the design principles used in the EDM ontology. In the future, it may be also defined as a subclass of schema:Organization, so as to facilitate linking with existing entities already defined according to schema.org."""@en ;
    rdfs:isDefinedBy "http://postdata.linhd.uned.es/ontology/postdata-core/" ;
    rdfs:subClassOf [ a owl:Restriction ;
            owl:allValuesFrom <http://postdata.linhd.uned.es/ontology/postdata-core#Place> ;
            owl:onProperty <http://postdata.linhd.uned.es/ontology/postdata-core#isFrom> ],
        <http://postdata.linhd.uned.es/ontology/postdata-core#Agent>,
        <http://xmlns.com/foaf/0.1/Organization> .

<http://postdata.linhd.uned.es/ontology/postdata-core#certainty> a owl:ObjectProperty ;
    rdfs:label "certainty"@en ;
    rdfs:comment "Certainty"@en,
        "Level of confidence regarding the correspondent function"@en ;
    rdfs:isDefinedBy <http://postdata.linhd.uned.es/ontology/postdata-core>,
        "http://postdata.linhd.uned.es/ontology/postdata-core/" ;
    rdfs:range [ a owl:Restriction ;
            owl:hasValue <http://postdata.linhd.uned.es/kos/certainty> ;
            owl:onProperty skos:inScheme ],
        skos:Concept .

<http://postdata.linhd.uned.es/ontology/postdata-core#isFrom> a owl:ObjectProperty ;
    rdfs:label "is From"@en ;
    rdfs:comment "This property points to the Place which is the provenance of the item"@en ;
    rdfs:isDefinedBy "http://postdata.linhd.uned.es/ontology/postdata-core/" ;
    rdfs:range <http://postdata.linhd.uned.es/ontology/postdata-core#Place> .

<http://postdata.linhd.uned.es/ontology/postdata-core#isTranslationOf> a owl:ObjectProperty ;
    rdfs:label "is Translation Of"@en ;
    rdfs:comment "This property points to another version (an instance of Redaction) of which this one is a translation"@en ;
    rdfs:domain <http://postdata.linhd.uned.es/ontology/postdata-core#Redaction> ;
    rdfs:isDefinedBy "http://postdata.linhd.uned.es/ontology/postdata-core/" ;
    rdfs:range <http://postdata.linhd.uned.es/ontology/postdata-core#Redaction> .

<http://postdata.linhd.uned.es/ontology/postdata-dates#ApproximateDateExpression> a owl:Class ;
    rdfs:label "ApproximateDate"@en ;
    rdfs:comment "Aproximate date expressed in any format, also like a natural language text"@en ;
    rdfs:isDefinedBy "http://postdata.linhd.uned.es/ontology/postdata-dates" ;
    rdfs:subClassOf [ a owl:Restriction ;
            owl:onDataRange xsd:string ;
            owl:onProperty <http://postdata.linhd.uned.es/ontology/postdata-dates#stringContent> ;
            owl:qualifiedCardinality "1"^^xsd:nonNegativeInteger ],
        <http://postdata.linhd.uned.es/ontology/postdata-dates#DateExpression> .

<http://postdata.linhd.uned.es/ontology/postdata-dates#ExactDateExpression> a owl:Class ;
    rdfs:label "ExactDate"@en ;
    rdfs:comment "Exact date"@en ;
    rdfs:isDefinedBy "http://postdata.linhd.uned.es/ontology/postdata-dates" ;
    rdfs:subClassOf [ a owl:Restriction ;
            owl:onDataRange xsd:date ;
            owl:onProperty <http://postdata.linhd.uned.es/ontology/postdata-dates#stringContent> ;
            owl:qualifiedCardinality "1"^^xsd:nonNegativeInteger ],
        <http://postdata.linhd.uned.es/ontology/postdata-dates#DateExpression> .

<http://postdata.linhd.uned.es/ontology/postdata-literaryAnalysisElements#content> a owl:DatatypeProperty ;
    rdfs:label "content"@en ;
    rdfs:comment """Full content of the literary resource. For example, the content of the  acrostic is  the letters that compose it.
En la figura de la palabra, el contenido es una palabra o frase que se utiliza en la figura y que posee un significado separado de su definición literal"""@en ;
    rdfs:isDefinedBy "http://postdata.linhd.uned.es/ontology/postdata-literaryAnalysisElements/"@en ;
    rdfs:range xsd:string .

<http://postdata.linhd.uned.es/ontology/postdata-prosodicElements#Metaplasm> a owl:Class ;
    rdfs:label "Metaplasm"@en ;
    rdfs:comment """A figure of transformation or metaplasm is a figure of diction that consists of altering the writing or pronunciation of words without altering their meaning.
Some examples are dieresis, syneresis, sinalefa or hiatus.
There is a pdprosodic:typeOfMetaplasm property whose range of values is a controlled metaplasm type vocabulary, which allows to specify the nature of it."""@en ;
    rdfs:isDefinedBy "http://postdata.linhd.uned.es/ontology/postdata-prosodicElements"@en .

<http://postdata.linhd.uned.es/ontology/postdata-prosodicElements#RhymeMatch> a owl:Class ;
    rdfs:label "RhymeMatch"@en ;
    rdfs:comment "Entity to define the correspondences between rhyming words"@en ;
    rdfs:isDefinedBy "http://postdata.linhd.uned.es/ontology/postdata-prosodicElements"@en .

<http://postdata.linhd.uned.es/ontology/postdata-prosodicElements#altCountingMetricalScheme> a owl:DatatypeProperty ;
    rdfs:label "altCountingMetricalScheme"@en ;
    dc:creator "mluisadiez" ;
    rdfs:comment "Alternative syllabic/moraic metrical schemae (e.g. long lines with caesura opposite to short lines)" ;
    rdfs:isDefinedBy "http://postdata.linhd.uned.es/ontology/postdata-prosodicElements"@en ;
    rdfs:range xsd:string ;
    rdfs:subPropertyOf owl:topDataProperty .

<http://postdata.linhd.uned.es/ontology/postdata-prosodicElements#altPatterningMetricalScheme> a owl:DatatypeProperty ;
    rdfs:label "altPatterningMetricalScheme"@en ;
    dc:creator "mluisadiez" ;
    rdfs:comment "Distribution of stresses/long syllables, but, for instance, with the addition of punctuation marks to present word boundaries in the line" ;
    rdfs:range xsd:string ;
    rdfs:subPropertyOf owl:topDataProperty .

<http://postdata.linhd.uned.es/ontology/postdata-prosodicElements#countingMetricalScheme> a owl:DatatypeProperty ;
    rdfs:label "countingMetricalScheme"@en ;
    dc:creator "mluisadiez" ;
    dc:date "2018-06-16T18:39:21+00:00"^^xsd:dateTime ;
    rdfs:comment "Metrical scheme according to the number of syllables/morae" ;
    rdfs:isDefinedBy "http://postdata.linhd.uned.es/ontology/postdata-prosodicElements"@en ;
    rdfs:range xsd:string ;
    rdfs:subPropertyOf owl:topDataProperty .

<http://postdata.linhd.uned.es/ontology/postdata-prosodicElements#hasCaesura> a owl:DatatypeProperty ;
    rdfs:label "hasCaesura"@en ;
    dc:creator "mluisadiez" ;
    rdfs:comment "Whether it contains any lines with a pause/break near its middle" ;
    rdfs:isDefinedBy "http://postdata.linhd.uned.es/ontology/postdata-prosodicElements"@en ;
    rdfs:range xsd:boolean ;
    rdfs:subPropertyOf owl:topDataProperty .

<http://postdata.linhd.uned.es/ontology/postdata-prosodicElements#patterningMetricalScheme> a owl:DatatypeProperty ;
    rdfs:label "patterningMetricalScheme"@en ;
    dc:creator "mluisadiez" ;
    dc:date "2018-06-16T18:39:21+00:00"^^xsd:dateTime ;
    rdfs:comment "Metrical scheme for quantitative, tonal, accentual or accentual-syllabic metre" ;
    rdfs:isDefinedBy "http://postdata.linhd.uned.es/ontology/postdata-prosodicElements"@en ;
    rdfs:range xsd:string ;
    rdfs:subPropertyOf owl:topDataProperty .

<http://www.europeana.eu/schemas/edm/Event> a owl:Class ;
    rdfs:label "Event"@en ;
    skos:definition """An event is a change "of states in cultural, social or physical systems,
 regardless of scale, brought about by a series or group of coherent physical,
cultural, technological or legal phenomena" (E5 Event in CIDOC CRM) or a "set of coherent phenomena or cultural manifestations bounded in time and  space" (E4 Period in CIDOC CRM)
"""@en ;
    skos:example "the 2nd World War"@en,
        "the act of painting Mona Lisa"@en,
        "the change of custody of Mona Lisa"@en ;
    skos:note "Events are identified either by the content provider or by Europeana enrichment at ingestion time"@en .

<http://xmlns.com/foaf/0.1/Organization> a owl:Class ;
    rdfs:label "Organization"@en ;
    rdfs:comment "The Organization class represents a kind of Agent corresponding to social institutions such as companies, societies, etc"@en ;
    rdfs:subClassOf [ a owl:Restriction ;
            owl:maxCardinality "1"^^xsd:nonNegativeInteger ;
            owl:onProperty <http://postdata.linhd.uned.es/ontology/postdata-core#address> ] .

<http://postdata.linhd.uned.es/kos/trope-variety> a owl:NamedIndividual,
        skos:ConceptScheme .

<http://postdata.linhd.uned.es/ontology/postdata-core#isMentionedIn> a owl:ObjectProperty ;
    rdfs:label "is Mentioned In"@en ;
    rdfs:comment "This  property points to the text (an instance of Redaction) that records the current item (Event, Place, Organization or Person) under analysis"@en ;
    rdfs:domain [ a owl:Class ;
            owl:unionOf ( <http://postdata.linhd.uned.es/ontology/postdata-core#Event> <http://postdata.linhd.uned.es/ontology/postdata-core#Place> <http://xmlns.com/foaf/0.1/Organization> <http://xmlns.com/foaf/0.1/Person> ) ] ;
    rdfs:isDefinedBy "http://postdata.linhd.uned.es/ontology/postdata-core/" ;
    rdfs:range <http://postdata.linhd.uned.es/ontology/postdata-core#Redaction> ;
    owl:inverseOf <http://postdata.linhd.uned.es/ontology/postdata-core#mentions> .

<http://postdata.linhd.uned.es/ontology/postdata-core#isReferencedIn> a owl:ObjectProperty ;
    rdfs:label "is Referenced In"@en ;
    rdfs:comment "This property points to the specific location in a bibliographic item (an instance of Location) whose contents are related to the current item under analysis (usually, its specific bibliography)"@en ;
    rdfs:domain <http://postdata.linhd.uned.es/ontology/postdata-core#Person> ;
    rdfs:isDefinedBy "http://postdata.linhd.uned.es/ontology/postdata-core/" ;
    rdfs:range <http://postdata.linhd.uned.es/ontology/postdata-transmission#Location> .

<http://postdata.linhd.uned.es/ontology/postdata-dates#DateExpression> a owl:Class ;
    rdfs:label "DateExpression"@en ;
    rdfs:comment "Format or expression mode to represent the date related with the creation or another event asociated witn the entity."@en ;
    rdfs:isDefinedBy "http://postdata.linhd.uned.es/ontology/postdata-dates" ;
    owl:equivalentClass [ a owl:Class ;
            owl:unionOf ( <http://postdata.linhd.uned.es/ontology/postdata-dates#ApproximateDateExpression> <http://postdata.linhd.uned.es/ontology/postdata-dates#ExactDateExpression> <http://postdata.linhd.uned.es/ontology/postdata-dates#IntervalExpression> ) ] .

<http://postdata.linhd.uned.es/ontology/postdata-dates#IntervalExpression> a owl:Class ;
    rdfs:label "Interval"@en ;
    rdfs:isDefinedBy "http://postdata.linhd.uned.es/ontology/postdata-dates" ;
    rdfs:subClassOf <http://postdata.linhd.uned.es/ontology/postdata-dates#DateExpression>,
        <http://www.europeana.eu/schemas/edm/TimeSpan> .

<http://postdata.linhd.uned.es/ontology/postdata-literaryAnalysisElements#figureVariety> a owl:ObjectProperty ;
    rdfs:label "figureCategory"@en ;
    rdfs:comment "Categorisation of the item at hand."@en ;
    rdfs:domain <http://postdata.linhd.uned.es/ontology/postdata-literaryAnalysisElements#FigureOfSpeech> ;
    rdfs:isDefinedBy "http://postdata.linhd.uned.es/ontology/postdata-literaryAnalysisElements/"@en ;
    rdfs:range [ a owl:Restriction ;
            owl:hasValue <http://postdata.linhd.uned.es/kos/trope-variety> ;
            owl:onProperty skos:inScheme ],
        skos:Concept .

<http://postdata.linhd.uned.es/ontology/postdata-prosodicElements#MetricalEncoding> a owl:Class ;
    rdfs:label "MetricalEncoding"@en ;
    dc:creator "mluisadiez" ;
    dc:date "2018-06-16T18:37:24+00:00"^^xsd:dateTime ;
    rdfs:comment """The notation employed to represent a metrical pattern.
Eg.: The definition of the plus sign to encode strong positions."""@en ;
    rdfs:isDefinedBy "http://postdata.linhd.uned.es/ontology/postdata-prosodicElements"@en ;
    rdfs:subClassOf [ a owl:Restriction ;
            owl:maxQualifiedCardinality "1"^^xsd:nonNegativeInteger ;
            owl:onDataRange xsd:string ;
            owl:onProperty <http://postdata.linhd.uned.es/ontology/postdata-prosodicElements#metricalNotes> ] .

<http://postdata.linhd.uned.es/ontology/postdata-prosodicElements#StanzaPattern> a owl:Class ;
    rdfs:label "StanzaPattern"@en ;
    dc:creator "mluisadiez" ;
    dc:date "2018-06-16T18:37:24+00:00"^^xsd:dateTime ;
    rdfs:comment """The prosodic analysis using a Stanza as the unit of reference
Eg.: The number of lines of a Stanza or its categorisation according to metrics (such as “quatrain”)"""@en ;
    rdfs:subClassOf [ a owl:Restriction ;
            owl:maxQualifiedCardinality "1"^^xsd:nonNegativeInteger ;
            owl:onDataRange xsd:string ;
            owl:onProperty <http://postdata.linhd.uned.es/ontology/postdata-prosodicElements#altRhymeScheme> ],
        [ a owl:Restriction ;
            owl:maxQualifiedCardinality "1"^^xsd:nonNegativeInteger ;
            owl:onClass [ a owl:Class ;
                    owl:intersectionOf ( skos:Concept [ a owl:Restriction ;
                                owl:hasValue <http://postdata.linhd.uned.es/kos/metrical-type> ;
                                owl:onProperty skos:inScheme ] ) ] ;
            owl:onProperty <http://postdata.linhd.uned.es/ontology/postdata-prosodicElements#metricalType> ],
        [ a owl:Restriction ;
            owl:maxQualifiedCardinality "1"^^xsd:nonNegativeInteger ;
            owl:onDataRange xsd:boolean ;
            owl:onProperty <http://postdata.linhd.uned.es/ontology/postdata-prosodicElements#hasCaesura> ],
        [ a owl:Restriction ;
            owl:maxQualifiedCardinality "1"^^xsd:nonNegativeInteger ;
            owl:onDataRange xsd:string ;
            owl:onProperty <http://postdata.linhd.uned.es/ontology/postdata-prosodicElements#patterningMetricalScheme> ],
        [ a owl:Restriction ;
            owl:maxQualifiedCardinality "1"^^xsd:nonNegativeInteger ;
            owl:onDataRange xsd:string ;
            owl:onProperty <http://postdata.linhd.uned.es/ontology/postdata-prosodicElements#altPatterningMetricalScheme> ],
        [ a owl:Restriction ;
            owl:maxQualifiedCardinality "1"^^xsd:nonNegativeInteger ;
            owl:onClass [ a owl:Class ;
                    owl:intersectionOf ( skos:Concept [ a owl:Restriction ;
                                owl:hasValue <http://postdata.linhd.uned.es/kos/clausulaScheme-type> ;
                                owl:onProperty skos:inScheme ] ) ] ;
            owl:onProperty <http://postdata.linhd.uned.es/ontology/postdata-prosodicElements#clausulaSchemeType> ],
        [ a owl:Restriction ;
            owl:maxQualifiedCardinality "1"^^xsd:nonNegativeInteger ;
            owl:onClass [ a owl:Class ;
                    owl:intersectionOf ( skos:Concept [ a owl:Restriction ;
                                owl:hasValue <http://postdata.linhd.uned.es/kos/rhymeMatching-type> ;
                                owl:onProperty skos:inScheme ] ) ] ;
            owl:onProperty <http://postdata.linhd.uned.es/ontology/postdata-prosodicElements#presentsRhymeMatching> ],
        [ a owl:Restriction ;
            owl:maxQualifiedCardinality "1"^^xsd:nonNegativeInteger ;
            owl:onClass [ a owl:Class ;
                    owl:intersectionOf ( skos:Concept [ a owl:Restriction ;
                                owl:hasValue <http://postdata.linhd.uned.es/kos/feet-type> ;
                                owl:onProperty skos:inScheme ] ) ] ;
            owl:onProperty <http://postdata.linhd.uned.es/ontology/postdata-prosodicElements#feetType> ],
        [ a owl:Restriction ;
            owl:maxQualifiedCardinality "1"^^xsd:nonNegativeInteger ;
            owl:onDataRange xsd:string ;
            owl:onProperty <http://postdata.linhd.uned.es/ontology/postdata-prosodicElements#rhymeScheme> ],
        [ a owl:Restriction ;
            owl:maxQualifiedCardinality "1"^^xsd:nonNegativeInteger ;
            owl:onDataRange xsd:string ;
            owl:onProperty <http://postdata.linhd.uned.es/ontology/postdata-prosodicElements#metricalNotes> ],
        [ a owl:Restriction ;
            owl:maxQualifiedCardinality "1"^^xsd:nonNegativeInteger ;
            owl:onDataRange xsd:string ;
            owl:onProperty <http://postdata.linhd.uned.es/ontology/postdata-prosodicElements#countingMetricalScheme> ],
        [ a owl:Restriction ;
            owl:maxQualifiedCardinality "1"^^xsd:nonNegativeInteger ;
            owl:onDataRange xsd:string ;
            owl:onProperty <http://postdata.linhd.uned.es/ontology/postdata-prosodicElements#altCountingMetricalScheme> ],
        <http://postdata.linhd.uned.es/ontology/postdata-prosodicElements#Pattern> .

<http://postdata.linhd.uned.es/ontology/postdata-prosodicElements#Symbol> a owl:Class ;
    rdfs:label "Symbol"@en ;
    rdfs:comment "Each element of the notation used to describe a metrical pattern"@en ;
    rdfs:isDefinedBy "http://postdata.linhd.uned.es/ontology/postdata-prosodicElements"@en .

<http://postdata.linhd.uned.es/ontology/postdata-prosodicElements#isAnalysedThrough> a owl:ObjectProperty ;
    dc:creator "mluisadiez" ;
    dc:date "2018-06-16T20:30:43+00:00"^^xsd:dateTime ;
    rdfs:comment "This property points to an item (Pattern) that contains analytical content about the current instance of Redaction, stanzas or lines"@en ;
    rdfs:range <http://postdata.linhd.uned.es/ontology/postdata-prosodicElements#Pattern> ;
    rdfs:subPropertyOf owl:topObjectProperty .

<http://postdata.linhd.uned.es/ontology/postdata-prosodicElements#metricalNotes> a owl:DatatypeProperty ;
    rdfs:label "metricalNotes"@en ;
    dc:creator "mluisadiez" ;
    dc:date "2018-06-16T18:39:21+00:00"^^xsd:dateTime ;
    rdfs:comment "Metrical commentary" ;
    rdfs:isDefinedBy "http://postdata.linhd.uned.es/ontology/postdata-prosodicElements"@en ;
    rdfs:range xsd:string ;
    rdfs:subPropertyOf owl:topDataProperty .

<http://postdata.linhd.uned.es/ontology/postdata-prosodicElements#presentsRhymeMatching> a owl:ObjectProperty ;
    rdfs:label "presentsRhymeMatching"@en ;
    rdfs:comment "Categorisation of the stanza or  work according to the degree in which the different rhyming sounds match (e.g. assonant, consonant...)"@en ;
    rdfs:isDefinedBy "http://postdata.linhd.uned.es/ontology/postdata-prosodicElements"@en ;
    rdfs:range [ a owl:Restriction ;
            owl:hasValue <http://postdata.linhd.uned.es/kos/rhymeMatching-type> ;
            owl:onProperty skos:inScheme ],
        skos:Concept .

<http://postdata.linhd.uned.es/kos/certainty> a owl:NamedIndividual,
        skos:ConceptScheme ;
    skos:definition "Controlled vocabulary about certainty degree"@en .

<http://postdata.linhd.uned.es/ontology/postdata-core#OrderedTextUnitList> a owl:Class ;
    rdfs:label "Ordered Text Unit List"@en ;
    rdfs:comment "An ordered list of text units with a given length and indexed elements. Examples of these lists are the list of stanzas and the list of lines, associated to a Redaction."@en ;
    rdfs:isDefinedBy "http://postdata.linhd.uned.es/ontology/postdata-core/" ;
    rdfs:subClassOf <http://purl.org/ontology/olo/core#OrderedList> .

<http://postdata.linhd.uned.es/ontology/postdata-core#TextUnit> a owl:Class ;
    rdfs:label "Text Unit"@en ;
    rdfs:comment "Text unit of an ordered list. For example, a word, a line or a stanza."@en ;
    rdfs:isDefinedBy "http://postdata.linhd.uned.es/ontology/postdata-core/" ;
    rdfs:subClassOf [ a owl:Restriction ;
            owl:maxQualifiedCardinality "1"^^xsd:nonNegativeInteger ;
            owl:onClass <http://postdata.linhd.uned.es/ontology/postdata-core#OrderedTextUnitList> ;
            owl:onProperty <http://purl.org/ontology/olo/core#ordered_list> ],
        [ a owl:Restriction ;
            owl:maxQualifiedCardinality "1"^^xsd:nonNegativeInteger ;
            owl:onClass <http://postdata.linhd.uned.es/ontology/postdata-core#TextUnit> ;
            owl:onProperty <http://purl.org/ontology/olo/core#next> ],
        [ a owl:Restriction ;
            owl:maxQualifiedCardinality "1"^^xsd:nonNegativeInteger ;
            owl:onClass <http://postdata.linhd.uned.es/ontology/postdata-core#TextUnit> ;
            owl:onProperty <http://purl.org/ontology/olo/core#previous> ],
        <http://purl.org/ontology/olo/core#Slot> .

<http://postdata.linhd.uned.es/ontology/postdata-literaryAnalysisElements#Acrostic> a owl:Class ;
    rdfs:label "Acrostic"@en ;
    rdfs:comment "Grouping of the first letter of each line that form a word, the alphabet or any other message. This class also includes telestichs, that is, the message create it with the last letter of each line"@en ;
    rdfs:isDefinedBy "http://postdata.linhd.uned.es/ontology/postdata-literaryAnalysisElements/"@en ;
    rdfs:subClassOf [ a owl:Restriction ;
            owl:onDataRange xsd:string ;
            owl:onProperty <http://postdata.linhd.uned.es/ontology/postdata-literaryAnalysisElements#content> ;
            owl:qualifiedCardinality "1"^^xsd:nonNegativeInteger ],
        <http://iflastandards.info/ns/fr/frbr/frbroo/F2_Expression> .

<http://postdata.linhd.uned.es/ontology/postdata-structuralElements#content> a owl:DatatypeProperty ;
    rdfs:label "content"@en ;
    dc:creator "mluisadiez" ;
    rdfs:comment "Full content of item" ;
    rdfs:isDefinedBy "http://postdata.linhd.uned.es/ontology/postdata-structuralElements"@en ;
    rdfs:range xsd:string ;
    rdfs:subPropertyOf owl:topDataProperty .

<http://xmlns.com/foaf/0.1/Person> a owl:Class ;
    rdfs:label "Person"@en ;
    rdfs:comment "The Person class represents people. Something is a Person if it is a person. We don't nitpic about whether they're alive, dead, real, or imaginary. The Person class is a sub-class of the Agent class, since all people are considered 'agents' in FOAF."@en .

<http://postdata.linhd.uned.es/kos/rhymeMatching-type> a owl:NamedIndividual,
        skos:ConceptScheme .

<http://postdata.linhd.uned.es/ontology/postdata-core#hasCreator> a owl:ObjectProperty ;
    rdfs:label "has Creator"@en ;
    rdfs:comment "This property points to the entity Creator that has created the current work under analysis"@en ;
    rdfs:domain [ a owl:Class ;
            owl:unionOf ( <http://postdata.linhd.uned.es/ontology/postdata-core#Ensemble> <http://postdata.linhd.uned.es/ontology/postdata-core#PoeticWork> <http://postdata.linhd.uned.es/ontology/postdata-core#Redaction> ) ] ;
    rdfs:isDefinedBy "http://postdata.linhd.uned.es/ontology/postdata-core/" ;
    rdfs:range <http://postdata.linhd.uned.es/ontology/postdata-core#CreatorRole> ;
    rdfs:subPropertyOf <http://www.ontologydesignpatterns.org/cp/owl/objectrole.owl#hasRole> .

xsd:date a rdfs:Datatype .

<http://postdata.linhd.uned.es/ontology/postdata-core#Event> a owl:Class ;
    rdfs:label "Event"@en ;
    rdfs:comment """Something that happens or takes place. It is generally mentioned in the text (Redaction) and represented using isMentionedin property.
This class is defined as a subclass of edm:Event. In the future, it may be also defined as a subclass of schema:Event or bibframe:Event, so as to facilitate linking with existing entities already defined according to schema.org or those available in knowledge graphs such as the one from the US Library of Congress."""@en ;
    rdfs:isDefinedBy "http://postdata.linhd.uned.es/ontology/postdata-core/" ;
    rdfs:subClassOf [ a owl:Restriction ;
            owl:maxCardinality "1"^^xsd:nonNegativeInteger ;
            owl:onProperty <http://postdata.linhd.uned.es/ontology/postdata-core#eventNarration> ],
        [ a owl:Restriction ;
            owl:allValuesFrom <http://postdata.linhd.uned.es/ontology/postdata-core#Redaction> ;
            owl:onProperty <http://postdata.linhd.uned.es/ontology/postdata-core#isMentionedIn> ],
        [ a owl:Restriction ;
            owl:allValuesFrom <http://postdata.linhd.uned.es/ontology/postdata-dates#DateEntity> ;
            owl:onProperty <http://postdata.linhd.uned.es/ontology/postdata-core#date> ],
        <http://www.europeana.eu/schemas/edm/Event> .

<http://postdata.linhd.uned.es/ontology/postdata-core#date> a owl:ObjectProperty ;
    rdfs:label "date"@en ;
    rdfs:comment "This property points to a date entity, which represents a particular point or period of time at which something happened or existed, or is expected to happen"@en ;
    rdfs:domain [ a owl:Class ;
            owl:unionOf ( <http://postdata.linhd.uned.es/ontology/postdata-core#Ensemble> <http://postdata.linhd.uned.es/ontology/postdata-core#Place> <http://postdata.linhd.uned.es/ontology/postdata-core#PoeticWork> <http://postdata.linhd.uned.es/ontology/postdata-core#Redaction> <http://www.europeana.eu/schemas/edm/Event> <http://www.ontologydesignpatterns.org/cp/owl/objectrole.owl#Role> ) ] ;
    rdfs:isDefinedBy "http://postdata.linhd.uned.es/ontology/postdata-core/" ;
    rdfs:range <http://postdata.linhd.uned.es/ontology/postdata-dates#DateEntity> .

<http://postdata.linhd.uned.es/ontology/postdata-prosodicElements#FootDivision> a owl:Class ;
    rdfs:label "FootDivision"@en ;
    dc:creator "mluisadiez" ;
    dc:date "2018-06-16T18:37:24+00:00"^^xsd:dateTime ;
    rdfs:comment "Unit smaller than Foot." .

<http://postdata.linhd.uned.es/ontology/postdata-structuralElements#OrderedLineList> a owl:Class ;
    rdfs:label "OrderedLineList"@en ;
    rdfs:comment "Ordered list of lines  of a redaction"@en ;
    rdfs:isDefinedBy "http://postdata.linhd.uned.es/ontology/postdata-structuralElements"@en ;
    rdfs:subClassOf <http://purl.org/ontology/olo/core#OrderedList> .

<http://postdata.linhd.uned.es/ontology/postdata-core#Agent> a owl:Class ;
    rdfs:label "Agent"@en ;
    rdfs:comment "Any agentive Object , either physical or social. In the context of the POSTDATA ontology network it will mostly refer to organisations or persons"@en ;
    rdfs:isDefinedBy "http://postdata.linhd.uned.es/ontology/postdata-core/" ;
    rdfs:subClassOf [ a owl:Restriction ;
            owl:allValuesFrom <http://postdata.linhd.uned.es/ontology/postdata-core#Redaction> ;
            owl:onProperty <http://postdata.linhd.uned.es/ontology/postdata-core#isMentionedIn> ],
        [ a owl:Restriction ;
            owl:allValuesFrom <http://postdata.linhd.uned.es/ontology/postdata-core#Event> ;
            owl:onProperty <http://postdata.linhd.uned.es/ontology/postdata-core#isInvolvedIn> ],
        [ a owl:Restriction ;
            owl:allValuesFrom <http://postdata.linhd.uned.es/ontology/postdata-core#Role> ;
            owl:onProperty <http://www.ontologydesignpatterns.org/cp/owl/objectrole.owl#hasRole> ],
        <http://www.europeana.eu/schemas/edm/Agent>,
        <http://www.ontologydesignpatterns.org/cp/owl/agentrole.owl#Agent> .

<http://postdata.linhd.uned.es/ontology/postdata-structuralElements#OrderedStanzaList> a owl:Class ;
    rdfs:label "OrderedStanzaList"@en ;
    rdfs:comment "Ordered list of stanzas  of a redaction."@en ;
    rdfs:isDefinedBy "http://postdata.linhd.uned.es/ontology/postdata-structuralElements"@en ;
    rdfs:subClassOf <http://purl.org/ontology/olo/core#OrderedList> .

<http://postdata.linhd.uned.es/ontology/postdata-core#Ensemble> a owl:Class ;
    rdfs:label "Ensemble"@en ;
    rdfs:comment "An abstract work that contains more than one Poetic Work. An Ensemble might be conceived as a collection of works, organized by author, by book song, by book of poems; or as a work mainly written in prose that contains more than one poetic pieces (each one of them being its own Poetic Work). For example, Les fleurs du mal"@en ;
    rdfs:isDefinedBy "http://postdata.linhd.uned.es/ontology/postdata-core/" ;
    rdfs:subClassOf [ a owl:Restriction ;
            owl:allValuesFrom <http://postdata.linhd.uned.es/ontology/postdata-transmission#Location> ;
            owl:onProperty <http://postdata.linhd.uned.es/ontology/postdata-core#isReferencedIn> ],
        [ a owl:Restriction ;
            owl:onProperty <http://postdata.linhd.uned.es/ontology/postdata-core#hasCreator> ;
            owl:someValuesFrom <http://postdata.linhd.uned.es/ontology/postdata-core#CreatorRole> ],
        [ a owl:Class ;
            owl:intersectionOf ( [ a owl:Restriction ;
                        owl:onProperty <http://www.ontologydesignpatterns.org/cp/owl/partof.owl#hasPart> ;
                        owl:someValuesFrom <http://postdata.linhd.uned.es/ontology/postdata-core#PoeticWork> ] [ a owl:Restriction ;
                        owl:allValuesFrom <http://postdata.linhd.uned.es/ontology/postdata-core#PoeticWork> ;
                        owl:onProperty <http://www.ontologydesignpatterns.org/cp/owl/partof.owl#hasPart> ] ) ],
        [ a owl:Restriction ;
            owl:maxQualifiedCardinality "1"^^xsd:nonNegativeInteger ;
            owl:onClass <http://postdata.linhd.uned.es/ontology/postdata-core#Place> ;
            owl:onProperty <http://postdata.linhd.uned.es/ontology/postdata-core#hasProvenance> ],
        [ a owl:Restriction ;
            owl:maxQualifiedCardinality "1"^^xsd:nonNegativeInteger ;
            owl:onDataRange xsd:integer ;
            owl:onProperty <http://postdata.linhd.uned.es/ontology/postdata-core#numberOfLines> ],
        [ a owl:Restriction ;
            owl:allValuesFrom <http://postdata.linhd.uned.es/ontology/postdata-dates#DateEntity> ;
            owl:onProperty <http://postdata.linhd.uned.es/ontology/postdata-core#date> ],
        [ a owl:Restriction ;
            owl:allValuesFrom <http://postdata.linhd.uned.es/ontology/postdata-core#Role> ;
            owl:onProperty <http://www.ontologydesignpatterns.org/cp/owl/objectrole.owl#hasRole> ],
        [ a owl:Restriction ;
            owl:maxQualifiedCardinality "1"^^xsd:nonNegativeInteger ;
            owl:onDataRange xsd:integer ;
            owl:onProperty <http://postdata.linhd.uned.es/ontology/postdata-core#numberOfPlays> ],
        [ a owl:Restriction ;
            owl:maxQualifiedCardinality "1"^^xsd:nonNegativeInteger ;
            owl:onDataRange xsd:integer ;
            owl:onProperty <http://postdata.linhd.uned.es/ontology/postdata-core#numberOfPoems> ],
        [ a owl:Restriction ;
            owl:allValuesFrom <http://postdata.linhd.uned.es/ontology/postdata-core#CreatorRole> ;
            owl:onProperty <http://postdata.linhd.uned.es/ontology/postdata-core#hasCreator> ],
        [ a owl:Restriction ;
            owl:allValuesFrom <http://postdata.linhd.uned.es/ontology/postdata-core#Place> ;
            owl:onProperty <http://postdata.linhd.uned.es/ontology/postdata-core#isFrom> ],
        <http://iflastandards.info/ns/fr/frbr/frbroo/F17> .

<http://postdata.linhd.uned.es/ontology/postdata-core#Role> a owl:Class ;
    rdfs:label "Role"@en ;
    rdfs:comment "This class relates a work (e.g., poetic work, redaction, other transmission elements) and an Agent (Person or Organisation), and allows specifying the role that the agent plays in such work (e.g., creator, sponsor, editor)"@en ;
    rdfs:isDefinedBy "http://postdata.linhd.uned.es/ontology/postdata-core/" ;
    rdfs:subClassOf [ a owl:Restriction ;
            owl:onProperty <http://postdata.linhd.uned.es/ontology/postdata-core#roleFunction> ;
            owl:someValuesFrom [ a owl:Class ;
                    owl:intersectionOf ( skos:Concept [ a owl:Restriction ;
                                owl:hasValue <http://postdata.linhd.uned.es/kos/role-function> ;
                                owl:onProperty skos:inScheme ] ) ] ],
        [ a owl:Restriction ;
            owl:allValuesFrom <http://postdata.linhd.uned.es/ontology/postdata-dates#DateEntity> ;
            owl:onProperty <http://postdata.linhd.uned.es/ontology/postdata-core#date> ],
        [ a owl:Restriction ;
            owl:maxQualifiedCardinality "1"^^xsd:nonNegativeInteger ;
            owl:onClass [ a owl:Class ;
                    owl:intersectionOf ( skos:Concept [ a owl:Restriction ;
                                owl:hasValue <http://postdata.linhd.uned.es/kos/certainty> ;
                                owl:onProperty skos:inScheme ] ) ] ;
            owl:onProperty <http://postdata.linhd.uned.es/ontology/postdata-core#certainty> ],
        [ a owl:Restriction ;
            owl:allValuesFrom [ a owl:Class ;
                    owl:unionOf ( <http://postdata.linhd.uned.es/ontology/postdata-core#Agent> <http://postdata.linhd.uned.es/ontology/postdata-core#Ensemble> <http://postdata.linhd.uned.es/ontology/postdata-core#PoeticWork> <http://postdata.linhd.uned.es/ontology/postdata-core#Redaction> ) ] ;
            owl:onProperty <http://www.ontologydesignpatterns.org/cp/owl/objectrole.owl#isRoleOf> ],
        <http://www.ontologydesignpatterns.org/cp/owl/objectrole.owl#Role> .

<http://postdata.linhd.uned.es/ontology/postdata-prosodicElements#Pattern> a owl:Class .

<http://postdata.linhd.uned.es/ontology/postdata-core#CreatorRole> a owl:Class ;
    rdfs:label "Creator Role"@en ;
    rdfs:comment """The CreatorRole class models the role that an agent plays with respect to the creation or authorship of a work. In this sense, it has specific properties that are important for the study of authorship of poetic works.
These properties are:
penName - It is common for authors to use an alias
isAnonymous - In many of the works, especially the older ones, the author is not known and this is an aspect that should be considered.
isWrongAttribution - Sometimes, especially in older works as well, attributions of authorship have been made that are not correct, but this fact is considered an important aspect for scholars of the subject.
typeofDesignation, which is the type of name or designation used, e.g. pseudonyms, heteronyms, etc."""@en ;
    rdfs:isDefinedBy "http://postdata.linhd.uned.es/ontology/postdata-core/" ;
    rdfs:subClassOf [ a owl:Restriction ;
            owl:maxQualifiedCardinality "1"^^xsd:nonNegativeInteger ;
            owl:onClass [ a owl:Class ;
                    owl:intersectionOf ( skos:Concept [ a owl:Restriction ;
                                owl:hasValue <http://postdata.linhd.uned.es/kos/certainty> ;
                                owl:onProperty skos:inScheme ] ) ] ;
            owl:onProperty <http://postdata.linhd.uned.es/ontology/postdata-core#certainty> ],
        [ a owl:Restriction ;
            owl:maxQualifiedCardinality "1"^^xsd:nonNegativeInteger ;
            owl:onDataRange xsd:string ;
            owl:onProperty <http://postdata.linhd.uned.es/ontology/postdata-core#penName> ],
        [ a owl:Restriction ;
            owl:maxQualifiedCardinality "1"^^xsd:nonNegativeInteger ;
            owl:onClass [ a owl:Class ;
                    owl:intersectionOf ( skos:Concept [ a owl:Restriction ;
                                owl:hasValue <http://postdata.linhd.uned.es/kos/designation-type> ;
                                owl:onProperty skos:inScheme ] ) ] ;
            owl:onProperty <http://postdata.linhd.uned.es/ontology/postdata-core#typeOfDesignation> ],
        <http://postdata.linhd.uned.es/ontology/postdata-core#Role> .

<http://postdata.linhd.uned.es/ontology/postdata-literaryAnalysisElements#FigureOfSpeech> a owl:Class ;
    rdfs:label "FigureOfSpeech"@en ;
    dc:creator "M Luisa Diez"@en ;
    rdfs:comment "A word or phrase used in a non-literal sense for rhetorical or vivid effect"@en ;
    rdfs:isDefinedBy "http://postdata.linhd.uned.es/ontology/postdata-literaryAnalysisElements/"@en ;
    rdfs:subClassOf [ a owl:Restriction ;
            owl:onClass [ a owl:Class ;
                    owl:intersectionOf ( skos:Concept [ a owl:Restriction ;
                                owl:hasValue <http://postdata.linhd.uned.es/kos/trope-variety> ;
                                owl:onProperty skos:inScheme ] ) ] ;
            owl:onProperty <http://postdata.linhd.uned.es/ontology/postdata-literaryAnalysisElements#figureVariety> ;
            owl:qualifiedCardinality "1"^^xsd:nonNegativeInteger ],
        [ a owl:Restriction ;
            owl:maxQualifiedCardinality "1"^^xsd:nonNegativeInteger ;
            owl:onDataRange xsd:string ;
            owl:onProperty <http://postdata.linhd.uned.es/ontology/postdata-literaryAnalysisElements#figureReferent> ],
        [ a owl:Restriction ;
            owl:maxQualifiedCardinality "1"^^xsd:nonNegativeInteger ;
            owl:onDataRange xsd:string ;
            owl:onProperty <http://postdata.linhd.uned.es/ontology/postdata-literaryAnalysisElements#figureMeaning> ],
        [ a owl:Restriction ;
            owl:allValuesFrom [ a owl:Class ;
                    owl:intersectionOf ( skos:Concept [ a owl:Restriction ;
                                owl:hasValue <http://postdata.linhd.uned.es/kos/trope-variety> ;
                                owl:onProperty skos:inScheme ] ) ] ;
            owl:onProperty <http://postdata.linhd.uned.es/ontology/postdata-literaryAnalysisElements#figureVariety> ],
        <http://bakulf.github.io/raop/0.1#RethoricalDevice> .

<http://postdata.linhd.uned.es/ontology/postdata-literaryAnalysisElements#Intertextuality> a owl:Class ;
    rdfs:label "Intertextuality"@en ;
    dc:creator "mluisadiez" ;
    dc:date "2018-06-16T18:37:24+00:00"^^xsd:dateTime ;
    rdfs:comment "Shared textual materials between two or more contemporary texts; Text from which information or ideas are derived for the composition of the Opus/Redaction;Text that took information or ideas from the Opus/Redaction" ;
    rdfs:subClassOf [ a owl:Restriction ;
            owl:cardinality "1"^^xsd:nonNegativeInteger ;
            owl:onProperty dc:title ],
        [ a owl:Restriction ;
            owl:maxQualifiedCardinality "1"^^xsd:nonNegativeInteger ;
            owl:onDataRange xsd:string ;
            owl:onProperty <http://postdata.linhd.uned.es/ontology/postdata-literaryAnalysisElements#referenceLocation> ],
        [ a owl:Restriction ;
            owl:maxQualifiedCardinality "1"^^xsd:nonNegativeInteger ;
            owl:onDataRange xsd:string ;
            owl:onProperty <http://postdata.linhd.uned.es/ontology/postdata-literaryAnalysisElements#reference> ],
        <http://iflastandards.info/ns/fr/frbr/frbroo/F2_Expression> .

<http://postdata.linhd.uned.es/ontology/postdata-prosodicElements#WorkPattern> a owl:Class ;
    rdfs:label "WorkPattern"@en ;
    dc:creator "mluisadiez" ;
    dc:date "2018-06-16T18:37:24+00:00"^^xsd:dateTime ;
    rdfs:comment """The prosodic analysis using a Redaction as the unit of reference
Eg.: The complete distribution of accented syllables of a work"""@en ;
    rdfs:subClassOf [ a owl:Restriction ;
            owl:maxQualifiedCardinality "1"^^xsd:nonNegativeInteger ;
            owl:onDataRange xsd:string ;
            owl:onProperty <http://postdata.linhd.uned.es/ontology/postdata-prosodicElements#grammaticalStressPattern> ],
        [ a owl:Restriction ;
            owl:maxQualifiedCardinality "1"^^xsd:nonNegativeInteger ;
            owl:onDataRange xsd:string ;
            owl:onProperty <http://postdata.linhd.uned.es/ontology/postdata-prosodicElements#altRhymeScheme> ],
        [ a owl:Restriction ;
            owl:maxQualifiedCardinality "1"^^xsd:nonNegativeInteger ;
            owl:onDataRange xsd:string ;
            owl:onProperty <http://postdata.linhd.uned.es/ontology/postdata-prosodicElements#altCountingMetricalScheme> ],
        [ a owl:Restriction ;
            owl:maxQualifiedCardinality "1"^^xsd:nonNegativeInteger ;
            owl:onClass [ a owl:Class ;
                    owl:intersectionOf ( skos:Concept [ a owl:Restriction ;
                                owl:hasValue <http://postdata.linhd.uned.es/kos/metrical-type> ;
                                owl:onProperty skos:inScheme ] ) ] ;
            owl:onProperty <http://postdata.linhd.uned.es/ontology/postdata-prosodicElements#metricalType> ],
        [ a owl:Restriction ;
            owl:maxQualifiedCardinality "1"^^xsd:nonNegativeInteger ;
            owl:onDataRange xsd:string ;
            owl:onProperty <http://postdata.linhd.uned.es/ontology/postdata-prosodicElements#patterningMetricalScheme> ],
        [ a owl:Restriction ;
            owl:maxQualifiedCardinality "1"^^xsd:nonNegativeInteger ;
            owl:onDataRange xsd:string ;
            owl:onProperty <http://postdata.linhd.uned.es/ontology/postdata-prosodicElements#altPatterningMetricalScheme> ],
        [ a owl:Restriction ;
            owl:maxQualifiedCardinality "1"^^xsd:nonNegativeInteger ;
            owl:onClass [ a owl:Class ;
                    owl:intersectionOf ( skos:Concept [ a owl:Restriction ;
                                owl:hasValue <http://postdata.linhd.uned.es/kos/rhymeMatching-type> ;
                                owl:onProperty skos:inScheme ] ) ] ;
            owl:onProperty <http://postdata.linhd.uned.es/ontology/postdata-prosodicElements#presentsRhymeMatching> ],
        [ a owl:Restriction ;
            owl:maxQualifiedCardinality "1"^^xsd:nonNegativeInteger ;
            owl:onDataRange xsd:boolean ;
            owl:onProperty <http://postdata.linhd.uned.es/ontology/postdata-prosodicElements#hasCaesura> ],
        [ a owl:Restriction ;
            owl:maxQualifiedCardinality "1"^^xsd:nonNegativeInteger ;
            owl:onDataRange xsd:string ;
            owl:onProperty <http://postdata.linhd.uned.es/ontology/postdata-prosodicElements#metricalNotes> ],
        [ a owl:Restriction ;
            owl:maxQualifiedCardinality "1"^^xsd:nonNegativeInteger ;
            owl:onDataRange xsd:string ;
            owl:onProperty <http://postdata.linhd.uned.es/ontology/postdata-prosodicElements#countingMetricalScheme> ],
        [ a owl:Restriction ;
            owl:maxQualifiedCardinality "1"^^xsd:nonNegativeInteger ;
            owl:onDataRange xsd:string ;
            owl:onProperty <http://postdata.linhd.uned.es/ontology/postdata-prosodicElements#rhymeScheme> ],
        [ a owl:Restriction ;
            owl:maxQualifiedCardinality "1"^^xsd:nonNegativeInteger ;
            owl:onDataRange xsd:string ;
            owl:onProperty <http://postdata.linhd.uned.es/ontology/postdata-core#notes> ],
        [ a owl:Restriction ;
            owl:maxQualifiedCardinality "1"^^xsd:nonNegativeInteger ;
            owl:onDataRange xsd:boolean ;
            owl:onProperty <http://postdata.linhd.uned.es/ontology/postdata-prosodicElements#hasAnacrusis> ],
        <http://postdata.linhd.uned.es/ontology/postdata-prosodicElements#Pattern> .

<http://postdata.linhd.uned.es/ontology/postdata-structuralElements#Token> a owl:Class ;
    rdfs:label "Token"@en ;
    rdfs:comment "A lexical element"@en ;
    rdfs:isDefinedBy "http://postdata.linhd.uned.es/ontology/postdata-structuralElements"@en .

<http://postdata.linhd.uned.es/ontology/postdata-transmission#Location> a owl:Class .

<http://postdata.linhd.uned.es/ontology/postdata-prosodicElements#Rhyme> a owl:Class ;
    rdfs:label "Rhyme"@en ;
    dc:creator "mluisadiez"@en ;
    rdfs:comment "Repetition of similar sounding words occurring at the end of lines in poems or songs"@en .

<http://postdata.linhd.uned.es/ontology/postdata-dates#DateEntity> a owl:Class ;
    rdfs:label "DateEntity"@en ;
    rdfs:comment "The temporal entity asociated to an opus, manifestation, event.." ;
    rdfs:isDefinedBy "http://postdata.linhd.uned.es/ontology/postdata-dates" .

<http://postdata.linhd.uned.es/ontology/postdata-structuralElements#Syllable> a owl:Class ;
    rdfs:label "Syllable"@en ;
    dc:creator "mluisadiez" ;
    rdfs:comment """A single unit of speech sound as written or spoken; specifically, a vowel preceded by zero to three consonants (“awl,” “bring,” “strand”), and followed by zero to four consonants (“too,” “brag,” “gloss,” “stings,” “sixths”).
It is the reference unit of a literary analysis, in some poetic tradicions
Eg.: The onset and coda of the rhyme vowel""",
        "As a structure, a Syllable is an item (a subclass of old:slot) of a Word"@en ;
    rdfs:isDefinedBy "http://postdata.linhd.uned.es/ontology/postdata-structuralElements" ;
    rdfs:subClassOf [ a owl:Restriction ;
            owl:onDataRange xsd:string ;
            owl:onProperty <http://postdata.linhd.uned.es/ontology/postdata-structuralElements#content> ;
            owl:qualifiedCardinality "1"^^xsd:nonNegativeInteger ],
        [ a owl:Restriction ;
            owl:maxQualifiedCardinality "1"^^xsd:nonNegativeInteger ;
            owl:onDataRange xsd:boolean ;
            owl:onProperty <http://postdata.linhd.uned.es/ontology/postdata-structuralElements#isRefrain> ],
        [ a owl:Restriction ;
            owl:maxQualifiedCardinality "1"^^xsd:nonNegativeInteger ;
            owl:onDataRange xsd:string ;
            owl:onProperty <http://postdata.linhd.uned.es/ontology/postdata-structuralElements#lineNumber> ],
        <http://purl.org/ontology/olo/core#Slot>,
        owl:Thing .

<http://postdata.linhd.uned.es/ontology/postdata-prosodicElements#LinePattern> a owl:Class ;
    rdfs:label "LinePattern"@en ;
    dc:creator "mluisadiez" ;
    dc:date "2018-06-16T18:37:24+00:00"^^xsd:dateTime ;
    rdfs:comment """The prosodic analysis using a Line as the unit of reference
Eg.: The number of syllables of the Line"""@en ;
    rdfs:subClassOf [ a owl:Restriction ;
            owl:maxQualifiedCardinality "1"^^xsd:nonNegativeInteger ;
            owl:onDataRange xsd:boolean ;
            owl:onProperty <http://postdata.linhd.uned.es/ontology/postdata-prosodicElements#hasAnacrusis> ],
        [ a owl:Restriction ;
            owl:maxQualifiedCardinality "1"^^xsd:nonNegativeInteger ;
            owl:onDataRange xsd:string ;
            owl:onProperty <http://postdata.linhd.uned.es/ontology/postdata-prosodicElements#accentedVowels> ],
        [ a owl:Restriction ;
            owl:maxQualifiedCardinality "1"^^xsd:nonNegativeInteger ;
            owl:onDataRange xsd:string ;
            owl:onProperty <http://postdata.linhd.uned.es/ontology/postdata-prosodicElements#altCountingMetricalScheme> ],
        [ a owl:Restriction ;
            owl:maxQualifiedCardinality "1"^^xsd:nonNegativeInteger ;
            owl:onDataRange xsd:string ;
            owl:onProperty <http://postdata.linhd.uned.es/ontology/postdata-prosodicElements#patterningMetricalScheme> ],
        [ a owl:Restriction ;
            owl:maxQualifiedCardinality "1"^^xsd:nonNegativeInteger ;
            owl:onDataRange xsd:string ;
            owl:onProperty <http://postdata.linhd.uned.es/ontology/postdata-prosodicElements#altPatterningMetricalScheme> ],
        [ a owl:Restriction ;
            owl:maxQualifiedCardinality "1"^^xsd:nonNegativeInteger ;
            owl:onDataRange xsd:string ;
            owl:onProperty <http://postdata.linhd.uned.es/ontology/postdata-prosodicElements#metricalNotes> ],
        [ a owl:Restriction ;
            owl:maxQualifiedCardinality "1"^^xsd:nonNegativeInteger ;
            owl:onDataRange xsd:boolean ;
            owl:onProperty <http://postdata.linhd.uned.es/ontology/postdata-prosodicElements#hasCaesura> ],
        [ a owl:Restriction ;
            owl:maxQualifiedCardinality "1"^^xsd:nonNegativeInteger ;
            owl:onDataRange xsd:string ;
            owl:onProperty <http://postdata.linhd.uned.es/ontology/postdata-prosodicElements#grammaticalStressPattern> ],
        [ a owl:Restriction ;
            owl:maxQualifiedCardinality "1"^^xsd:nonNegativeInteger ;
            owl:onClass [ a owl:Class ;
                    owl:intersectionOf ( skos:Concept [ a owl:Restriction ;
                                owl:hasValue <http://postdata.linhd.uned.es/kos/feet-type> ;
                                owl:onProperty skos:inScheme ] ) ] ;
            owl:onProperty <http://postdata.linhd.uned.es/ontology/postdata-prosodicElements#feetType> ],
        [ a owl:Restriction ;
            owl:maxQualifiedCardinality "1"^^xsd:nonNegativeInteger ;
            owl:onDataRange xsd:string ;
            owl:onProperty <http://postdata.linhd.uned.es/ontology/postdata-prosodicElements#countingMetricalScheme> ],
        <http://postdata.linhd.uned.es/ontology/postdata-prosodicElements#Pattern> .

<http://postdata.linhd.uned.es/ontology/postdata-prosodicElements#Foot> a owl:Class ;
    rdfs:label "Foot"@en ;
    dc:creator "mluisadiez" ;
    dc:date "2018-06-16T18:37:24+00:00"^^xsd:dateTime ;
    rdfs:comment "A unit of poetic meter consisting of stressed and unstressed syllables or long and short syllables in any of various set combinations"@en ;
    rdfs:subClassOf [ a owl:Restriction ;
            owl:maxQualifiedCardinality "1"^^xsd:nonNegativeInteger ;
            owl:onClass [ a owl:Class ;
                    owl:intersectionOf ( skos:Concept [ a owl:Restriction ;
                                owl:hasValue <http://postdata.linhd.uned.es/kos/clausula> ;
                                owl:onProperty skos:inScheme ] ) ] ;
            owl:onProperty <http://postdata.linhd.uned.es/ontology/postdata-prosodicElements#clausula> ],
        <http://purl.org/linguistics/gold/Foot> .

<http://postdata.linhd.uned.es/ontology/postdata-core#Place> a owl:Class ;
    rdfs:label "Place"@en ;
    rdfs:comment """A particular position, point, or area in space; a location
This class is defined as a subclass of edm:Place. In the future, it may be also defined as a subclass of schema:Place and geonames:Feature, so as to facilitate linking with existing entities already defined according to schema.org or available in the GeoNames knowledge graph."""@en ;
    rdfs:isDefinedBy "http://postdata.linhd.uned.es/ontology/postdata-core/" ;
    rdfs:subClassOf [ a owl:Restriction ;
            owl:allValuesFrom <http://postdata.linhd.uned.es/ontology/postdata-dates#DateEntity> ;
            owl:onProperty <http://postdata.linhd.uned.es/ontology/postdata-core#date> ],
        [ a owl:Restriction ;
            owl:allValuesFrom <http://postdata.linhd.uned.es/ontology/postdata-core#Redaction> ;
            owl:onProperty <http://postdata.linhd.uned.es/ontology/postdata-core#isMentionedIn> ],
        [ a owl:Restriction ;
            owl:maxQualifiedCardinality "1"^^xsd:nonNegativeInteger ;
            owl:onDataRange xsd:string ;
            owl:onProperty <http://postdata.linhd.uned.es/ontology/postdata-core#originalName> ],
        <http://www.europeana.eu/schemas/edm/Place> .

owl:topObjectProperty rdfs:domain owl:Thing .

<http://postdata.linhd.uned.es/ontology/postdata-structuralElements#Stanza> a owl:Class ;
    rdfs:label "Stanza"@en ;
    rdfs:comment """Group of lines. Usually, this grouping forms the basic recurring metrical unit of a poem, song or play
Eg.: As armas e os barões assinalados,
Que da ocidental praia Lusitana,
Por mares nunca de antes navegados,
Passaram ainda além da Taprobana,
Em perigos e guerras esforçados,
Mais do que prometia a força humana,
E entre gente remota edificaram
Novo Reino, que tanto sublimaram;""",
        """As a structure, a Stanza can be modelled from two points of view:
- An item (a subclass of old:slot) of the list of Stanzas of the Redaction 
- A list of lines"""@en ;
    rdfs:isDefinedBy "http://postdata.linhd.uned.es/ontology/postdata-structuralElements"@en ;
    rdfs:subClassOf [ a owl:Restriction ;
            owl:onClass <http://postdata.linhd.uned.es/ontology/postdata-structuralElements#Line> ;
            owl:onProperty <http://postdata.linhd.uned.es/ontology/postdata-structuralElements#hasFirstLine> ;
            owl:qualifiedCardinality "1"^^xsd:nonNegativeInteger ],
        [ a owl:Restriction ;
            owl:maxQualifiedCardinality "1"^^xsd:nonNegativeInteger ;
            owl:onClass [ a owl:Class ;
                    owl:intersectionOf ( skos:Concept [ a owl:Restriction ;
                                owl:hasValue <http://postdata.linhd.uned.es/kos/rhymeMatching-type> ;
                                owl:onProperty skos:inScheme ] ) ] ;
            owl:onProperty <http://postdata.linhd.uned.es/ontology/postdata-prosodicElements#presentsRhymeMatching> ],
        [ a owl:Restriction ;
            owl:onClass <http://postdata.linhd.uned.es/ontology/postdata-structuralElements#Line> ;
            owl:onProperty <http://postdata.linhd.uned.es/ontology/postdata-structuralElements#hasLastLine> ;
            owl:qualifiedCardinality "1"^^xsd:nonNegativeInteger ],
        [ a owl:Restriction ;
            owl:maxQualifiedCardinality "1"^^xsd:nonNegativeInteger ;
            owl:onDataRange xsd:string ;
            owl:onProperty <http://postdata.linhd.uned.es/ontology/postdata-structuralElements#content> ],
        [ a owl:Restriction ;
            owl:maxQualifiedCardinality "1"^^xsd:nonNegativeInteger ;
            owl:onDataRange xsd:string ;
            owl:onProperty <http://postdata.linhd.uned.es/ontology/postdata-structuralElements#paraphrasis> ],
        [ a owl:Restriction ;
            owl:maxQualifiedCardinality "1"^^xsd:nonNegativeInteger ;
            owl:onClass <http://postdata.linhd.uned.es/ontology/postdata-prosodicElements#Pattern> ;
            owl:onProperty <http://postdata.linhd.uned.es/ontology/postdata-prosodicElements#isAnalysedThrough> ],
        [ a owl:Restriction ;
            owl:maxQualifiedCardinality "1"^^xsd:nonNegativeInteger ;
            owl:onDataRange xsd:string ;
            owl:onProperty <http://postdata.linhd.uned.es/ontology/postdata-structuralElements#altStanzaNumber> ],
        <http://purl.org/ontology/olo/core#OrderedList>,
        <http://purl.org/ontology/olo/core#Slot>,
        owl:Thing .

<http://postdata.linhd.uned.es/ontology/postdata-structuralElements#Word> a owl:Class ;
    rdfs:label "Word"@en ;
    dc:creator "mluisadiez" ;
    rdfs:comment """A single distinct meaningful element of writing, used with others (or sometimes alone) to form a sentence and typically shown with a space on either side when written or printed
Eg.: The word “life”"""@en,
        """As a structure, a Word can be modelled from two points of view:
- An item (a subclass of old:slot) of the Line 
- A list of Syllables"""@en ;
    rdfs:isDefinedBy "http://postdata.linhd.uned.es/ontology/postdata-structuralElements" ;
    rdfs:subClassOf [ a owl:Restriction ;
            owl:maxQualifiedCardinality "1"^^xsd:nonNegativeInteger ;
            owl:onDataRange xsd:string ;
            owl:onProperty <http://postdata.linhd.uned.es/ontology/postdata-structuralElements#lemma> ],
        [ a owl:Restriction ;
            owl:maxQualifiedCardinality "1"^^xsd:nonNegativeInteger ;
            owl:onClass <http://postdata.linhd.uned.es/ontology/postdata-structuralElements#Word> ;
            owl:onProperty <http://postdata.linhd.uned.es/ontology/postdata-structuralElements#isInflectedForm> ],
        [ a owl:Restriction ;
            owl:maxQualifiedCardinality "1"^^xsd:nonNegativeInteger ;
            owl:onDataRange xsd:string ;
            owl:onProperty <http://postdata.linhd.uned.es/ontology/postdata-structuralElements#phoneticTranscription> ],
        [ a owl:Restriction ;
            owl:maxQualifiedCardinality "1"^^xsd:nonNegativeInteger ;
            owl:onDataRange xsd:string ;
            owl:onProperty <http://postdata.linhd.uned.es/ontology/postdata-structuralElements#morphologicalAnnotation> ],
        [ a owl:Restriction ;
            owl:onDataRange xsd:string ;
            owl:onProperty <http://postdata.linhd.uned.es/ontology/postdata-structuralElements#content> ;
            owl:qualifiedCardinality "1"^^xsd:nonNegativeInteger ],
        <http://bakulf.github.io/raop/0.1#Word>,
        <http://postdata.linhd.uned.es/ontology/postdata-structuralElements#Token>,
        <http://purl.org/ontology/olo/core#OrderedList>,
        <http://purl.org/ontology/olo/core#Slot> .

<http://postdata.linhd.uned.es/ontology/postdata-core#PoeticWork> a owl:Class ;
    rdfs:label "Poetic Work"@en ;
    rdfs:comment "Abstract concept of an artistic creation. In the POSTDATA ontology network these creations must be in verse (e.g., poem, play, song). For example, Os Lusíadas by Luis Vaz de Camões; La Commedia by Dante; the poem Ad te deus by an Anonymous author written in between the 7th and 9th centuries."@en ;
    rdfs:isDefinedBy "http://postdata.linhd.uned.es/ontology/postdata-core/" ;
    rdfs:subClassOf [ a owl:Restriction ;
            owl:onClass <http://postdata.linhd.uned.es/ontology/postdata-dates#DateEntity> ;
            owl:onProperty <http://postdata.linhd.uned.es/ontology/postdata-core#date> ;
            owl:qualifiedCardinality "1"^^xsd:nonNegativeInteger ],
        [ a owl:Restriction ;
            owl:allValuesFrom <http://postdata.linhd.uned.es/ontology/postdata-core#Ensemble> ;
            owl:onProperty <http://www.ontologydesignpatterns.org/cp/owl/partof.owl#isPartOf> ],
        [ a owl:Restriction ;
            owl:maxQualifiedCardinality "1"^^xsd:nonNegativeInteger ;
            owl:onClass <http://postdata.linhd.uned.es/ontology/postdata-core#Place> ;
            owl:onProperty <http://postdata.linhd.uned.es/ontology/postdata-core#hasProvenance> ],
        [ a owl:Restriction ;
            owl:allValuesFrom <http://postdata.linhd.uned.es/ontology/postdata-dates#DateEntity> ;
            owl:onProperty <http://postdata.linhd.uned.es/ontology/postdata-core#date> ],
        [ a owl:Restriction ;
            owl:maxQualifiedCardinality "1"^^xsd:nonNegativeInteger ;
            owl:onClass [ a owl:Class ;
                    owl:intersectionOf ( skos:Concept [ a owl:Restriction ;
                                owl:hasValue <http://postdata.linhd.uned.es/kos/poetic-type> ;
                                owl:onProperty skos:inScheme ] ) ] ;
            owl:onProperty <http://postdata.linhd.uned.es/ontology/postdata-core#poeticType> ],
        [ a owl:Restriction ;
            owl:maxQualifiedCardinality "1"^^xsd:nonNegativeInteger ;
            owl:onClass [ a owl:Class ;
                    owl:intersectionOf ( skos:Concept [ a owl:Restriction ;
                                owl:hasValue <http://postdata.linhd.uned.es/kos/genre> ;
                                owl:onProperty skos:inScheme ] ) ] ;
            owl:onProperty <http://postdata.linhd.uned.es/ontology/postdata-core#genre> ],
        [ a owl:Restriction ;
            owl:allValuesFrom <http://postdata.linhd.uned.es/ontology/postdata-core#Role> ;
            owl:onProperty <http://www.ontologydesignpatterns.org/cp/owl/objectrole.owl#hasRole> ],
        [ a owl:Restriction ;
            owl:maxQualifiedCardinality "1"^^xsd:nonNegativeInteger ;
            owl:onDataRange xsd:string ;
            owl:onProperty <http://postdata.linhd.uned.es/ontology/postdata-core#narrativeLocation> ],
        [ a owl:Restriction ;
            owl:allValuesFrom <http://postdata.linhd.uned.es/ontology/postdata-transmission#Location> ;
            owl:onProperty <http://postdata.linhd.uned.es/ontology/postdata-core#isReferencedIn> ],
        [ a owl:Restriction ;
            owl:onProperty <http://postdata.linhd.uned.es/ontology/postdata-core#hasCreator> ;
            owl:someValuesFrom <http://postdata.linhd.uned.es/ontology/postdata-core#CreatorRole> ],
        [ a owl:Restriction ;
            owl:maxQualifiedCardinality "1"^^xsd:nonNegativeInteger ;
            owl:onDataRange xsd:string ;
            owl:onProperty <http://postdata.linhd.uned.es/ontology/postdata-core#originalTitle> ],
        [ a owl:Restriction ;
            owl:allValuesFrom <http://postdata.linhd.uned.es/ontology/postdata-core#CreatorRole> ;
            owl:onProperty <http://postdata.linhd.uned.es/ontology/postdata-core#hasCreator> ],
        [ a owl:Restriction ;
            owl:maxQualifiedCardinality "1"^^xsd:nonNegativeInteger ;
            owl:onClass [ a owl:Class ;
                    owl:intersectionOf ( skos:Concept [ a owl:Restriction ;
                                owl:hasValue <http://postdata.linhd.uned.es/kos/author-education-level> ;
                                owl:onProperty skos:inScheme ] ) ] ;
            owl:onProperty <http://postdata.linhd.uned.es/ontology/postdata-core#authorEducationLevel> ],
        <http://iflastandards.info/ns/fr/frbr/frbroo/F1>,
        <http://www.europeana.eu/schemas/edm/ProvidedCHO> .

<http://postdata.linhd.uned.es/ontology/postdata-structuralElements#Line> a owl:Class ;
    rdfs:label "Line"@en ;
    dc:creator "mluisadiez" ;
    rdfs:comment """A unit of verse that usually ends in a visual or typographic break and generally characterized by its length and meter
Eg.: “As armas e os barões assinalados” - from Os Lusíadas""",
        """As a structure, a List can be modelled from two points of view:
- An item (a subclass of old:slot) of the list of lines of the Redaction 
- A list of tokens"""@en ;
    rdfs:isDefinedBy "http://postdata.linhd.uned.es/ontology/postdata-structuralElements" ;
    rdfs:subClassOf [ a owl:Restriction ;
            owl:maxQualifiedCardinality "1"^^xsd:nonNegativeInteger ;
            owl:onClass <http://postdata.linhd.uned.es/ontology/postdata-prosodicElements#LinePattern> ;
            owl:onProperty <http://postdata.linhd.uned.es/ontology/postdata-prosodicElements#isAnalysedThrough> ],
        [ a owl:Restriction ;
            owl:maxQualifiedCardinality "1"^^xsd:nonNegativeInteger ;
            owl:onDataRange xsd:boolean ;
            owl:onProperty <http://postdata.linhd.uned.es/ontology/postdata-structuralElements#isRefrain> ],
        [ a owl:Restriction ;
            owl:maxQualifiedCardinality "1"^^xsd:nonNegativeInteger ;
            owl:onDataRange xsd:string ;
            owl:onProperty <http://postdata.linhd.uned.es/ontology/postdata-structuralElements#content> ],
        [ a owl:Restriction ;
            owl:maxQualifiedCardinality "1"^^xsd:nonNegativeInteger ;
            owl:onDataRange xsd:string ;
            owl:onProperty <http://postdata.linhd.uned.es/ontology/postdata-structuralElements#lineNumber> ],
        <http://purl.org/ontology/olo/core#OrderedList>,
        <http://purl.org/ontology/olo/core#Slot>,
        owl:Thing .

skos:ConceptScheme a owl:Class .

<http://postdata.linhd.uned.es/ontology/postdata-core#Person> a owl:Class ;
    rdfs:label "Person"@en ;
    rdfs:comment """A human being regarded as an individual. This person may have existed in real life (e.g., Miguel de Cervantes) or may be fictional (e.g., Don Quijote de la Mancha).
This class is defined as a subclass of pdcore:Agent (which is a subclass of edm:Agent) and foaf:Person, following the design principles used in the EDM ontology. In the future, it may be also defined as a subclass of schema:Person, so as to facilitate linking with existing entities already defined according to schema.org"""@en ;
    rdfs:isDefinedBy "http://postdata.linhd.uned.es/ontology/postdata-core/" ;
    rdfs:subClassOf [ a owl:Restriction ;
            owl:maxQualifiedCardinality "1"^^xsd:nonNegativeInteger ;
            owl:onDataRange xsd:string ;
            owl:onProperty <http://postdata.linhd.uned.es/ontology/postdata-core#nameLink> ],
        [ a owl:Restriction ;
            owl:allValuesFrom <http://postdata.linhd.uned.es/ontology/postdata-dates#DateEntity> ;
            owl:onProperty <http://postdata.linhd.uned.es/ontology/postdata-core#birthDate> ],
        [ a owl:Restriction ;
            owl:allValuesFrom <http://postdata.linhd.uned.es/ontology/postdata-core#Place> ;
            owl:onProperty <http://postdata.linhd.uned.es/ontology/postdata-core#birthPlace> ],
        [ a owl:Restriction ;
            owl:maxQualifiedCardinality "1"^^xsd:nonNegativeInteger ;
            owl:onClass [ a owl:Class ;
                    owl:intersectionOf ( skos:Concept [ a owl:Restriction ;
                                owl:hasValue <http://postdata.linhd.uned.es/kos/certainty> ;
                                owl:onProperty skos:inScheme ] ) ] ;
            owl:onProperty <http://postdata.linhd.uned.es/ontology/postdata-core#birthPlaceCertainty> ],
        [ a owl:Restriction ;
            owl:maxQualifiedCardinality "1"^^xsd:nonNegativeInteger ;
            owl:onClass [ a owl:Class ;
                    owl:intersectionOf ( skos:Concept [ a owl:Restriction ;
                                owl:hasValue <http://postdata.linhd.uned.es/kos/gender> ;
                                owl:onProperty skos:inScheme ] ) ] ;
            owl:onProperty <http://postdata.linhd.uned.es/ontology/postdata-core#gender> ],
        [ a owl:Restriction ;
            owl:maxQualifiedCardinality "1"^^xsd:nonNegativeInteger ;
            owl:onDataRange xsd:string ;
            owl:onProperty <http://postdata.linhd.uned.es/ontology/postdata-core#sourceNote> ],
        [ a owl:Restriction ;
            owl:allValuesFrom <http://postdata.linhd.uned.es/ontology/postdata-transmission#Location> ;
            owl:onProperty <http://postdata.linhd.uned.es/ontology/postdata-core#isReferencedIn> ],
        [ a owl:Restriction ;
            owl:allValuesFrom <http://postdata.linhd.uned.es/ontology/postdata-dates#DateEntity> ;
            owl:onProperty <http://postdata.linhd.uned.es/ontology/postdata-core#floruit> ],
        [ a owl:Restriction ;
            owl:allValuesFrom [ a owl:Class ;
                    owl:intersectionOf ( skos:Concept [ a owl:Restriction ;
                                owl:hasValue <http://postdata.linhd.uned.es/kos/certainty> ;
                                owl:onProperty skos:inScheme ] ) ] ;
            owl:onProperty <http://postdata.linhd.uned.es/ontology/postdata-core#birthPlaceCertainty> ],
        [ a owl:Restriction ;
            owl:maxQualifiedCardinality "1"^^xsd:nonNegativeInteger ;
            owl:onDataRange xsd:string ;
            owl:onProperty <http://postdata.linhd.uned.es/ontology/postdata-core#originalName> ],
        [ a owl:Restriction ;
            owl:maxQualifiedCardinality "1"^^xsd:nonNegativeInteger ;
            owl:onDataRange xsd:string ;
            owl:onProperty <http://postdata.linhd.uned.es/ontology/postdata-core#forename> ],
        [ a owl:Restriction ;
            owl:maxQualifiedCardinality "1"^^xsd:nonNegativeInteger ;
            owl:onDataRange xsd:string ;
            owl:onProperty <http://postdata.linhd.uned.es/ontology/postdata-core#surname> ],
        [ a owl:Restriction ;
            owl:allValuesFrom [ a owl:Class ;
                    owl:intersectionOf ( skos:Concept [ a owl:Restriction ;
                                owl:hasValue <http://postdata.linhd.uned.es/kos/religious-affiliation> ;
                                owl:onProperty skos:inScheme ] ) ] ;
            owl:onProperty <http://postdata.linhd.uned.es/ontology/postdata-core#religiousAffiliation> ],
        [ a owl:Restriction ;
            owl:allValuesFrom <http://postdata.linhd.uned.es/ontology/postdata-dates#DateEntity> ;
            owl:onProperty <http://postdata.linhd.uned.es/ontology/postdata-core#deathDate> ],
        [ a owl:Restriction ;
            owl:allValuesFrom [ a owl:Class ;
                    owl:intersectionOf ( skos:Concept [ a owl:Restriction ;
                                owl:hasValue <http://postdata.linhd.uned.es/kos/social-status> ;
                                owl:onProperty skos:inScheme ] ) ] ;
            owl:onProperty <http://postdata.linhd.uned.es/ontology/postdata-core#socialStatus> ],
        [ a owl:Restriction ;
            owl:allValuesFrom [ a owl:Class ;
                    owl:intersectionOf ( skos:Concept [ a owl:Restriction ;
                                owl:hasValue <http://postdata.linhd.uned.es/kos/school> ;
                                owl:onProperty skos:inScheme ] ) ] ;
            owl:onProperty <http://postdata.linhd.uned.es/ontology/postdata-core#school> ],
        [ a owl:Restriction ;
            owl:allValuesFrom [ a owl:Class ;
                    owl:intersectionOf ( skos:Concept [ a owl:Restriction ;
                                owl:hasValue <http://postdata.linhd.uned.es/kos/literary-period> ;
                                owl:onProperty skos:inScheme ] ) ] ;
            owl:onProperty <http://postdata.linhd.uned.es/ontology/postdata-core#literaryPeriod> ],
        [ a owl:Restriction ;
            owl:allValuesFrom <http://postdata.linhd.uned.es/ontology/postdata-core#Redaction> ;
            owl:onProperty <http://postdata.linhd.uned.es/ontology/postdata-core#isMentionedIn> ],
        <http://postdata.linhd.uned.es/ontology/postdata-core#Agent>,
        <http://xmlns.com/foaf/0.1/Person> .

skos:Concept a owl:Class .

skos:inScheme a owl:ObjectProperty .

<http://postdata.linhd.uned.es/ontology/postdata-core#Redaction> a owl:Class ;
    rdfs:label "Redaction"@en ;
    rdfs:comment """Representatives of a work, that is, of a Poetic Work. Each version and edition of a work is its own redaction.
Eg.: The palaeographic edition of A solis ortu usque ad occidua preserved in Lat. 1154 (BNF) and its critical edition are two Redaction of the same Poetic Work"""@en ;
    rdfs:isDefinedBy "http://postdata.linhd.uned.es/ontology/postdata-core/" ;
    rdfs:subClassOf [ a owl:Restriction ;
            owl:allValuesFrom <http://postdata.linhd.uned.es/ontology/postdata-core#Redaction> ;
            owl:onProperty <http://postdata.linhd.uned.es/ontology/postdata-core#hasSynthesis> ],
        [ a owl:Restriction ;
            owl:maxCardinality "1"^^xsd:nonNegativeInteger ;
            owl:onProperty <http://postdata.linhd.uned.es/ontology/postdata-core#audience> ],
        [ a owl:Restriction ;
            owl:allValuesFrom <http://postdata.linhd.uned.es/ontology/postdata-transmission#Location> ;
            owl:onProperty <http://postdata.linhd.uned.es/ontology/postdata-core#isIndexedIn> ],
        [ a owl:Restriction ;
            owl:allValuesFrom <http://postdata.linhd.uned.es/ontology/postdata-transmission#Location> ;
            owl:onProperty <http://postdata.linhd.uned.es/ontology/postdata-core#retrievesText> ],
        [ a owl:Restriction ;
            owl:maxCardinality "1"^^xsd:nonNegativeInteger ;
            owl:onProperty <http://postdata.linhd.uned.es/ontology/postdata-core#incipit> ],
        [ a owl:Restriction ;
            owl:maxQualifiedCardinality "1"^^xsd:nonNegativeInteger ;
            owl:onClass <http://postdata.linhd.uned.es/ontology/postdata-core#PoeticWork> ;
            owl:onProperty <http://postdata.linhd.uned.es/ontology/postdata-core#realises> ],
        [ a owl:Restriction ;
            owl:maxQualifiedCardinality "1"^^xsd:nonNegativeInteger ;
            owl:onClass <http://postdata.linhd.uned.es/ontology/postdata-structuralElements#Line> ;
            owl:onProperty <http://postdata.linhd.uned.es/ontology/postdata-structuralElements#hasFirstLine> ],
        [ a owl:Restriction ;
            owl:allValuesFrom <http://postdata.linhd.uned.es/ontology/postdata-transmission#Location> ;
            owl:onProperty <http://postdata.linhd.uned.es/ontology/postdata-core#hasTranslation> ],
        [ a owl:Restriction ;
            owl:allValuesFrom <http://postdata.linhd.uned.es/ontology/postdata-transmission#Location> ;
            owl:onProperty <http://postdata.linhd.uned.es/ontology/postdata-core#editedIn> ],
        [ a owl:Restriction ;
            owl:maxQualifiedCardinality "1"^^xsd:nonNegativeInteger ;
            owl:onDataRange xsd:string ;
            owl:onProperty <http://postdata.linhd.uned.es/ontology/postdata-core#paraphrasis> ],
        [ a owl:Restriction ;
            owl:maxQualifiedCardinality "1"^^xsd:nonNegativeInteger ;
            owl:onDataRange xsd:string ;
            owl:onProperty <http://postdata.linhd.uned.es/ontology/postdata-core#originalTitle> ],
        [ a owl:Restriction ;
            owl:onProperty <http://postdata.linhd.uned.es/ontology/postdata-core#hasCreator> ;
            owl:someValuesFrom <http://postdata.linhd.uned.es/ontology/postdata-core#CreatorRole> ],
        [ a owl:Restriction ;
            owl:allValuesFrom <http://postdata.linhd.uned.es/ontology/postdata-core#Redaction> ;
            owl:onProperty <http://postdata.linhd.uned.es/ontology/postdata-core#hasTranslation> ],
        [ a owl:Restriction ;
            owl:maxQualifiedCardinality "1"^^xsd:nonNegativeInteger ;
            owl:onClass <http://postdata.linhd.uned.es/ontology/postdata-core#Redaction> ;
            owl:onProperty <http://postdata.linhd.uned.es/ontology/postdata-core#isTranslationOf> ],
        [ a owl:Restriction ;
            owl:maxQualifiedCardinality "1"^^xsd:nonNegativeInteger ;
            owl:onDataRange xsd:string ;
            owl:onProperty <http://postdata.linhd.uned.es/ontology/postdata-core#narrativeLocation> ],
        [ a owl:Restriction ;
            owl:allValuesFrom <http://postdata.linhd.uned.es/ontology/postdata-core#Redaction> ;
            owl:onProperty <http://postdata.linhd.uned.es/ontology/postdata-core#isSynthesisOf> ],
        [ a owl:Restriction ;
            owl:allValuesFrom [ a owl:Class ;
                    owl:intersectionOf ( skos:Concept [ a owl:Restriction ;
                                owl:hasValue <http://postdata.linhd.uned.es/kos/textual-element-type> ;
                                owl:onProperty skos:inScheme ] ) ] ;
            owl:onProperty <http://postdata.linhd.uned.es/ontology/postdata-core#typeOfTextualElement> ],
        [ a owl:Restriction ;
            owl:maxQualifiedCardinality "1"^^xsd:nonNegativeInteger ;
            owl:onClass [ a owl:Class ;
                    owl:intersectionOf ( skos:Concept [ a owl:Restriction ;
                                owl:hasValue <http://postdata.linhd.uned.es/kos/rhymeMatching-type> ;
                                owl:onProperty skos:inScheme ] ) ] ;
            owl:onProperty <http://postdata.linhd.uned.es/ontology/postdata-prosodicElements#presentsRhymeMatching> ],
        [ a owl:Restriction ;
            owl:maxQualifiedCardinality "1"^^xsd:nonNegativeInteger ;
            owl:onDataRange xsd:string ;
            owl:onProperty <http://postdata.linhd.uned.es/ontology/postdata-core#unusedWitnesses> ],
        [ a owl:Restriction ;
            owl:allValuesFrom <http://postdata.linhd.uned.es/ontology/postdata-core#Role> ;
            owl:onProperty <http://postdata.linhd.uned.es/ontology/postdata-core#hasEditor> ],
        [ a owl:Restriction ;
            owl:maxQualifiedCardinality "1"^^xsd:nonNegativeInteger ;
            owl:onDataRange xsd:integer ;
            owl:onProperty <http://postdata.linhd.uned.es/ontology/postdata-core#numberOfWitnessesUsed> ],
        [ a owl:Restriction ;
            owl:maxQualifiedCardinality "1"^^xsd:nonNegativeInteger ;
            owl:onClass <http://postdata.linhd.uned.es/ontology/postdata-structuralElements#OrderedStanzaList> ;
            owl:onProperty <http://postdata.linhd.uned.es/ontology/postdata-structuralElements#hasStanzaItem> ],
        [ a owl:Restriction ;
            owl:allValuesFrom <http://postdata.linhd.uned.es/ontology/postdata-transmission#Location> ;
            owl:onProperty <http://postdata.linhd.uned.es/ontology/postdata-core#isReferencedIn> ],
        [ a owl:Restriction ;
            owl:maxQualifiedCardinality "1"^^xsd:nonNegativeInteger ;
            owl:onDataRange xsd:string ;
            owl:onProperty <http://postdata.linhd.uned.es/ontology/postdata-core#explicit> ],
        [ a owl:Restriction ;
            owl:allValuesFrom <http://postdata.linhd.uned.es/ontology/postdata-dates#DateEntity> ;
            owl:onProperty <http://postdata.linhd.uned.es/ontology/postdata-core#date> ],
        [ a owl:Restriction ;
            owl:maxQualifiedCardinality "1"^^xsd:nonNegativeInteger ;
            owl:onDataRange xsd:string ;
            owl:onProperty <http://postdata.linhd.uned.es/ontology/postdata-core#workNumber> ],
        [ a owl:Restriction ;
            owl:maxQualifiedCardinality "1"^^xsd:nonNegativeInteger ;
            owl:onClass <http://postdata.linhd.uned.es/ontology/postdata-prosodicElements#Pattern> ;
            owl:onProperty <http://postdata.linhd.uned.es/ontology/postdata-prosodicElements#isAnalysedThrough> ],
        [ a owl:Restriction ;
            owl:maxQualifiedCardinality "1"^^xsd:nonNegativeInteger ;
            owl:onClass <http://postdata.linhd.uned.es/ontology/postdata-structuralElements#OrderedLineList> ;
            owl:onProperty <http://postdata.linhd.uned.es/ontology/postdata-structuralElements#hasLineItem> ],
        [ a owl:Restriction ;
            owl:maxQualifiedCardinality "1"^^xsd:nonNegativeInteger ;
            owl:onDataRange [ a rdfs:Datatype ;
                    owl:unionOf ( xsd:language xsd:string ) ] ;
            owl:onProperty <http://postdata.linhd.uned.es/ontology/postdata-core#originalLanguage> ],
        [ a owl:Restriction ;
            owl:allValuesFrom <http://postdata.linhd.uned.es/ontology/postdata-core#Redaction> ;
            owl:onProperty <http://postdata.linhd.uned.es/ontology/postdata-core#isTranslationOf> ],
        [ a owl:Restriction ;
            owl:allValuesFrom <http://postdata.linhd.uned.es/ontology/postdata-core#CreatorRole> ;
            owl:onProperty <http://postdata.linhd.uned.es/ontology/postdata-core#hasCreator> ],
        [ a owl:Restriction ;
            owl:maxQualifiedCardinality "1"^^xsd:nonNegativeInteger ;
            owl:onDataRange xsd:string ;
            owl:onProperty <http://postdata.linhd.uned.es/ontology/postdata-core#text> ],
        [ a owl:Restriction ;
            owl:allValuesFrom <http://postdata.linhd.uned.es/ontology/postdata-core#OrderedTextUnitList> ;
            owl:onProperty <http://postdata.linhd.uned.es/ontology/postdata-core#hasOrderedTextUnitList> ],
        [ a owl:Restriction ;
            owl:allValuesFrom [ a owl:Class ;
                    owl:intersectionOf ( skos:Concept [ a owl:Restriction ;
                                owl:hasValue <http://postdata.linhd.uned.es/kos/genre> ;
                                owl:onProperty skos:inScheme ] ) ] ;
            owl:onProperty <http://postdata.linhd.uned.es/ontology/postdata-core#genre> ],
        [ a owl:Restriction ;
            owl:allValuesFrom <http://postdata.linhd.uned.es/ontology/postdata-core#Role> ;
            owl:onProperty <http://www.ontologydesignpatterns.org/cp/owl/objectrole.owl#hasRole> ],
        <http://iflastandards.info/ns/fr/frbr/frbroo/F22> .

[] owl:maxQualifiedCardinality "1"^^xsd:nonNegativeInteger .

[] owl:maxQualifiedCardinality "1"^^xsd:nonNegativeInteger .

[] a owl:AllDisjointClasses ;
    owl:members ( <http://postdata.linhd.uned.es/ontology/postdata-dates#ApproximateDateExpression> <http://postdata.linhd.uned.es/ontology/postdata-dates#ExactDateExpression> <http://postdata.linhd.uned.es/ontology/postdata-dates#IntervalExpression> ) .

